@prefix : <http://linked.data.gov.au/def/ra-vocab/> .               # this vocab's namespace
@prefix ca: <http://test.linked.data.gov.au/dataset/crs/ca/> .      # the register of CAs in the CRS dataset
@prefix crs: <http://linked.data.gov.au/def/crs#> .                 # the namespace of the CRS ontology
@prefix dct: <http://purl.org/dc/terms/> .
@prefix dct: <http://purl.org/dc/terms/> .
@prefix owl: <http://www.w3.org/2002/07/owl#> .
@prefix ra: <http://linked.data.gov.au/def/ra#> .                   # the namespace of the RA ontology
@prefix ras: <http://linked.data.gov.au/dataset/ra/> .              # a non-existing Dataset of Records Authorities
@prefix rdf: <http://www.w3.org/1999/02/22-rdf-syntax-ns#> .
@prefix rdfs: <http://www.w3.org/2000/01/rdf-schema#> .
@prefix sdo: <https://schema.org/> .
@prefix skos: <http://www.w3.org/2004/02/skos/core#> .
@prefix xsd: <http://www.w3.org/2001/XMLSchema#> .

:conceptScheme a skos:ConceptScheme ;
    rdfs:label "Records Authority Classes" ;
    rdfs:comment "Classes from Records Authories (formulated according to the Records Authority Ontology) with data from the NAA's internal database." ;
    dct:created "2019-07-10"^^xsd:date ;
    dct:modified "2019-08-26"^^xsd:date ;
    dct:source "NAA internal database." ;
    dct:creator [
            sdo:email <mailto:nicholas.car@surroundaustralia.com> ;
            sdo:identifier <http://orcid.org/0000-0002-8742-7730> ;
            sdo:affiliation [
                sdo:identifier <https://surroundaustralia.com> ;
                sdo:name "SURROUND Australia Pty Ltd"
            ] ;
            sdo:name "Nicholas J. Car" ;
    ] ;
    dct:contributor [
        sdo:email <mailto:information.governance@naa.gov.au> ;
        sdo:memberOf [
            sdo:identifier <http://catalogue.linked.data.gov.au/org/naa>
        ] ;
        sdo:name "National Archives of Australia, Information Governance Section"
    ] ;
    owl:versionIRI <http://linked.data.gov.au/def/ra-vocab/alpha> ;
    owl:versionInfo "For the LongSpine project testing" .


:0001  a crs:Function, ra:Class,
        skos:Concept ;
    crs:isPerformedBy [ crs:hasAgent ca:0001 ],
        [ crs:hasAgent ca:0001 ],
        [ crs:hasAgent ca:0001 ] ;
    dct:source ras:1999-00000104,
        ras:2009-00815192 ;
    skos:definition """The core business of managing the deliberations and administrative activities of statutory and non-statutory bodies established to provide independent advice to the Minister, government and the supporting agency. These bodies represent stakeholder communities and provide informed advice and guidance responding to issues as requested or as required in their charters. Covers advisory body meetings, advising and reporting on results of deliberations including consulting and liaising with interested parties through forums, conferences, workshops, visits and formal submissions. Includes managing the nomination, appointment and separation of advisory board members. Also includes the provision of secretariat support to advisory body members such as arranging meetings, organizing travel, arranging allowances and remuneration for duties performed and carrying out research. Excludes governing bodies that are a part of the management structure of an organization established to direct and support good governance practices.

Core business note:  Advisory bodies support the policy development, decision making and service delivery activities of government by providing informed and independent advice. Unlike Governing Bodies they have no executive or decision making powers and play no role in an agency’s governance activities.

This core business includes such advisory body related activities as:

•	providing advice to the Minister, the government and the supporting agency;
•	supporting the development of addresses (presentations);
•	arranging conferences and supporting members’ attendance at conferences;
•	undertaking consultations with interested parties;
•	administering members’ disclosures of interest;
•	managing meetings of advisory bodies and their committees;
•	managing membership of advisory bodies (ie appointments and separations); and
•	administering members’ remunerations arrangements.

The performance of the core business is supported by routine administrative tasks such as:

•	making arrangements to support journeys and visits;
•	managing media relationships;
•	planning, researching, reporting and reviewing; and
•	developing policies and procedures.
""";
    skos:inScheme :conceptScheme: ;
    skos:prefLabel "Advisory Bodies" .

:0002  a crs:Function, ra:Class,
        skos:Concept ;
    crs:isPerformedBy [ crs:hasAgent ca:0001 ] ;
    dct:source ras:2017-00324680 ;
    skos:definition """The function of supplying, maintaining, managing, repairing and disposing of moveable assets. Moveable assets may include equipment (eg instruments, tools, machines, plant, furniture and furnishings) and stores (eg chemicals, hardware, homeware items, kitchen/cleaning items, medical supplies and stationery) stocked and used by the organisation, as well as vehicles (ie any means of conveyance owned or used by the organisation to transport people or items).

Excludes:
•	information and communication technology equipment (eg computer hardware and software, multifunction copiers, phones, faxes, mobiles and other communication devices);
•	vehicles, equipment and stores acquired to support the Defence combat function; and
•	activities associated with the procurement of moveable assets, including selection and acquisition, leasing, tendering and contracting arrangements.

Note: Where agencies possess highly specialised or unique moveable assets with specific retention requirements (eg military equipment, scientific research equipment or nuclear materials), these should be covered within the agency’s own records authority.

The core activities include:
•	allocation, distribution and installation of moveable assets;
•	arranging use and storage of moveable assets, including managing arrangements for day-to-day vehicle use and arrangements for the delivery of moveable assets to an agency;
•	inspections and maintenance of moveable assets, including arranging vehicle maintenance and roadworthy inspections;
•	planning, conducting and facilitating audits, creating inventories and stocktaking;
•	leasing-out agency moveable assets to other bodies, including managing leases;
•	negotiating, establishing, managing and reviewing agreements and contracts (eg agreements to manage, maintain and dispose of equipment and stores; contracts leasing-out agency assets);
•	disposing of moveable assets, including leased assets, through any means including sale, transfer, auction, exchange, return and destruction;
•	managing insurance policies and claims covering moveable assets;
•	managing vehicle accidents, including arranging repairs;
•	handling breaches of rules, including handling operator or vehicle infringement notices;
•	managing asset warranties and related claims; and
•	securing and protecting moveable assets.

The performance of the function is supported by general activities such as:
•	developing policies, procedures and programs;
•	handling enquiries;
•	delegating powers and authorising actions (eg authorising use of vehicles);
•	establishing, managing and participating in committees and meetings;
•	fulfilling compliance requirements, including fiscal, legal, regulatory and quality standards and requirements;
•	planning and reporting;
•	evaluating and reviewing; and
•	identifying, assessing and managing risks.""";
    skos:inScheme :conceptScheme: ;
    skos:prefLabel "Asset Management" .

:0003  a crs:Function, ra:Class,
        skos:Concept ;
    crs:isPerformedBy [ crs:hasAgent ca:0001 ],
        [ crs:hasAgent ca:0001 ] ;
    dct:source ras:1999-00000104,
        ras:2009-00450477 ;
    skos:definition "The function of establishing rapport with the community and raising and maintaining the organisation's broad public profile. Includes marketing, advertising, media liaison, exhibitions, celebrations, ceremonies, speeches, official representation at functions and participation in community activities. Also includes relationships with professional bodies and industry, the management of customer services, handling reactions to those services, customer consultation and feedback.","""The function of establishing rapport with the community and raising and maintaining the organisation’s broad public profile.  Includes marketing, advertising, media liaison, exhibitions, celebrations, ceremonies, speeches, official representation at functions and participation in community activities.  Also includes relations with professional bodies and industry, the management of customer services, handling reactions to those services, customer consultations and feedback.

Function note: Where an agency has specific or unique relationships with the public Community Relations should not be used, rather these core business activities should be covered in the agency’s own Records Authority. For example exhibitions developed by the Australian War Memorial are central to its operations and would not be covered under Community Relations. Where an agency participates in a joint activity with another government agency, aimed at interacting with the community, and where the activity is not central to its operations, Community Relations should be used, rather than Government Relations.

This function includes such community relations activities as:

•	preparing and presenting addresses
•	arranging and managing agency events and attending external events including celebrations, ceremonies, conferences, exhibitions, social functions and visits
•	managing customer services, public reactions and media relations
•	receiving and making donations and seeking grant funding
•	receiving and responding to enquiries and suggestions
•	receiving and responding to greetings
•	managing joint venture arrangements
•	marketing activities
•	representing the agency on community organisations and liaising
•	managing security arrangements
•	making submissions; and
•	arranging visits.

The performance of the function is supported by routine administrative tasks such as:

• making arrangements
• managing committees and meetings
• evaluating and reviewing
• planning
• researching and reporting; and
• developing policies and procedures.""";
    skos:inScheme :conceptScheme: ;
    skos:prefLabel "Community Relations" .

:0004  a crs:Function, ra:Class,
        skos:Concept ;
    crs:isPerformedBy [ crs:hasAgent ca:0001 ],
        [ crs:hasAgent ca:0001 ] ;
    dct:source ras:1999-00000104,
        ras:2009-00450477 ;
    skos:definition "The function of providing compensation to personnel and visitors injured while proceeding to or from work, during working hours or on the organisation's premises. Includes the rehabilitation of injured workers and compensation for damage to property where such damage is claimed as the organisation's responsibility. This function excludes Defence military personnel.","""The function of providing compensation to personnel and visitors injured while proceeding to or from work, during working hours or on the organisation’s premises.  Includes the rehabilitation of injured workers and compensation for damage to property where such damage is claimed as the organisation’s responsibility.  This function excludes Defence military personnel.

Function note:  Compensation is one of the of AFDA Express suite of functions covering the management of an agency’s human resources.  Others are – Establishment, Industrial Relations, Occupational Health & Safety (OH&S), Personnel, and Staff Development.  This function covers staff and the public who have sustained injuries at work or when visiting the agency and lodged a compensation claim.  The two functions most closely linked to Compensation are OH&S, which aims at establishing and implementing preventative health and safety measures and Personnel, which manages the engagement of individual staff members and their conditions of employment with the APS.  Personnel also covers the rehabilitation of employees who have been injured but have not lodged a compensation claim.

Records of all current and finalized asbestos-related claims for compensation must be transferred to the central agency, with legislative responsibility for the management of asbestos liability in the Commonwealth (currently Comcare) under the Asbestos-related Claims (Management of Commonwealth Liabilities) Act 2005.

The function includes such compensation related activities as:

•	taking out insurance and managing claims; and
•	managing compensation cases, including appealing decisions, entering into agreements and any subsequent rehabilitation activities.

The performance of the function is supported by routine administrative tasks such as:

•	providing and receiving advice;
•	managing committees;
•	fulfilling compliance requirements;
•	delegating powers and authorising actions;
•	developing policies and procedures;
•	reporting;
•	reviewing the management of the function; and
•	managing risks.""";
    skos:inScheme :conceptScheme: ;
    skos:prefLabel "Compensation",
        "Compensation  " .

:0005  a crs:Function, ra:Class,
        skos:Concept ;
    crs:isPerformedBy [ crs:hasAgent ca:0001 ] ;
    dct:source ras:2019-00026231 ;
    skos:definition """The business activities related to developing and executing formal contracts under seal or deeds (also known as deeds under seal, speciality, speciality contracts) that set out a binding promise, commitment or obligation usually not involving a consideration (ie a payment of some kind), and state that it is executed or signed as a deed. Includes managing deeds (eg deeds of transfer, deeds of gift) relating to the acquisition and transfer of property. The making of the deed needs to follow certain formalities and is subject to specific time periods set down in State and Territory legislation. Excludes simple contracts, agreements and memoranda of understanding.

The core activities include:
•	negotiating with parties on terms and conditions;
•	identifying, assessing and managing risks;
•	drawing up the contract under seal/deed;
•	executing the document as legally required;
•	registering the document with the relevant State or Territory authority;
•	administering the deed;
•	managing any variations or extensions;
•	managing breaches; and
•	managing the termination and discharge of the deed.""";
    skos:inScheme :conceptScheme: ;
    skos:prefLabel "Contracts Under Seal/Deeds" .

:0006  a crs:Function, ra:Class,
        skos:Concept ;
    crs:isPerformedBy [ crs:hasAgent ca:0001 ],
        [ crs:hasAgent ca:0001 ] ;
    dct:source ras:1999-00000104,
        ras:2009-00450477 ;
    skos:definition "The function of acquiring, supplying, maintaining, repairing and disposing of equipment and stores stocked and used by the organisation.  Items of equipment include instruments, implements, tools, machines, plant, furniture and furnishings.  Stores include chemicals, hardware, homeware items, kitchen/cleaning items, medical supplies and stationery.  Excludes equipment and stores acquired to support the Defence combat function.","""The function of supplying, maintaining, repairing and disposing of equipment and stores stocked and used by the organisation.  Items of equipment include instruments, tools, machines, plant, furniture and furnishings.  Stores include chemicals, hardware, homeward items, kitchen/cleaning items, medical supplies and stationery.  Excludes equipment and stores acquired to support the Defence combat function.

Function note:  Equipment & Stores is one of the AFDA Express functions that relates to managing agency assets.  The other asset management functions are – Fleet Management, Property Management and Technology and Telecommunications.  Equipment & Stores covers portable and less durable assets, but not computer and telecommunications equipment.  The function Technology & Telecommunications should be used for managing computer hardware and software and phones, faxes, mobiles and other communication devices.  The evaluation and selection of equipment and stores, and the subsequent acquisition of those items, through leasing, tendering and contracting arrangements, is covered by the Procurement function.

The function includes such equipment and stores related activities as:

•	establishing and managing agreements;
•	allocation and distribution;
•	arranging use and storage;
•	auditing, creating inventories and stocktaking;
•	contracting-out (not related to procurement activities;
•	disposing of items;
•	installation, inspections and maintenance;
•	managing insurance policies and claims; and
•	securing and protecting.

The performance of the function is supported by routine administrative tasks such as:

•	fulfilling compliance requirements;
•	delegating powers and authorising actions;
•	developing policies and procedures;
•	reviewing and reporting; and
•	managing risks.""";
    skos:inScheme :conceptScheme: ;
    skos:prefLabel "Equipment & Stores",
        "Equipment & Stores  " .

:0007  a crs:Function, ra:Class,
        skos:Concept ;
    crs:isPerformedBy [ crs:hasAgent ca:0001 ],
        [ crs:hasAgent ca:0001 ] ;
    dct:source ras:1999-00000104,
        ras:2009-00450477 ;
    skos:definition "The function of establishing and changing the organisational structure.  Including moving employees from one agency to another and reducing and increasing an agency's staffing levels.  Also includes internal reorganisations to meet agency goals.","""The function of establishing and changing the organisational structure.  Including moving employees from one agency to another and reducing and increasing an agency’s staffing levels.  Also includes internal reorganisations to meet agency goals.

Function note:  Establishment is one of the AFDA Express suite of functions covering the management of an agency’s human resources.  Others are – Compensation, Industrial Relations, Occupational Health & Safety (OH&S), Personnel, and Staff Development. Establishment relates to managing the overall administrative structure of an agency to ensure it meets its assigned role within government.  It is closely related to Personnel.  Under the Establishment function the structure of the agency is developed, including the nomination, classification and allocation of duties and under Personnel staff are recruited to fill those positions.

Before using this Authority, agencies that employ staff under legislation other than the Public Service Act 1999 should check their own enabling legislation and other regulatory directives for major variations from this Act.  In cases where the variations differ greatly the AFDA and consequently AFDA Express is not applicable and should not be used.  In such circumstances relevant classes must be included under the agency’s own Records Authority.

The function includes such Establishment related activities as:

•	restructuring;
•	setting work level standards; and
•	creating and abolishing positions (managing variations).

The performance of the function is supported by routine administrative tasks such as:

•	providing and receiving advice;
•	managing committees and meetings;
•	delegating powers and authorising actions;
•	planning;
•	developing policies and procedures;
•	evaluating and reviewing; and
•	reporting.
""";
    skos:inScheme :conceptScheme: ;
    skos:prefLabel "Establishment" .

:0008  a crs:Function, ra:Class,
        skos:Concept ;
    crs:isPerformedBy [ crs:hasAgent ca:0001 ],
        [ crs:hasAgent ca:0001 ] ;
    dct:source ras:1999-00000104,
        ras:2009-00450477 ;
    skos:definition "The function of managing the organisation's financial resources.  Includes establishing, operating, and maintaining accounting systems, controls and procedures, financial planning, framing budgets and budget submissions, obtaining grants, managing funds in the form of allocations from the Consolidated Revenue Fund and revenue from charging, trading and investments. Also includes the monitoring and analysis of assets to assist the delivery of economic and social services to government, industry and the community.","""The function of managing the organisation’s financial resources.  Includes establishing, operating, and maintaining accounting systems, controls and procedures, financial planning, framing budgets and budget submissions, obtaining grants, managing funds in the form of allocations from the Consolidated Revenue Fund and revenue from charging, trading and investments.  Also includes the monitoring and analysis of assets to assist the delivery of economic and social services to government, industry and the community.

Function note: The Financial Management function supports the allocation and spending of funds to support the performance of all other general administrative functions and agency core businesses. Closely linked is the Strategic Management function which sets the overall goals and objectives of an agency and the allocation of resources.  It is also linked to the Procurement function which manages the acquisition of goods and services to support the performance of an agency’s business.

This function includes such financial management activities as:

•	keeping the agency’s principal accounting records;
•	providing and receiving advice;
•	managing agreements;
•	managing the agency’s asset register;
•	auditing and inventory management;
•	budgeting and allocating funds;
•	adopting fraud control measures;
•	preparing financial statements;
•	managing grant funding and donations;
•	paying accounts/salaries;
•	standards implementation; and
•	treasury management.

The performance of the function is supported by routine administrative tasks such as:

•	managing committees and meetings;
•	fulfilling compliance requirements;
•	delegating powers and authorising actions;
•	planning and reporting;
•	developing policies and procedures;
•	reviewing and evaluating; and
•	risk management.

""";
    skos:inScheme :conceptScheme: ;
    skos:prefLabel "Financial Management",
        "Financial Management  " .

:0009  a crs:Function, ra:Class,
        skos:Concept ;
    crs:isPerformedBy [ crs:hasAgent ca:0001 ] ;
    dct:source ras:2017-00324183 ;
    skos:definition """The function of managing the organisation’s financial resources includes establishing, operating, and maintaining accounting systems, controls and procedures, financial planning and analysis, framing budgets and budget submissions, obtaining grants, managing funds in the form of allocations from the Consolidated Revenue Fund and revenue from charging, trading and investments, and allocation and spending of funds to support the performance of agency functions. It also includes the monitoring and analysis of assets to assist the delivery of economic and social services to government, industry and the community.

The core activities include:
•	keeping the agency’s principal accounting records, including managing the agency’s revenue and expenditure;
•	collecting and analysing information on financial transactions and on the financial position and operating results of the agency;
•	implementing, maintaining and monitoring accounting systems and internal financial controls;
•	providing and receiving advice;
•	negotiating, establishing, managing and reviewing agreements and contracts;
•	establishing and managing the agency’s asset register;
•	budgeting and allocating funds, including production of whole of agency budget estimates;
•	managing taxation matters;
•	establishing agency bank accounts and managing banking activities, including managing credit card accounts;
•	adopting fraud control measures and identification of specific instances of fraud;
•	preparing and compiling financial statements, showing income and expenditure, assets and liabilities;
•	preparation and payment of money, including checking invoices, paying accounts, settling claims, paying grants to external recipients, and paying salaries and allowances;
•	receiving monetary payments, including receipt of dividends and revenue from agency activities;
•	managing financial transactions associated with monetary donations made or received by the agency, including results of fundraising;
•	managing grant funding received by the agency;
•	planning, conducting and facilitating audits;
•	managing incidental benefits received by agency personnel (eg frequent flyer points);
•	inventory management supporting the financial management function (eg inventories of cab charge vouchers);
•	managing debt recovery; and
•	treasury management, including managing the agency’s funds, trusts, investments, unclaimed moneys and loans.

The performance of the function is supported by general activities such as:
•	developing policies and procedures;
•	establishing, managing and participating in committees and meetings;
•	fulfilling compliance requirements, including fiscal, legal, regulatory and quality standards and requirements;
•	delegating powers and authorising actions;
•	planning and reporting;
•	handling internal enquiries;
•	evaluating and reviewing; and
•	identifying, assessing and managing risks.""";
    skos:inScheme :conceptScheme: ;
    skos:prefLabel "Financial Management 17" .

:0010  a crs:Function, ra:Class,
        skos:Concept ;
    crs:isPerformedBy [ crs:hasAgent ca:0001 ],
        [ crs:hasAgent ca:0001 ] ;
    dct:source ras:1999-00000104,
        ras:2009-00450477 ;
    skos:definition "The function of acquiring (either by purchase, leasing or chartering), managing, maintaining, repairing and disposing of vehicles.  Vehicles are any means of conveyance owned or used by the organisation to transport people or items. Excludes vehicles acquired to support the Defence combat function, but includes all other special purpose vehicles.","""The function of managing, maintaining, repairing and disposing of vehicles.  Vehicles are any means of conveyance owned or used by the organisation to transport people or items.  Excludes vehicles acquired to support the Defence combat function, but includes all other special purpose vehicles.

Function note: Fleet Management is one of the AFDA Express functions that relates to managing agency assets.  The other asset management functions are – Equipment & Stores, Property Management and Technology & Telecommunications.  The evaluation and selection of vehicles, and the subsequent acquisition of those items, through leasing, tendering and contracting arrangements, is covered by the Procurement function.

The function includes such fleet management related activities as:

•	managing vehicle accidents;
•	managing agreements;
•	arranging vehicle allowances;
•	managing arrangements for day-to-day vehicle use;
•	disposal;
•	handling infringements;
•	taking out insurance and managing claims; and
•	vehicle maintenance.

The performance of the function is supported by routine administrative tasks such as:

•	managing committees and meetings;
•	fulfilling compliance requirements;
•	delegating powers and authorising actions;
•	developing policies and procedures; and
•	reporting.

""";
    skos:inScheme :conceptScheme: ;
    skos:prefLabel "Fleet Management",
        "Fleet Management  " .

:0011  a crs:Function, ra:Class,
        skos:Concept ;
    crs:isPerformedBy [ crs:hasAgent ca:0001 ],
        [ crs:hasAgent ca:0001 ] ;
    dct:source ras:1999-00000104,
        ras:2010-00182807 ;
    skos:definition """The business of establishing membership and managing the administration of governing bodies, such as boards, trusts, councils, commissions and so on, that direct, oversee or provide a framework for the control of an organisation.  Includes governing bodies regulated by the Commonwealth Authorities and Companies Act 1997 (or its equivalent).  Covers activities associated with providing secretariat support to the governing body in the performance of its duties and administrative support to governing body members, including arrangements for travel, leave entitlements, allowances and remuneration for duties performed.  Also includes the nomination, election, appointment and separation of governing body members, disclosures of pecuniary interests, professional indemnity insurance, relations between an organisation and its governing body and meetings of governing bodies.  Excludes governing bodies that do not undertake a governance role.

Note:  Governing Bodies is a business area relating to the agency’s governance management.  The other governance business area is Strategic Management which covers broad systematic administration, planning and reporting.  The focus of the Governing Bodies is the establishment and day-to-day administration of an agency’s internal governing authority.  The activities of the governing body support other business areas, in particular Community Relations, Government Relations, Strategic Management, and all other agency core businesses where they are covered.

Governing bodies does not cover the activities of advisory bodies. Governing bodies have executive powers and focus on administrative control of an agency’s governance framework while advisory bodies provide informed advice to the Minister, the Government and the agency.  Advisory bodies undertake no role in governance activities.  Their administration and operations are covered by a separate general records authority issued by the National Archives.

This business area includes such governing bodies related activities as:

•	managing accidents involving members of governing bodies;
•	supporting the development of addresses (presentations);
•	negotiating and establishing agreements (eg contracts of appointments);
•	handling appeals;
•	managing compensation cases;
•	managing disclosures of interest;
•	administering leave;
•	administering meetings of governing bodies;
•	managing membership of governing bodies (i.e. establishment and composition);
•	supporting performance management frameworks;
•	managing remuneration arrangements; and
•	supporting training requirements.

The performance of the business area is supported by routine administrative tasks such as:

•	providing and receiving advice;
•	complying with external management requirements;
•	delegating powers and authorising actions;
•	managing insurance and claims;
•	managing administrative meetings;
•	planning, researching, reporting and reviewing; and
•	developing policies and procedures.
""";
    skos:inScheme :conceptScheme: ;
    skos:prefLabel "Governing Bodies" .

:0012  a crs:Function, ra:Class,
        skos:Concept ;
    crs:isPerformedBy [ crs:hasAgent ca:0001 ],
        [ crs:hasAgent ca:0001 ] ;
    dct:source ras:1999-00000104,
        ras:2009-00450477 ;
    skos:definition "The function of administering the formal relationship between the organisation and those processes of government not covered by general administrative or agency core functions.  Includes the organisation's relationship with Ministers and Members of Parliament and the political processes of Government; liaison with bodies carrying out investigations and participating in formal inquiries and investigations such as Royal Commissions, and inquiries by Parliamentary Committees and the Ombudsman; and relationships with Local, State, or overseas governments.","""The function of administering the formal relationship between the organisation and those processes of government not covered by other general administrative or agency core businesses.  Includes the organisation’s relationship with Ministers and Members of Parliament and the political processes of Government; liaison with bodies carrying out investigations and participating in formal inquiries and investigations such as Royal Commissions, and inquiries by Parliamentary Committees and the Ombudsman; and relationship with Local, State or overseas governments.

Function note:  This function should only be used if the agency’s Records Authority does not include relevant classes, or if activities are not covered in another AFDA Express function eg Financial Management should be used to cover interaction between the agency and the Department of Finance and Deregulation and Compensation and OH&S should be used for interactions between the agency and Comcare.  Communications between the public (individuals and groups) relating to the responsibilities and actions of the agency, received by the Minister (‘Ministerials’), are covered by the Government Relations function.

The function includes government relations activities such as:

•	preparing addresses and presentations;
•	providing advice;
•	agency liaison;
•	managing agreements and joint ventures;
•	managing committees and meetings;
•	fulfilling compliance requirements;
•	managing customer services;
•	contributing to inquiries;
•	preparing legislation for presentation in Parliament;
•	managing media relations;
•	developing policies and procedures;
•	researching, reporting and reviewing;
•	responding to representations from Members of Parliament and the public (‘Ministerials’);
•	managing staff representatives on government bodies;
•	managing security requirements for government representatives;
•	making submissions; and
•	arranging visits.

""";
    skos:inScheme :conceptScheme: ;
    skos:prefLabel "Government Relations" .

:0013  a crs:Function, ra:Class,
        skos:Concept ;
    crs:isPerformedBy [ crs:hasAgent ca:0001 ],
        [ crs:hasAgent ca:0001 ] ;
    dct:source ras:1999-00000104,
        ras:2009-00450477 ;
    skos:definition "The function of establishing formal relations with the organisation's employees and their representatives to achieve a harmonious workplace.  Includes negotiations conducted to obtain determinations, agreements or awards, industrial disputes settled within the organisation or by an external arbitrator and reports of the state of industrial relations within an organisation.","""The function of establishing formal relations with the organisation’s employees and their representatives to achieve a harmonious workplace.  Includes negotiations conducted to obtain determinations, agreements or awards, industrial disputes settled within the organisation or by an external arbitrator and reports of the state of industrial relations within an organisation.

Function note:  Industrial Relations is one of the of AFDA Express suite of functions covering the management of an agency’s human resources.  Others functions are – Compensation, Establishment, Occupational Health & Safety (OH&S), Personnel and Staff Development.  Industrial Relations establishes and manages the overall relationships between management and agency staff.  It is closely linked to the Personnel function which covers the engagement of individual staff members and their conditions of employment.

This function includes such industrial relations related activities as:

•	negotiating, establishing and maintaining awards and agreements;
•	managing appeals to central arbitration or determining body;
•	handling disputes;
•	undertaking enterprise bargaining negotiations;
•	handling grievances;
•	managing industrial action;
•	handling infringements; and
•	undertaking inspections.

The performance of the function is supported by routine administrative tasks such as:

•	providing and receiving advice;
•	organising allowances;
•	managing committees and meetings;
•	fulfilling compliance requirements;
•	managing insurance and claims;
•	planning;
•	developing policies and procedures;
•	reporting and research; and
•	managing risk.

""";
    skos:inScheme :conceptScheme: ;
    skos:prefLabel "Industrial Relations" .

:0014  a crs:Function, ra:Class,
        skos:Concept ;
    crs:isPerformedBy [ crs:hasAgent ca:0001 ],
        [ crs:hasAgent ca:0001 ] ;
    dct:source ras:1999-00000104,
        ras:2009-00450477 ;
    skos:definition "The function of managing the organisation's information resources. Includes creating, capturing, registering, classifying, indexing, storing, retrieving and disposing of records and developing strategies to manage records. Also includes the acquisition, control and disposal of library and other information products, items kept for reference purposes and the provision of services to internal and external customers, based on information resources. Data administration, archival records and the handling of Freedom of Information (FOI) requests are also classified under this keyword.","""The function of managing the organisation’s information resources.  Includes creating, capturing, registering, classifying, indexing, storing, retrieving and disposing of records and developing strategies to manage records.  Also includes the control and disposal of library and other information products, items kept for reference purposes and the provision of services to internal and external customers, based on information resources.  Data administration, archival records and the handling of Freedom of Information (FOI) requests are also classified under this keyword.

Function note:  Information Management is one of the AFDA Express functions relating to the management of an agency’s information and knowledge resources.  The other function is Publication.  The Information Management function covers all library and reference material and records created to support the performance of an agency’s business activities.  Publication covers published works created for distribution by the agency.

This function includes such information management related activities as:

•	managing access requests to information under FOI, Archives Act and Privacy Act;
•	negotiating and establishing agreements;
•	conserving, maintaining and restoring;
•	controlling information sources;
•	handling customer services, enquiries and suggestions;
•	data administration;
•	disposing of records and publications;
•	distributing information sources;
•	managing donations;
•	supporting inspections;
•	managing intellectual property;
•	creating inventories;
•	marketing;
•	administering privacy requirements;
•	managing information security;
•	administering standards; and
•	preparing submissions.

The performance of the function is supported by routine administrative tasks such as:

•	providing advice;
•	auditing;
•	managing committees and meetings;
•	fulfilling compliance requirements;
•	delegating powers and authorising actions;
•	managing insurance and claims;
•	planning;
•	developing policies and procedures;
•	researching and reporting;
•	reviewing and evaluating; and
•	managing risks.

""";
    skos:inScheme :conceptScheme: ;
    skos:prefLabel "Information Management",
        "Information Management  " .

:0015  a crs:Function, ra:Class,
        skos:Concept ;
    crs:isPerformedBy [ crs:hasAgent ca:0001 ],
        [ crs:hasAgent ca:0001 ],
        [ crs:hasAgent ca:0001 ] ;
    dct:source ras:1999-00000104,
        ras:2009-00450477,
        ras:2017-00491822 ;
    skos:definition """The function of providing legal services to the organisation.  Includes the interpretation and provision of advice to the organisation regarding legal matters, the drawing up of legal agreements and the handling of legal actions and disputes.  Also includes legal advice received from in-house consultants and external sources.

Function note:  Legal Services, covering the provision of specialist legal advice, supports all general administrative AFDA Express functions and agency core businesses.

This function includes such legal services activities as:

•	managing claims;
•	supporting the conduct or participation in inquiries;
•	managing infringements;
•	managing intellectual property;
•	providing legal advice; and
•	handling litigation.


The performance of the function is supported by routine administrative tasks such as:

•	managing agreements;
•	managing committees and meetings;
•	fulfilling compliance requirements;
•	delegating powers and authorising actions;
•	planning;
•	developing policies and procedures;
•	researching and reporting;
•	reviewing; and
•	managing risks.

""",
        "The function of providing legal services to the organisation. Includes the interpretation and provision of advice to the organisation regarding legal matters, the drawing up of legal agreements and the handling of legal actions and disputes. Also includes legal advice received from in-house consultants and external sources." ;
    skos:inScheme :conceptScheme: ;
    skos:prefLabel "Legal Services",
        "Legal Services  " .

:0016  a crs:Function, ra:Class,
        skos:Concept ;
    crs:isPerformedBy [ crs:hasAgent ca:0001 ] ;
    dct:source ras:2009-00450477 ;
    skos:definition """The function of implementing and coordinating occupational health and safety and associated legislation throughout the organisation.  Includes safety, occupational hygiene, ergonomic, occupational medicine and first aid measures together with policy, procedural and monitoring matters associated with the organisation's preventive and curative OH&S program.  Includes the establishment of committees to investigate and advise on health and safety issues in the workplace.

Function note:  Occupational Health & Safety is one of the of AFDA Express suite of functions covering the management of an agency’s human resources.  Others are – Compensation, Establishment, Industrial Relations, Personnel, and Staff Development.  The OH&S function aims at establishing and implementing preventative health and safety measures. The two functions most closely linked to OH&S are Compensation, which covers the provision of compensation to those who have sustained injuries and Personnel, which manages the engagement of individual staff members and their conditions of employment with the APS.  Staff Development should be used for OH&S training, including the handling of hazardous substances.

The function includes such OH&S related activities as:

•	accident management;
•	providing advice;
•	managing agreements;
•	managing appeals to the Australian Industrial Relations Commission;
•	auditing, inspecting and reviewing;
•	managing committees and meetings;
•	fulfilling compliance requirements;
•	delegating powers and authorising actions;
•	health surveillance, promotion, provision of first aid treatment and preventive measures;
•	inquiry management;
•	planning;
•	developing policies and procedures;
•	reporting and researching;
•	nominating and electing OH&S representatives;
•	managing risks; and
•	implementing standards.

""";
    skos:inScheme :conceptScheme: ;
    skos:prefLabel "Occupational Health & Safety (Oh & S)" .

:0017  a crs:Function, ra:Class,
        skos:Concept ;
    crs:isPerformedBy [ crs:hasAgent ca:0001 ] ;
    dct:source ras:1999-00000104 ;
    skos:definition "The function of implementing and coordinating occupational health and safety and associated legislation throughout the organisation.  Includes safety, occupational hygiene, ergonomic, occupational medicine and first aid measures together with policy, procedural and monitoring matters associated with the organisations' preventive and curative OH&S program.  Includes the establishment of committees to investigate and advise on health and safety issues in the workplace." ;
    skos:inScheme :conceptScheme: ;
    skos:prefLabel "Occupational Health & Safety (Oh&S)" .

:0018  a crs:Function, ra:Class,
        skos:Concept ;
    crs:isPerformedBy [ crs:hasAgent ca:0001 ],
        [ crs:hasAgent ca:0001 ] ;
    dct:source ras:1999-00000104,
        ras:2009-00450477 ;
    skos:definition """The function of managing all employees in the organisation employed under the Public Service Act 1999 and previous legislation and volunteer workers.  Includes review of actions, overtime, salaries, superannuation and working hours for individuals.

Function note:  Personnel is one of the of AFDA Express suite of functions covering the management of an agency’s human resources.  Others functions are – Compensation, Establishment, Industrial Relations, Occupational Health & Safety (OH&S), and Staff Development.  The Personnel function covers the engagement of individual staff members and their conditions of employment, including appraising performance and resolving disputes.  Compensation supports employees who have sustained injuries while at work; Establishment covers setting up and changing the organisational structure; OH&S relates to implementing and coordinating preventative health and safety measures in the workplace; Industrial Relations establishes and manages the overall relationship between management and agency employees and Staff Development supports the development of staff skills and abilities.

Before using this Authority, agencies who employ staff under legislation other than the Public Service Act 1999, should check their own enabling legislation and other regulatory directives for major variations from the Public Service Act in scope and conditions of employment.  In cases where the variations differ greatly AFDA and consequentially AFDA Express is not applicable and should not be used.  In such circumstances relevant classes must be included under the agency’s own Records Authority.

This function includes such personnel related activities as:

•	negotiating and establishing employment agreements (eg AWAs);
•	managing allowances;
•	managing conditions of employment for individual workers;
•	counselling;
•	handling grievances, disciplinary action and appeals;
•	handling infringements;
•	managing insurance and claims;
•	administering leave;
•	moving personnel;
•	supporting performance management frameworks;
•	managing recruitment and separation from the APS;
•	administering rehabilitation not related to a compensation case;
•	arranging staff representations;
•	administering salaries;
•	overseeing personnel security requirements;
•	supporting social clubs; and
•	seeking and using staff suggestions.

The performance of the function is supported by routine administrative tasks such as:

•	providing and receiving advice;
•	managing committees and meetings;
•	fulfilling compliance requirements;
•	delegating powers and authorising actions;
•	planning;
•	developing policies and procedures;
•	reporting; and
•	reviewing and evaluating.

""",
        "The function of managing all employees in the organisation employed under the Public Service Act 1999 and previous legislation and volunteer workers. Includes review of actions, overtime, salaries, superannuation and working hours for individuals." ;
    skos:inScheme :conceptScheme: ;
    skos:prefLabel "Personnel",
        "Personnel  " .

:0019  a crs:Function, ra:Class,
        skos:Concept ;
    crs:isPerformedBy [ crs:hasAgent ca:0001 ],
        [ crs:hasAgent ca:0001 ] ;
    dct:source ras:1999-00000104,
        ras:2009-00450477 ;
    skos:definition """The function of obtaining goods and services to support an agency’s business, including the services of consultants and contractors.  Includes the activities of acquisition, agreements, contracting-out and tendering.  Also includes the development and review of policies and procedures to support the function, planning the procurement process, assessment and management of associated risks, auditing, authorisation of delegates and reporting.  Excludes acquisition of land and construction of buildings, and procurement undertaken to support the Defence combat function.

Function note:  Procurement covers both simple purchases and complex contractual acquisition processes to obtain goods and services needed to support the performance of administrative functions and agency core businesses.  It is closely linked to the Financial Management function through managing financial transactions associated with the procurement activities.

This function includes such procurement activities as:

•	acquiring goods and services;
•	negotiating, establishing, maintaining and reviewing agreements;
•	complaint handling;
•	undertaking and managing construction works;
•	contracting-out;
•	evaluating goods and services;
•	leasing; and
•	tendering and finalising contracts.

The performance of the function is supported by routine administrative tasks such as:

•	providing advice;
•	auditing;
•	managing committees and meetings;
•	fulfilling compliance requirements;
•	delegating powers and authorising actions;
•	planning;
•	developing policies and procedures;
•	reviewing and reporting; and
•	managing risks.

""",
        "The function of obtaining goods and services to support an agency’s business, including the services of consultants and contractors. Includes the activities of acquisition, agreements, contracting-out and tendering. Also includes the development and review of policies and procedures to support the function, planning the procurement process, assessment and management of associated risks, auditing, authorisation of delegations and reporting. Excludes acquisition of land and construction of buildings. Also excludes procurement undertaken to support the Defence combat function.  " ;
    skos:inScheme :conceptScheme: ;
    skos:prefLabel "Procurement",
        "Procurement  " .

:0020  a crs:Function, ra:Class,
        skos:Concept ;
    crs:isPerformedBy [ crs:hasAgent ca:0001 ] ;
    dct:source ras:2018-00546118 ;
    skos:definition "PROCUREMENT 2018" ;
    skos:inScheme :conceptScheme: ;
    skos:prefLabel "Procurement 2018" .

:0021  a crs:Function, ra:Class,
        skos:Concept ;
    crs:isPerformedBy [ crs:hasAgent ca:0001 ],
        [ crs:hasAgent ca:0001 ] ;
    dct:source ras:1999-00000104,
        ras:2009-00450477 ;
    skos:definition """The function of managing land and working, storage or living spaces within premises, and of acquiring, constructing, fitting-out, managing, maintaining, protecting and disposing of premises.  Includes the removal of pollutants and waste.  This function also covers properties owned by the Commonwealth or Commonwealth institutions which have national significance including natural, historic and indigenous significance and are listed in the Register of the National Estate, by the World Heritage Commission, classified by the National Trusts or on State heritage listings.

Function Note: Property Management is one of the AFDA Express functions that relates to managing agency assets.  The other asset management functions are – Equipment & Stores, Fleet Management and Technology & Telecommunications.  The Property Management function covers the acquisition, maintenance, use and disposal of land and buildings.

Care should be taken when using this function for records covering the management of specialised premises, i.e. purpose-built, specialised premises supporting core functions, or with unique design features eg army barracks, immigration detention centres, Lucas Heights Nuclear Reactor Building or Mt Stromlo Observatory.  While this function should provide classes that cover most property management matters relating to specialised premises, there may be unique requirements that will necessitate specific classes for specialised premises within an agency's own Records Authority.

This function includes such property management related activities as:

•	acquiring (including compulsory acquisition) purchasing and leasing;
•	managing compensation appeals;
•	constructing, conserving and carrying out enhancements;
•	disposing of property;
•	implementing disaster plans;
•	carrying out inspections (routine and to determine the existence of contaminants);
•	managing fit-outs;
•	installing equipment;
•	maintaining properties;
•	undertaking inventories;
•	managing lost property;
•	arranging moves;
•	removing hazardous material; and
•	managing property security.

The performance of the function is supported by routine administrative tasks such as:

•	providing advice;
•	establishing and managing agreements;
•	managing routine arrangements for the use of properties;
•	managing internal and external audits;
•	managing committees and meetings;
•	fulfilling compliance requirements;
•	managing contracting-out arrangements;
•	delegating powers and authorising actions;
•	planning;
•	developing policies and procedures;
•	managing property insurance and claims;
•	reporting, reviewing and evaluating; and
•	managing risks.

""",
        "The function of managing land and working, storage, or living space within premises, and of acquiring, constructing, fitting-out, managing, maintaining, protecting and disposing of premises. Includes buildings and land allotments either owned, rented, or leased by the organisation. Also includes the removal of pollutants and waste. This function also covers properties owned by the Commonwealth or Commonwealth institutions which have national significance including natural, historic and indigenous significance and are listed in the Register of the National Estate, by the World Heritage Commission, classified by the National Trusts or on State heritage listings." ;
    skos:inScheme :conceptScheme: ;
    skos:prefLabel "Property Management",
        "Property Management  " .

:0022  a crs:Function, ra:Class,
        skos:Concept ;
    crs:isPerformedBy [ crs:hasAgent ca:0001 ],
        [ crs:hasAgent ca:0001 ] ;
    dct:source ras:1999-00000104,
        ras:2009-00450477 ;
    skos:definition """The function of having works, irrespective of format, issued for sale or distribution internally or to the public.  Includes drafting, manual or electronic production (design, layout, typesetting, printing etc), marketing and supply of publications by the organisation.  Includes external publications (such as technical papers, issues papers, articles for professional journals and reports) and leaflets which aim to promote the services and public image of the organisation, and internal publications (such as newsletters, circulars, procedure manuals etc), which are not produced for public relations reasons.  Also includes multi media publications, CD-ROM and online information services.

Function note:  Publication is one of the functions relating to the management of an agency’s information and knowledge resources.  The other is Information Management.  Publication relates to published works created by the agency and Information Management covers the collection, dissemination, use and control of information sources required by the agency to carry out its business activities.  The Publication function supports all administrative functions and core businesses in the production and distribution of publications to support the goals and objectives of the agency.

This function includes such publication related activities as:

•	negotiating, establishing, maintaining and reviewing agreements and joint ventures;
•	managing corporate style;
•	disposing of publications;
•	distributing publications;
•	drafting;
•	managing intellectual property;
•	marketing;
•	managing publication production (covers paper, electronic and films and video); and
•	stocktaking.

The performance of the function is supported by routine administrative tasks such as:

•	providing advice and responding to enquiries;
•	managing routine arrangements for the use of properties;
•	managing internal and external audits;
•	managing committees and meetings;
•	fulfilling compliance requirements;
•	delegating powers and authorising actions;
•	planning;
•	developing policies and procedures;
•	managing property insurance and claims;
•	research and reporting;
•	reviewing and evaluating; and
•	managing risks.

""",
        "The function of having works, irrespective of format, issued for sale or distribution internally or to the public.  Includes drafting, manual or electronic production (design, layout, typesetting, printing etc.), marketing and supply of publications by the organisation.  Includes external publications (such as technical papers, issues papers, articles for professional journals and reports) and leaflets which aim to promote the services and public image of the organisation; and internal publications (such as newsletters, circulars, procedure manuals etc.), which are not produced for public relations reasons. Also includes multi media publications, CD-ROM and on-line information services." ;
    skos:inScheme :conceptScheme: ;
    skos:prefLabel "Publication" .

:0023  a crs:Function, ra:Class,
        skos:Concept ;
    crs:isPerformedBy [ crs:hasAgent ca:0001 ],
        [ crs:hasAgent ca:0001 ] ;
    dct:source ras:1999-00000104,
        ras:2009-00450477 ;
    skos:definition "The function of encouraging staff to develop their skills and abilities (through activities, programs and events) to maximise their potential and increase their productivity.  Includes identifying and implementing all aspects of training needs and programs (internal and external) available to staff.","""The function of encouraging staff to develop their skills and abilities (through activities, programs and events) to maximize their potential and increase their productivity.  Includes identifying and implementing all aspects of training needs and programs (internal and external) available to staff.

Function notes:  Staff Development is one of the of AFDA Express suite of functions covering the management of an agency’s human resources.  Others are – Compensation, Establishment, Industrial Relations, Occupational Health & Safety (OH&S) and Personnel.  Staff Development relates to acquiring and updating skills and knowledge for both career and personal advancement.  It is closely related to Personnel which covers the management of staff from recruitment to separation from the APS and establishing employment conditions.  It is also linked to the Establishment function which is concerned with setting up the structure of the agency, including the identification of positions, classifications and duties.

The function includes such staff development related activities as:

•	developing addresses and presentations;
•	conference management; and
•	training.

The performance of the function is supported by routine administrative tasks such as:

•	providing advice;
•	allocating allowances;
•	making arrangements;
•	auditing;
•	managing committees and meetings;
•	fulfilling compliance requirements;
•	delegating powers and authorising actions;
•	evaluating, reviewing and reporting on the management of the function;
•	planning; and
•	developing policies and procedures.

""";
    skos:inScheme :conceptScheme: ;
    skos:prefLabel "Staff Development" .

:0024  a crs:Function, ra:Class,
        skos:Concept ;
    crs:isPerformedBy [ crs:hasAgent ca:0001 ],
        [ crs:hasAgent ca:0001 ] ;
    dct:source ras:1999-00000104,
        ras:2009-00450477 ;
    skos:definition """The function of applying broad systematic management planning for the organisation.  Includes the activities involved with the development, monitoring and reviewing of business plans, strategic plans, corporate plans, and other long-term organisational strategies.  Also includes the development of the corporate mission, objectives, continuous improvement processes, quality assurance and certification, and the formulation and amendment of legislation which provides the legislative basis for the organisation.

Function note:  Strategic Management aims at aligning policies, plans and strategic priorities across the agency to achieve goals and objectives.  Activities undertaken to provide overall direction for the agency usually involve senior agency officers and the executive team.  Strategic Management decisions impact on resource allocations through the Financial Management function, and the administrative structure of the organisation through the Establishment function.

This function includes such strategic management activities as:

•	providing advice;
•	negotiating, establishing, maintaining and reviewing agreements;
•	auditing;
•	fulfilling compliance requirements;
•	developing agency-wide strategies and processes to deliver customer services, to prevent fraud; and applying for grants;
•	identifying and investigating fraud allegations;
•	developing proposals for new and amended legislation;
•	managing meetings, internal management conferences and participation in external or inter-agency committees;
•	reporting, evaluating and reviewing strategic performance, programs and services;
•	developing national and unit level work plans aimed at achieving agency objectives;
•	developing plans to support specific ongoing cross agency administrative and operational activities (eg fraud control plan, business continuity plans, risk management plans);
•	developing and implementing government-wide and agency specific policies, procedures and instructions and commenting on government-wide strategic management policies;
•	developing formal and periodic reports;
•	undertaking research and responding to surveys of other agencies;
•	managing risks across the agency; and
•	implementing industry standards.
""",
        "The function of applying broad systematic management planning for the organisation. Includes the activities involved with the development, monitoring and reviewing of business plans, strategic plans, corporate plans, and other long-term organisational strategies. Also includes the development of the corporate mission, objectives, continuous improvement processes, quality assurance and certification, and the formulation and amendment of legislation which provides the legislative basis for the organisation." ;
    skos:inScheme :conceptScheme: ;
    skos:prefLabel "Strategic Management" .

:0025  a crs:Function, ra:Class,
        skos:Concept ;
    crs:isPerformedBy [ crs:hasAgent ca:0001 ],
        [ crs:hasAgent ca:0001 ] ;
    dct:source ras:1999-00000104,
        ras:2009-00450477 ;
    skos:definition """The function of developing and acquiring, testing and implementing applications, systems and databases to support the business needs of the organisation, to capture, store, retrieve, transfer, communicate and disseminate information through automated systems.  Includes the evaluation of software and hardware, licensing and disposal of systems.  Also includes communication network systems such as video conferencing, voice mail and electronic mail and the technical aspects of the internet, intranet and Web Sites.

Function note:  Technology  & Telecommunications is one of the AFDA Express functions that relates to managing agency assets.  The other asset management functions are – Equipment & Stores, Fleet Management, and Property Management.  The function relates to the management of an agency’s computer hardware and software and telecommunications equipment eg phones, faxes, mobiles etc.  The acquisition of technology and telecommunication products and services through leasing, tendering and contracting arrangements is covered by the Procurement function.  Training staff in how to use technology and telecommunication equipment is covered by Staff Development.

This function includes such technology and telecommunication development activities as:
•	analysing and developing business or technical models or prototype;
•	supporting work of certifying authorities;
•	evaluating ‘commercial-off-the-shelf’ products;
•	researching;
•	configuring corporate software;
•	developing and modifying specific agency applications;
•	post implementation reviews;
•	testing applications; and
•	rolling out and installing new systems, including migrating records between systems.

and such ongoing technical management activities as:
•	allocating equipment, services and facilities;
•	managing databases;
•	managing the implementation of security and privacy arrangements and investigating security breaches;
•	relocating and maintaining systems and equipment and carrying out routine inspections;
•	transferring or integrating systems following an administrative change;
•	supporting users (eg help desk operations; and
•	maintaining data dictionaries.

The function is supported by regular, routine administrative tasks such as:
•	providing advice;
•	establishing and managing agreements;
•	managing internal and external audits;
•	managing committees and meetings;
•	fulfilling compliance requirements;
•	developing customer service standards;
•	delegating powers and authorising actions;
•	evaluating services (eg contracting-out activities);
•	managing an agency’s technological and telecommunications intellectual property;
•	planning, developing policies and procedures;
•	project management and managing risks; and
•	reporting and reviewing.

""",
        "The function of developing or acquiring, testing and implementing applications, systems and databases to support the business needs of the organisation, to capture, store, retrieve, transfer, communicate and disseminate information through automated systems.  Includes the evaluation of software and hardware and the acquisition, tendering, leasing, licensing and disposal of systems. Also includes communication network systems such as video conferencing, voice mail and electronic mail and the technical aspects of the Internet, Intranet and Web Sites." ;
    skos:inScheme :conceptScheme: ;
    skos:prefLabel "Technology & Telecommunications",
        "Technology & Telecommunications " .

:0026  a crs:Function, ra:Class,
        skos:Concept ;
    crs:isPerformedBy [ crs:hasAgent ca:0005 ] ;
    dct:source ras:2002-04572652 ;
    skos:definition "The function of making and managing formal appointments authorised by the Governor-General and the Minister to support portfolio responsibilities, including those to the judiciary, magistracy, commissions, councils and appointments as marriage celebrants. Includes the processes involved in seeking advice on suitable candidates, advertising, making appointments, arranging formal authorisation and providing ongoing support to the appointee eg  approving leave, overseas travel etc and reviewing appointments. Also includes overall management of appointment activities. Excludes the appointment of staff under the Public Service Act 1999, and Departmental staff appointments to inter-governmental, inter-departmental and international committees, councils, boards etc." ;
    skos:inScheme :conceptScheme: ;
    skos:prefLabel "Appointments Management" .

:0027  a crs:Function, ra:Class,
        skos:Concept ;
    crs:isPerformedBy [ crs:hasAgent ca:0005 ] ;
    dct:source ras:2002-04572652 ;
    skos:definition "The function of identifying ways to prevent crime and violence in Australian communities.  Includes the development and provision of policy advice to Government, and Commonwealth departments and agencies; undertaking targeted research; liaising with community groups; supporting education programs; sharing information; coordinating and assisting States and Territories to enhance their crime prevention strategies; and contributing to relevant United Nations activities. Also includes negotiating, establishing, monitoring and reviewing projects and tendering for services and subsequent contract-management activities." ;
    skos:inScheme :conceptScheme: ;
    skos:prefLabel "Crime Prevention" .

:0028  a crs:Function, ra:Class,
        skos:Concept ;
    crs:isPerformedBy [ crs:hasAgent ca:0005 ] ;
    dct:source ras:2002-04572652 ;
    skos:definition "The function of providing advice to the Minister on specific issues of importance that relate to the unique functions of the organisation.  The advice is provided by formally established committees, councils and similar statutory and non-statutory bodies associated with the organisation. The membership of these advising organisations consists of a range of stakeholders which may include experts in the field, representatives of the profession or of professional bodies and community representatives. Secretariat services are provided by the agency. Excludes government and inter-government committees, councils etc where the agency provides secretariat services, or is a representative." ;
    skos:inScheme :conceptScheme: ;
    skos:prefLabel "Independent Advising" .

:0029  a crs:Function, ra:Class,
        skos:Concept ;
    crs:isPerformedBy [ crs:hasAgent ca:0005 ] ;
    dct:source ras:2002-04572652 ;
    skos:definition "The function of collecting and managing information (eg. newspaper cuttings, journal articles, published reports etc) to provide background details relevant to subject areas of departmental responsibility. Includes intelligence collations. Excludes activities involved in researching a subject to support a specific project." ;
    skos:inScheme :conceptScheme: ;
    skos:prefLabel "Information Collection" .

:0030  a crs:Function, ra:Class,
        skos:Concept ;
    crs:isPerformedBy [ crs:hasAgent ca:0005 ] ;
    dct:source ras:2002-04572652 ;
    skos:definition "The function of coordinating the formulation and implementation of Commonwealth law enforcement policies and activities relating to information technology, fraud, firearms and illicit drugs and the operation of law enforcement agencies within the Attorney-General’s portfolio.  Includes formal on-going liaison with other government agencies, and State, Territory and overseas law enforcement agencies.  Excludes providing legal advice and legal policy advice on legislative matters." ;
    skos:inScheme :conceptScheme: ;
    skos:prefLabel "Law Enforcement" .

:0031  a crs:Function, ra:Class,
        skos:Concept ;
    crs:isPerformedBy [ crs:hasAgent ca:0005 ] ;
    dct:source ras:2002-04572652 ;
    skos:definition "The function of managing on-going legal case work resulting from the implementation of legislative requirements or in support of international obligations.  Includes the activities of authorisation and carrying out legislative requirements, reporting on developments, making and implementing decisions and monitoring and reviewing outcomes. Also includes planning and controlling the processes involved in managing the cases." ;
    skos:inScheme :conceptScheme: ;
    skos:prefLabel "Legal Case Management" .

:0032  a crs:Function, ra:Class,
        skos:Concept ;
    crs:isPerformedBy [ crs:hasAgent ca:0005 ] ;
    dct:source ras:2002-04572652 ;
    skos:definition "The function of providing legal opinions to the Attorney-General, other Ministers, departments, statutory bodies and other parts of the agency covering areas of portfolio responsibility. Includes the provision of legal opinions on the interpretation of legislation and on the legal aspects of Cabinet submissions.  Also includes policy advice relating to the effectiveness of portfolio legislation and developing proposals to change the law. Excludes ‘ministerials’ received by the Attorney from members of the public and external bodies, responses prepared for ‘Possible Parliamentary Questions’ (PPQ’s), and replies prepared to Parliamentary Questions (PQ’s)." ;
    skos:inScheme :conceptScheme: ;
    skos:prefLabel "Legal Counsel" .

:0033  a crs:Function, ra:Class,
        skos:Concept ;
    crs:isPerformedBy [ crs:hasAgent ca:0005 ] ;
    dct:source ras:2002-04572652 ;
    skos:definition "The function of administering relationships focusing on supporting the law.  Includes liaison between the Department and State, Territory and overseas government agencies, non-government agencies (eg business, community and professional groups and overseas international agencies such as the United Nations), Courts and Tribunals and other Commonwealth departments, and assistance to the Attorney-General in the performance of the role of First Law Officer and the Minister for Justice.  Also includes liaison activities managed by the Department on behalf of Australia with other countries or organisations.  Includes activities associated with the Department’s membership of committees, councils, working groups etc, but excludes activities where the Department provides a secretariat role to independent organisations.  Also excludes relationships where legal counsel is provided." ;
    skos:inScheme :conceptScheme: ;
    skos:prefLabel "Legal Liaison" .

:0034  a crs:Function, ra:Class,
        skos:Concept ;
    crs:isPerformedBy [ crs:hasAgent ca:0005 ] ;
    dct:source ras:2002-04572652 ;
    skos:definition "The function of drafting and publishing regulations made under Commonwealth Acts, Letters Patent, determinations, proclamations, commissions, orders and other legislative instruments.  Includes editing and making arrangements for printing, gazettal and tabling of instruments and arranging and executing electronic publication and distribution.  Also includes preparation of Act consolidations, publishing legislative instruments and documents produced by agencies eg Explanatory Statements.  Excludes drafting of Commonwealth Acts." ;
    skos:inScheme :conceptScheme: ;
    skos:prefLabel "Legislative Drafting" .

:0035  a crs:Function, ra:Class,
        skos:Concept ;
    crs:isPerformedBy [ crs:hasAgent ca:0005 ] ;
    dct:source ras:2002-04572652 ;
    skos:definition "The function of developing policies and implementing a consistent national security framework and a nation-wide counter-terrorism capability.  Includes activities associated with interacting with high-level government, inter-government and Commonwealth/State committees (eg the Standing Committee on Commonwealth and State Co-operation for Protection Against Violence (SAC-PAV), and the National Security Committee of Cabinet) to consider issues relevant to national security, including defence and intelligence matters. Also covers liaison activities with departments, agencies and the business community on national security, counter-terrorism, telecommunications interception, the National Information Infrastructure, and monitoring the security environment." ;
    skos:inScheme :conceptScheme: ;
    skos:prefLabel "National Security" .

:0036  a crs:Function, ra:Class,
        skos:Concept ;
    crs:isPerformedBy [ crs:hasAgent ca:0005 ] ;
    dct:source ras:2002-04572652 ;
    skos:definition "The function of developing and promoting, through training and other awareness activities, protective security policy, advice and common standards, procedures and practices for Commonwealth departments and agencies covering areas of personnel, information, physical and computer security. Includes the coordination of protective security services and managing protective security arrangements for the protection of Australia’s high office holders, high-level visiting dignitaries and residences of Ministers and other Parliamentarians assessed to be at risk.  Also includes the management of the security vetting service to Commonwealth agencies." ;
    skos:inScheme :conceptScheme: ;
    skos:prefLabel "Protective Security" .

:0037  a crs:Function, ra:Class,
        skos:Concept ;
    crs:isPerformedBy [ crs:hasAgent ca:0046 ],
        [ crs:hasAgent ca:0046 ] ;
    dct:source ras:2005-00171070 ;
    skos:definition "The function of developing, implementing and reviewing standards, policies, systems and products relating to Defence protective security. Includes external vetting and clearances, threat assessments and over-seeing security within the Defence organisation and associated industry. Also includes advising on risk management, evaluating and monitoring security performance, establishing and maintenance of international security instruments, investigations and managing security of nonintelligence special compartmented information." ;
    skos:inScheme :conceptScheme: ;
    skos:prefLabel "Defence Security" .

:0038  a crs:Function, ra:Class,
        skos:Concept ;
    crs:isPerformedBy [ crs:hasAgent ca:0046 ] ;
    dct:source ras:2009-00120068 ;
    skos:definition """Information Security is the business of administering guidelines and standards for the protection of Australian Government Information Communication Technology (ICT) networks and information systems from unauthorised access and other potential threats.  It includes providing material, advice and other assistance to Commonwealth and State authorities on matters relating to the security and integrity of information that is processed, stored or communicated by electronic or similar means. It also includes conducting research into cryptology and monitoring compliance with government security policy and providing advice and assistance to Australian Government and organisations that form part of the National Information Infrastructure (NII).
Tasks that support the business of Information Security include:
* Policy, liaison, research, development, industry collaboration, communication security monitoring, testing and reporting;
* Provision of guidelines and interpretation supporting government regulations and policies relating to Information Security;
* Evaluation of Information Security products in accordance with internationally recognised standards;
Oversight of licensed commercial evaluation services;
* Certification, accreditation, reviews and audit of Information Security systems for compliance with Australian Government Information and Communication Technology Security Instructions (also known as ACSI);
* Investigations and control of Information Security incidents;
* Investigation and control of emissions from information technology networks and equipment;
* Threat assessment and vulnerability analysis of information technology networks and equipment;
* Advice and assistance to Commonwealth and State authorities concerning cryptography, communications technology and other Information Security products;
* Plan, coordinate and approve the production, distribution and management of hard copy and electronic traditional key and modern keying material, and other cryptographic products;
* Consulting Services to assist planning, implementation and operation of appropriate security policies, solutions and practices;
* Registration and endorsement of information communication technology assessors;
* Registration (licensing) of information communication technology facilities to perform evaluation services;
* Controlled access for agencies to security materials, equipment, information systems;
* Information Security training and awareness services; and
* Promotion of and dialogue about Information Security through presentations, committees and other representatives.

For records relating to accreditation, certification and advice for ICT breach investigations, threat assessments, computer network vulnerability of ICT systems classified SECRET and below within Department of Defence, use Defence Security Records Authority (job no 2005/00170070).

For all intelligence activities, use General Disposal Authority (GDA) 21.
""";
    skos:inScheme :conceptScheme: ;
    skos:prefLabel "Information Security" .

:0039  a crs:Function, ra:Class,
        skos:Concept ;
    crs:isPerformedBy [ crs:hasAgent ca:0046 ],
        [ crs:hasAgent ca:0046 ],
        [ crs:hasAgent ca:0046 ],
        [ crs:hasAgent ca:0046 ],
        [ crs:hasAgent ca:0046 ],
        [ crs:hasAgent ca:0046 ] ;
    dct:source ras:2002-04896824,
        ras:2002-05014351,
        ras:2006-00323929,
        ras:2009-00741349,
        ras:2012-00443724,
        ras:2012-00443842 ;
    skos:definition "The function of managing all service members, accredited representatives, reservists and national service members from recruitment to final discharge. Also includes managing deployed civilians (in support of operations) for disciplinary conduct and honours and awards. Activities include career management, postings, promotions, reclassification, recruiting, appointment and enlistment, discharge and transfers, honours and awards, disciplinary conduct, pay, entitlements and allowances, travel, superannuation and retirement benefits, grievances, casualties, non compensable occupational rehabilitation and leave.",
        "The function of managing all service members, accredited representatives, reservists and national service members from recruitment to final discharge. Also includes managing deployed civilians (in support of operations) for disciplinary misconduct and honours and awards. Activities include career management, postings, promotions, reclassification, recruiting, appointment and enlistment, discharge and transfers, honours and awards, disciplinary misconduct, pay, entitlements and allowances, travel, superannuation and retirement benefits, grievances, casualties, non-compensable occupational rehabilitation and leave." ;
    skos:inScheme :conceptScheme: ;
    skos:prefLabel " Military Personnel",
        "Military Personnel" .

:0040  a crs:Function, ra:Class,
        skos:Concept ;
    crs:isPerformedBy [ crs:hasAgent ca:0046 ] ;
    dct:source ras:2001-01594969 ;
    skos:definition """The function of managing all service personnel, accredited representatives, service cadets, reserves, and national service personnel. Includes career management, recruiting, appointment and enlistment, discharge and transfers, honours and awards, discipline and misconduct, pay, allowances and superannuation, grievances, casualties, occupational rehabilitation, leave, postings.
""";
    skos:inScheme :conceptScheme: ;
    skos:prefLabel "Military Personnel [S26]" .

:0041  a crs:Function, ra:Class,
        skos:Concept ;
    crs:isPerformedBy [ crs:hasAgent ca:0046 ] ;
    dct:source ras:2001-00000525 ;
    skos:definition "The creating, building and modifying of various pieces of equipment and infrastructure to support experimental and observational requirements." ;
    skos:inScheme :conceptScheme: ;
    skos:prefLabel "Project Support" .

:0042  a crs:Function, ra:Class,
        skos:Concept ;
    crs:isPerformedBy [ crs:hasAgent ca:0046 ] ;
    dct:source ras:2001-00000525 ;
    skos:definition "The carrying out of scientific research and development to support the capabilities of Australian and other countries'  Defence Forces or in accordance with commercial agreement with industry or educational bodies." ;
    skos:inScheme :conceptScheme: ;
    skos:prefLabel "Research And Development" .

:0043  a crs:Function, ra:Class,
        skos:Concept ;
    crs:isPerformedBy [ crs:hasAgent ca:0225 ],
        [ crs:hasAgent ca:0225 ] ;
    dct:source ras:2004-00336830,
        ras:2007-00404051 ;
    skos:definition """The function of determining eligibility for, and entitlement to, income support for veterans, war widows, war widowers, and dependants of veterans; of determining eligibility for compensation to veterans in recognition of the effects of war service; and of providing the determined entitlements. Includes processing applications for pensions, allowances, and other entitlements such as income support, disability compensation, and education schemes for veterans' children.

Also includes activities that assist and support persons making claims for eligibility and entitlements. """;
    skos:inScheme :conceptScheme: ;
    skos:prefLabel "Benefits" .

:0044  a crs:Function, ra:Class,
        skos:Concept ;
    crs:isPerformedBy [ crs:hasAgent ca:0225 ] ;
    dct:source ras:2007-00032716 ;
    skos:definition "The function of managing the administrative activities of the Repatriation Commission. Includes notification of appointments and terminations of Commissioners, remuneration, Commission meetings, and arrangement for Commissioners to travel on Commission business." ;
    skos:inScheme :conceptScheme: ;
    skos:prefLabel "Governance" .

:0045  a crs:Function, ra:Class,
        skos:Concept ;
    crs:isPerformedBy [ crs:hasAgent ca:0225 ] ;
    dct:source ras:2007-00032716 ;
    skos:definition "The function of providing the eligible veteran community with access to health and support services that promote and maintain self-sufficiency, well-being and quality of life. Includes acquisition of services through arrangements with health care providers and the contract management of those arrangements. Also includes research, grant funding for the provision of activities to help the veteran community remain healthy and independent, providing vocational rehabilitation programs to assist veterans to continue in, or find, employment, promoting health lifestyle awareness, providing education services to assist service providers meet the needs of the veteran community and the management of transport arrangements for the veteran community to access health and hospital services." ;
    skos:inScheme :conceptScheme: ;
    skos:prefLabel "Health Care And Support Services" .

:0046  a crs:Function, ra:Class,
        skos:Concept ;
    crs:isPerformedBy [ crs:hasAgent ca:0225 ] ;
    dct:source ras:2007-00032716 ;
    skos:definition "The function of managing a hospital. Includes documenting treatment of patients who are not veterans or dependants of veterans, recording summary information regarding patients, diseases, operations and deaths, agreements and documents concerning the transfer of hospital administration to or from other agencies or organisations, research, and accreditation of hospitals according to recognised standards." ;
    skos:inScheme :conceptScheme: ;
    skos:prefLabel "Hospital Administration" .

:0047  a crs:Function, ra:Class,
        skos:Concept ;
    crs:isPerformedBy [ crs:hasAgent ca:0225 ] ;
    dct:source ras:2007-00032716 ;
    skos:definition "The function of providing artificial limbs and appliances to eligible ex-service personnel and certain categories of civilian amputees. Includes conducting research into the manufacturing and design of artificial limbs and appliances." ;
    skos:inScheme :conceptScheme: ;
    skos:prefLabel "Prosthetics Services" .

:0048  a crs:Function, ra:Class,
        skos:Concept ;
    crs:isPerformedBy [ crs:hasAgent ca:0225 ] ;
    dct:source ras:2007-00404051 ;
    skos:definition "Operational and administrative activities for the function of Veterans' Affairs (Boer War)" ;
    skos:inScheme :conceptScheme: ;
    skos:prefLabel "Veterans' Affairs (Boer War)" .

:0049  a crs:Function, ra:Class,
        skos:Concept ;
    crs:isPerformedBy [ crs:hasAgent ca:0280 ] ;
    dct:source ras:2009-00439481 ;
    skos:definition """The core business of developing and maintaining the organisation's collection of judicial archival material.  Includes:
• the creation, development and maintenance of the agency archive;
• developing and reviewing policies governing the archive including issues of funding, access, security and organisation;
• ensuring materials important to the history of the agencies and their antecedent bodies are preserved, restored and catalogued so they do not degrade over time and may be accessed for study and public information purposes;
• promoting an interest in the history of agencies and their antecedent bodies among individuals internally and externally;
• providing access to and use of the collection;
• establishment and meetings of the archives committee;
• managing donations to the collection;
• holding exhibitions, including travelling exhibitions;
• arranging and recording oral histories related to the collection.""";
    skos:inScheme :conceptScheme: ;
    skos:prefLabel "Archives Collection" .

:0050  a crs:Function, ra:Class,
        skos:Concept ;
    crs:isPerformedBy [ crs:hasAgent ca:0280 ] ;
    dct:source ras:2009-00439481 ;
    skos:definition """The core business of managing the agency's relationship with external stakeholders in association with broad industrial and employment matters. It includes:
• representation on and participation in industrial bodies and groups, such as the International Labour Organisation;
• participation in functions and events;
• presentations at national and international conferences;
• advice that is not related to a specific industrial case or registered organisations;
• meetings and other liaison with stakeholders, including industry consultative committees and heads of tribunal meetings;
• visits to and from external stakeholders, including international delegations.""";
    skos:inScheme :conceptScheme: ;
    skos:prefLabel "External Relations" .

:0051  a crs:Function, ra:Class,
        skos:Concept ;
    crs:isPerformedBy [ crs:hasAgent ca:0280 ] ;
    dct:source ras:2009-00439481 ;
    skos:definition """The core business of dealing with national employment issues.  It includes:
• assisting employers and employees to resolve industrial disputes
• handling termination of employment claims;
• making, rationalising and simplifying awards;
• handling applications for industrial action;
• liaising with and advising external and internal stakeholders in relation to specific cases; and
• responding to enquiries in relation to industrial matters.""";
    skos:inScheme :conceptScheme: ;
    skos:prefLabel "Industrial Relations Cases" .

:0052  a crs:Function, ra:Class,
        skos:Concept ;
    crs:isPerformedBy [ crs:hasAgent ca:0280 ] ;
    dct:source ras:2009-00439008 ;
    skos:definition """The core business of managing the registration and accountability of eligible unions and employer associations.  Includes:
• applications for registration;
• elections;
• annual returns and financial statements;
• right of entry permits;
• rules of the registered organisation, including alterations;
• details of loans, grants and donations given by the registered organisation;
• transitional registration;
• providing advice to and liaising with registered organisations in association with their registration.""";
    skos:inScheme :conceptScheme: ;
    skos:prefLabel "Registered Organisations" .

:0053  a crs:Function, ra:Class,
        skos:Concept ;
    crs:isPerformedBy [ crs:hasAgent ca:0280 ] ;
    dct:source ras:2009-00439481 ;
    skos:definition """The core business of managing statutory positions within the organisation and associated operational matters. Statutory appointments include those to judicial body positions. Includes matters concerning:
• appointments and remuneration, together with the appointment history of each individual member;
• internal policies and procedures;
• travel arrangements;
• notebooks and diaries created by appointees.""";
    skos:inScheme :conceptScheme: ;
    skos:prefLabel "Statutory Appointments" .

:0054  a crs:Function, ra:Class,
        skos:Concept ;
    crs:isPerformedBy [ crs:hasAgent ca:0280 ] ;
    dct:source ras:2009-00439008 ;
    skos:definition """The core business of managing statutory positions within the organisation. Statutory appointments include those to the industrial registrar and deputy registrar positions. Includes matters concerning:
•	appointments and remuneration, together with the appointment history of each individual member;
•	internal policies and procedures;
•	travel arrangements.""";
    skos:inScheme :conceptScheme: ;
    skos:prefLabel "Statutory Appointments (Air)" .

:0055  a crs:Function, ra:Class,
        skos:Concept ;
    crs:isPerformedBy [ crs:hasAgent ca:0616 ] ;
    dct:source ras:2005-00243341 ;
    skos:definition """The function of acquiring, documenting, controlling, conserving and preserving, researching, and making accessible the organisation’s national collection. Includes art, photographs, sound, film, relics,
objects, maps, private records and published material.""";
    skos:inScheme :conceptScheme: ;
    skos:prefLabel "Collection" .

:0056  a crs:Function, ra:Class,
        skos:Concept ;
    crs:isPerformedBy [ crs:hasAgent ca:0616 ] ;
    dct:source ras:2005-00243341 ;
    skos:definition "The function of commemorating the sacrifice of Australians who have died in war through the management of commemorative ceremonies and events. Includes providing advice to other organisations conducting commemorative ceremonies and the management of commemorative objects of significance, such as the Roll of Honour and Commemorative Roll." ;
    skos:inScheme :conceptScheme: ;
    skos:prefLabel "Commemoration" .

:0057  a crs:Function, ra:Class,
        skos:Concept ;
    crs:isPerformedBy [ crs:hasAgent ca:0616 ] ;
    dct:source ras:2005-00243341 ;
    skos:definition """The function of providing products and services on a commercial basis, such as retail and on-line sales, wholesale trading, tours, holiday programs, catering and venue hire. Includes acquiring,
producing, distributing and marketing products and services.""";
    skos:inScheme :conceptScheme: ;
    skos:prefLabel "Commercial Services" .

:0058  a crs:Function, ra:Class,
        skos:Concept ;
    crs:isPerformedBy [ crs:hasAgent ca:0616 ] ;
    dct:source ras:2005-00243341 ;
    skos:definition """The function of managing the activities of the agency’s council. Includes the provision of advice and reporting on council issues and council business, notification of appointments and terminations of
council members, remuneration, council meetings, committees established by the council, and arrangement for council members to travel on council business.""";
    skos:inScheme :conceptScheme: ;
    skos:prefLabel "Council Management" .

:0059  a crs:Function, ra:Class,
        skos:Concept ;
    crs:isPerformedBy [ crs:hasAgent ca:0616 ] ;
    dct:source ras:2005-00243341 ;
    skos:definition """The function of developing, coordinating and managing the agency’s galleries and exhibitions, including travelling exhibitions. Includes the development of the exhibition content and exhibition
design, fit-out, installation and demounting, and marketing and seeking sponsorships for exhibitions.""";
    skos:inScheme :conceptScheme: ;
    skos:prefLabel "Exhibitions" .

:0060  a crs:Function, ra:Class,
        skos:Concept ;
    crs:isPerformedBy [ crs:hasAgent ca:0616 ] ;
    dct:source ras:2005-00243341 ;
    skos:definition "The function of conducting historical research to enhance the knowledge and understanding of Australia’s military history. Includes endorsing historical information used in the organisation, the commissioning of official war histories, writing and editing of historical manuscripts and publications, the presentation of military history lectures and conferences, military history research and the development of battlefield tours." ;
    skos:inScheme :conceptScheme: ;
    skos:prefLabel "Historical Research" .

:0061  a crs:Function, ra:Class,
        skos:Concept ;
    crs:isPerformedBy [ crs:hasAgent ca:0616 ] ;
    dct:source ras:2005-00243341 ;
    skos:definition """The function of developing, providing and managing education and public programs to enhance the knowledge and understanding of the Australian experience of war. Includes the provision of a range of
services to visitors and the management of visits and tours to the Memorial.""";
    skos:inScheme :conceptScheme: ;
    skos:prefLabel "Interpretation" .

:0062  a crs:Function, ra:Class,
        skos:Concept ;
    crs:isPerformedBy [ crs:hasAgent ca:0641 ] ;
    dct:source ras:2002-04926193 ;
    skos:definition "The function of assessing applications referred from the Australian Tax Office for recognition as an Approved Research Institute under the relevant taxation legislation (including Section 73A of the Income Tax Assessment Act 1936)." ;
    skos:inScheme :conceptScheme: ;
    skos:prefLabel "Approved Research Institutes Assessment" .

:0063  a crs:Function, ra:Class,
        skos:Concept ;
    crs:isPerformedBy [ crs:hasAgent ca:0641 ] ;
    dct:source ras:2002-04926193 ;
    skos:definition "The function of increasing awareness the commercial benefits to industry from investment in research and development and formalising the involvement of the organisation in commercial transactions. Includes contracts and agreements for all research and technology transfer arrangements and confidentiality agreements other than with personnel." ;
    skos:inScheme :conceptScheme: ;
    skos:prefLabel "Business Development" .

:0064  a crs:Function, ra:Class,
        skos:Concept ;
    crs:isPerformedBy [ crs:hasAgent ca:0641 ] ;
    dct:source ras:2002-04926193 ;
    skos:definition "The function of establishing or maintaining international contacts and monitoring developments in the international scientific environment. Includes placement of overseas trainees on behalf of overseas organisations. Excludes international liaison undertaken in relation to research management or scentific research functions." ;
    skos:inScheme :conceptScheme: ;
    skos:prefLabel "International Scientific Liaison" .

:0065  a crs:Function, ra:Class,
        skos:Concept ;
    crs:isPerformedBy [ crs:hasAgent ca:0641 ] ;
    dct:source ras:2002-04926193 ;
    skos:definition "The function of managing the use of and access to National Facilities, including use of the Facilities by external parties." ;
    skos:inScheme :conceptScheme: ;
    skos:prefLabel "National Facilities Management" .

:0066  a crs:Function, ra:Class,
        skos:Concept ;
    crs:isPerformedBy [ crs:hasAgent ca:0641 ] ;
    dct:source ras:2002-04926193 ;
    skos:definition "The function of managing science buildings, which have been purpose built and have unique or specialised design features." ;
    skos:inScheme :conceptScheme: ;
    skos:prefLabel "Property Management (Special Buildings)" .

:0067  a crs:Function, ra:Class,
        skos:Concept ;
    crs:isPerformedBy [ crs:hasAgent ca:0641 ] ;
    dct:source ras:2002-04926193 ;
    skos:definition "The function of managing research and development activities at the operational level.  Includes project management and professional, academic and technical conferences and committees." ;
    skos:inScheme :conceptScheme: ;
    skos:prefLabel "Research Management" .

:0068  a crs:Function, ra:Class,
        skos:Concept ;
    crs:isPerformedBy [ crs:hasAgent ca:0641 ] ;
    dct:source ras:2002-04926193 ;
    skos:definition "The function of providing non-administrative support for scientific research.  Includes technical services, management of collections of data or specimens for on-going research reference purposes, and acquisition of major and unique items of scientific equipment constructed to agency specifications, such as purpose built research vessels." ;
    skos:inScheme :conceptScheme: ;
    skos:prefLabel "Research Support" .

:0069  a crs:Function, ra:Class,
        skos:Concept ;
    crs:isPerformedBy [ crs:hasAgent ca:0641 ] ;
    dct:source ras:2002-04926193 ;
    skos:definition "The function of promoting science and careers in science by alerting school students, their families and science teachers to the contribution of scientific research to the community, and by encouraging students to participate in scientific activities." ;
    skos:inScheme :conceptScheme: ;
    skos:prefLabel "Science Education" .

:0070  a crs:Function, ra:Class,
        skos:Concept ;
    crs:isPerformedBy [ crs:hasAgent ca:0641 ] ;
    dct:source ras:2002-04926193 ;
    skos:definition "The function of managing the employment of all employees in the organisation employed under the Science and Industry Act 1949 as amended and previous legislation and volunteer workers. Includes review of actions, overtime salaries, superannuation and work" ;
    skos:inScheme :conceptScheme: ;
    skos:prefLabel "Science Personnel" .

:0071  a crs:Function, ra:Class,
        skos:Concept ;
    crs:isPerformedBy [ crs:hasAgent ca:0641 ] ;
    dct:source ras:2002-04926193 ;
    skos:definition "The function of undertaking original scientific investigations, experimentation and theoretical, innovative development or systematic work aimed at the creation of new knowledge, and application of this knowledge to new or improved practices, products or processes. Includes liaison between scientists, meetings to discuss technical issues and unpublished technical papers." ;
    skos:inScheme :conceptScheme: ;
    skos:prefLabel "Scientific Research" .

:0072  a crs:Function, ra:Class,
        skos:Concept ;
    crs:isPerformedBy [ crs:hasAgent ca:0641 ] ;
    dct:source ras:2002-04926193 ;
    skos:definition """The function of providing external clients with technical services such as calibration, testing, analysis, assessment, and consulting services where existing knowledge is used to provide professional and technical advice. No original research is required and no
intellectual property developed. Includes technical training courses and workshops offered externally.""";
    skos:inScheme :conceptScheme: ;
    skos:prefLabel "Technical And Consulting Services" .

:0073  a crs:Function, ra:Class,
        skos:Concept ;
    crs:isPerformedBy [ crs:hasAgent ca:0641 ] ;
    dct:source ras:2002-04926193 ;
    skos:definition "The function of managing trust funds established by legislation (including the Science and Industry Endowment Act 1920) or by other means, within the terms of trusts established to support research and administered by the Agency. Includes the awarding of fellowships, studentships and grants in aid of research." ;
    skos:inScheme :conceptScheme: ;
    skos:prefLabel "Trust Funds Management" .

:0074  a crs:Function, ra:Class,
        skos:Concept ;
    crs:isPerformedBy [ crs:hasAgent ca:0863 ] ;
    dct:source ras:2006-00446555 ;
    skos:definition "The function of seeking new knowledge on the part of the University’s staff and students and the application of that knowledge for practical and commercial uses.  Includes conducting pure basic research (the seeking of new knowledge for its own sake), strategic basic research (the seeking of new knowledge with strategic outcomes in mind), applied research, experimental development and clinical trials, as well as the commercialisation of the results of that research. Also includes the processes involved in applying for and receiving of research grants and complying with research standards and regulatory requirements." ;
    skos:inScheme :conceptScheme: ;
    skos:prefLabel "Research & Development" .

:0075  a crs:Function, ra:Class,
        skos:Concept ;
    crs:isPerformedBy [ crs:hasAgent ca:0863 ] ;
    dct:source ras:2005-00347027 ;
    skos:definition "The function of recruiting, selecting and admitting students to academic programs, providing academic advice, scholarships and reviewing and monitoring academic progress. Includes administration of academic assessment and conferring of relevant awards on those students who graduate from a program of study." ;
    skos:inScheme :conceptScheme: ;
    skos:prefLabel "Student Progress" .

:0076  a crs:Function, ra:Class,
        skos:Concept ;
    crs:isPerformedBy [ crs:hasAgent ca:0863 ] ;
    dct:source ras:2005-00347027 ;
    skos:definition "The function of fostering academic and pesonal development of students including through residential life, extracurricular activities, social, health and career counselling. Also includes student counselling, financial assistance and the provision of services to enhance academic learning. " ;
    skos:inScheme :conceptScheme: ;
    skos:prefLabel "Student Services" .

:0077  a crs:Function, ra:Class,
        skos:Concept ;
    crs:isPerformedBy [ crs:hasAgent ca:0863 ] ;
    dct:source ras:2006-00446555 ;
    skos:definition "The function of formulating and delivering the teaching curriculum and undertaking the learning process. Includes course delivery, curriculum development, planning and review and exhibiting of student work." ;
    skos:inScheme :conceptScheme: ;
    skos:prefLabel "Teaching & Learning" .

:0078  a crs:Function, ra:Class,
        skos:Concept ;
    crs:isPerformedBy [ crs:hasAgent ca:1401 ] ;
    dct:source ras:2002-04959153 ;
    skos:definition """The function of endorsing events, programs or products associated with the Bicentenary. Endorsement was an official “seal of approval” that entitled the endorsee to non-commercial use of the logo, symbols and prescribed expressions associated with the Bicentenary and inclusion in the 1988 Calendar of Events and the Official 1988 Bicentennial Program. Those endorsed for commercial use (licensees) were required to pay a royalty to the Authority. Includes evaluation of applications, opinions and recommendations received from relevant stakeholders regarding endorsement/licensing, the decision to endorse/license (or otherwise), contracts and monitoring,
and samples of endorsed/licensed products. Also includes policy, procedures and reports regarding endorsement and licensing.""";
    skos:inScheme :conceptScheme: ;
    skos:prefLabel "Endorsement" .

:0079  a crs:Function, ra:Class,
        skos:Concept ;
    crs:isPerformedBy [ crs:hasAgent ca:1401 ] ;
    dct:source ras:2002-04959153 ;
    skos:definition """The function of organising or coordinating Bicentennial events, awards and ceremonies.  Includes planning, booking venues, organising catering and entertainment, liaising with relevant individuals, groups, government and industry about events, registration and other actions necessary to ensure smooth event management. Also includes planning for events to be included
in the National Program and other subsidiary programs such as the Women’s Program and Arts Program. The recognition of projects that do not involve endorsement or funding and donations to support event management come under this function. Photographs, slides and audio-visual materials etc, which document the implementation of Bicentennial events and awards in recognition of assistance given, form part of this function.""";
    skos:inScheme :conceptScheme: ;
    skos:prefLabel "Event Management" .

:0080  a crs:Function, ra:Class,
        skos:Concept ;
    crs:isPerformedBy [ crs:hasAgent ca:1401 ] ;
    dct:source ras:2002-04959153 ;
    skos:definition "The function of receiving or acquiring publications, irrespective of format, from external sources where the publication had been funded or endorsed or otherwise linked to the Authority." ;
    skos:inScheme :conceptScheme: ;
    skos:prefLabel "External Publication" .

:0081  a crs:Function, ra:Class,
        skos:Concept ;
    crs:isPerformedBy [ crs:hasAgent ca:1401 ] ;
    dct:source ras:2002-04959153 ;
    skos:definition """The function of allocating funding to organisations, individuals, groups, governments, councils, or Bicentennial Community Committees to assist in the development of events, projects or products to commemorate Australia’s Bicentenary. Includes evaluation of applications, opinions and recommendations received from relevant stakeholders regarding funding, Board decisions to fund
or not fund applications, contracts and commissions, monitoring and reviews of decisions, and samples of funded products. Also includes internal plans and policies concerning funding.""";
    skos:inScheme :conceptScheme: ;
    skos:prefLabel "Funding" .

:0082  a crs:Function, ra:Class,
        skos:Concept ;
    crs:isPerformedBy [ crs:hasAgent ca:1401 ] ;
    dct:source ras:2002-05022293 ;
    skos:definition "The function of coordinating a whole of government approach to the administration of government policies, official ceremonies and visits, national symbols, honours and awards, and government communications. Includes providing policy advice, arranging and coordinating social functions, and drawing up, issuing and assessing tenders." ;
    skos:inScheme :conceptScheme: ;
    skos:prefLabel "Government Coordination" .

:0083  a crs:Function, ra:Class,
        skos:Concept ;
    crs:isPerformedBy [ crs:hasAgent ca:1401 ] ;
    dct:source ras:2002-05022293 ;
    skos:definition "The function of managing Official Establishments and advising the Prime Minister of the day on the maintenance and restoration of the official residences consistent with their status as part of the National Estate, drawing upon guidance from the Official Establishments Trust. Covers management oversight of The Lodge and Kirribilli House, including staffing, administration, repairs, maintenance and restoration requirements of the residences." ;
    skos:inScheme :conceptScheme: ;
    skos:prefLabel "Official Establishments Management" .

:0084  a crs:Function, ra:Class,
        skos:Concept ;
    crs:isPerformedBy [ crs:hasAgent ca:1401 ] ;
    dct:source ras:2002-05022298 ;
    skos:definition "The function associated with providing advice and making recommendations to government on the operation, conservation, and long-term development of the four official residences. Also includes consultation with the occupants of the residences; officials of the Office of the Official Secretary to the Governor-General; and the Department of the Prime Minister and Cabinet." ;
    skos:inScheme :conceptScheme: ;
    skos:prefLabel "Official Establishments Trust" .

:0085  a crs:Function, ra:Class,
        skos:Concept ;
    crs:isPerformedBy [ crs:hasAgent ca:1401 ] ;
    dct:source ras:2002-04959153 ;
    skos:definition """The function of promoting public awareness of, and involvement in, Australia’s Bicentenary. Includes the selection, development and merchandising of Bicentennial products and themes, sponsorship, marketing and advertising, public information campaigns and media liaison. Also includes promotional relationships with stakeholders participating in the Bicentenary, involvement in non-Bicentennial speeches, functions and exhibitions for the purposes of promoting the
Bicentenary, customer consultation and feedback. Photographs, slides and audio-visual materials that promote the services of the Authority or Bicentennial events from part of this function. This function includes the promotion of endorsed and funded events that were not organised by the Authority.""";
    skos:inScheme :conceptScheme: ;
    skos:prefLabel "Promotion" .

:0086  a crs:Function, ra:Class,
        skos:Concept ;
    crs:isPerformedBy [ crs:hasAgent ca:1401 ] ;
    dct:source ras:2010-00039583 ;
    skos:definition "The core business of administering (the execution of) Royal Commissions established by Letters Patent signed by the Governor-General. Includes carrying out investigations and research, receiving submissions and holding hearings. Also includes activities associated with the presentation of a final report to the Governor-General and Parliament. " ;
    skos:inScheme :conceptScheme: ;
    skos:prefLabel "Royal Commission Administration" .

:0087  a crs:Function, ra:Class,
        skos:Concept ;
    crs:isPerformedBy [ crs:hasAgent ca:1776 ] ;
    dct:source ras:2001-00000540 ;
    skos:definition """The function of interpreting statistical data collected by survey and other means.

Includes econometric modelling and forecasting, seasonal adjustment and other time series analysis and the construction and interpretation of economic indicators.""";
    skos:inScheme :conceptScheme: ;
    skos:prefLabel "Statistical Analysis" .

:0088  a crs:Function, ra:Class,
        skos:Concept ;
    crs:isPerformedBy [ crs:hasAgent ca:1776 ],
        [ crs:hasAgent ca:1776 ] ;
    dct:source ras:2001-00000540,
        ras:2007-00105946 ;
    skos:definition "The function of acquiring statistical information in accordance with ABS legislation, on a particular topic or topics. Includes the collection of information directly by the census process, by sample, indirectly from an administrative by-product or from another collection. Includes collection by telephone interview and by mail and electronic means." ;
    skos:inScheme :conceptScheme: ;
    skos:prefLabel "Statistical Collections" .

:0089  a crs:Function, ra:Class,
        skos:Concept ;
    crs:isPerformedBy [ crs:hasAgent ca:1776 ] ;
    dct:source ras:2001-00000540 ;
    skos:definition """The function of contributing to the advancement of statistical operations and services at national and international levels.

Includes seminars and training sessions for providers and involvement in and representation on international statistical forums and committees, including the development of international Statistical Classifications.

Also includes the development of best practice in statistical operations, advice, support, training and technical assistance. """;
    skos:inScheme :conceptScheme: ;
    skos:prefLabel "Statistical Development And Support" .

:0090  a crs:Function, ra:Class,
        skos:Concept ;
    crs:isPerformedBy [ crs:hasAgent ca:1776 ] ;
    dct:source ras:2001-00000540 ;
    skos:definition """The function of providing customised statistical information to government, business and the broader community that is not otherwise published or available.

Includes quick reference information services and dissemination of material from consultancy services provided on a fee-for-service basis.

Also includes data provided under contract through Secondary Providers.""";
    skos:inScheme :conceptScheme: ;
    skos:prefLabel "Statistical Dissemination" .

:0091  a crs:Function, ra:Class,
        skos:Concept ;
    crs:isPerformedBy [ crs:hasAgent ca:1776 ] ;
    dct:source ras:2001-00000540 ;
    skos:definition "The function of preparing statistical data for dissemination. Includes capture and aggregation, cleaning  and confidentialising. Also includes compilation, mapping and classification." ;
    skos:inScheme :conceptScheme: ;
    skos:prefLabel "Statistical Processes" .

:0092  a crs:Function, ra:Class,
        skos:Concept ;
    crs:isPerformedBy [ crs:hasAgent ca:1873 ] ;
    dct:source ras:2005-00049707 ;
    skos:definition "Not entered" ;
    skos:inScheme :conceptScheme: ;
    skos:prefLabel "Operational Activities" .

:0093  a crs:Function, ra:Class,
        skos:Concept ;
    crs:isPerformedBy [ crs:hasAgent ca:2069 ] ;
    dct:source ras:2007-00213478 ;
    skos:definition "The function of managing and promoting the agency's holdings of national philatelic heritage and postal history artefacts such as posting boxes, postmarkers, furniture, equipment, clothing, and vehicles. Includes the acquisition, control, promotion, conservation, and making provision for the access and use of collection items. Also includes the holding of stamp stocks." ;
    skos:inScheme :conceptScheme: ;
    skos:prefLabel "Collection Management" .

:0094  a crs:Function, ra:Class,
        skos:Concept ;
    crs:isPerformedBy [ crs:hasAgent ca:2069 ] ;
    dct:source ras:2007-00213478 ;
    skos:definition """The function of managing and providing the agency's retail and other commercial services. Includes establishing licence, franchise, and agency agreements, training staff of non-corporate owned retail
outlets. Also includes the provision of commercial services such as product delivery, outsource logistics (including warehousing), financial processing including bill payments, banking, and money
order processing, as well as courier services and mailroom solutions.""";
    skos:inScheme :conceptScheme: ;
    skos:prefLabel "Commercial Operations" .

:0095  a crs:Function, ra:Class,
        skos:Concept ;
    crs:isPerformedBy [ crs:hasAgent ca:2069 ] ;
    dct:source ras:2007-00213478 ;
    skos:definition """The function of directing and controlling the agency. Includes high level advice, approvals, and policy issued by the Board and board management issues such as appointments, remuneration, meetings,
and performance management.""";
    skos:inScheme :conceptScheme: ;
    skos:prefLabel "Corporate Governance" .

:0096  a crs:Function, ra:Class,
        skos:Concept ;
    crs:isPerformedBy [ crs:hasAgent ca:2069 ] ;
    dct:source ras:2007-00213478 ;
    skos:definition "The function of establishing and maintaining relationships with the agency's customers or potential customers. Includes compliance with customer service standards, the development and management of customer service agreements, and handling complaints and customer enquiries." ;
    skos:inScheme :conceptScheme: ;
    skos:prefLabel "Customer Relations" .

:0097  a crs:Function, ra:Class,
        skos:Concept ;
    crs:isPerformedBy [ crs:hasAgent ca:2069 ] ;
    dct:source ras:2007-00213478 ;
    skos:definition "The function of managing the agency's relationship with industry and the community. It includes media liaison, official representation at functions, participation in community activities and relationships with professional bodies and industry groups, including international organisations such as the Universal Postal Union." ;
    skos:inScheme :conceptScheme: ;
    skos:prefLabel "External Relations" .

:0098  a crs:Function, ra:Class,
        skos:Concept ;
    crs:isPerformedBy [ crs:hasAgent ca:2069 ] ;
    dct:source ras:2007-00213478 ;
    skos:definition "The function of collecting, processing, and delivering letters, parcels, and international mail. It includes handling registered post, express post, telegraphic communication and defence force mail, determining and fixing postage charges and rates, processing insured claims for damaged or lost mail, and procuring mail delivery services. Also includes the installation and maintenance of post boxes and the allocation of post codes." ;
    skos:inScheme :conceptScheme: ;
    skos:prefLabel "Mail Operations" .

:0099  a crs:Function, ra:Class,
        skos:Concept ;
    crs:isPerformedBy [ crs:hasAgent ca:2069 ] ;
    dct:source ras:2007-00213478 ;
    skos:definition """The function of acquiring, manufacturing, supplying, maintaining, and disposing of equipment and stores. Equipment includes mail handling/sorting equipment, implements, tools, machines, plant,
furniture and furnishings.""";
    skos:inScheme :conceptScheme: ;
    skos:prefLabel "Post Equipment And Stores" .

:0100  a crs:Function, ra:Class,
        skos:Concept ;
    crs:isPerformedBy [ crs:hasAgent ca:2069 ] ;
    dct:source ras:2007-00213478 ;
    skos:definition "The function of acquiring (either by purchase, leasing, or chartering), designing, managing, maintaining, repairing, and disposing of vehicles. Vehicles are any means of conveyance owned or used by the agency, including special purpose vehicles, to transport people, post, or other items." ;
    skos:inScheme :conceptScheme: ;
    skos:prefLabel "Post Fleet Management" .

:0101  a crs:Function, ra:Class,
        skos:Concept ;
    crs:isPerformedBy [ crs:hasAgent ca:2069 ] ;
    dct:source ras:2007-00213478 ;
    skos:definition """The function of producing a range of philatelic items including all processes from initial planning through to distribution. It includes research, planning, design, printing, packaging, marketing, and
distribution of philatelic and related products.""";
    skos:inScheme :conceptScheme: ;
    skos:prefLabel "Stamp Management" .

:0102  a crs:Function, ra:Class,
        skos:Concept ;
    crs:isPerformedBy [ crs:hasAgent ca:2069 ] ;
    dct:source ras:2007-00213478 ;
    skos:definition "The function of applying broad systematic management planning for the agency. Includes business and strategic planning, identifying business partners and new business opportunities and building strategic alliances, developing benchmarking strategies and business growth plans (expansion, extension, and diversification) and managing fraud and insurance coverage." ;
    skos:inScheme :conceptScheme: ;
    skos:prefLabel "Strategic Planning And Management" .

:0103  a crs:Function, ra:Class,
        skos:Concept ;
    crs:isPerformedBy [ crs:hasAgent ca:2107 ] ;
    dct:source ras:2007-00025460 ;
    skos:definition "The function of commemoration of the service and sacrifice of veterans and those who served in wars, conflicts and peace operations. Includes managing officiai missions, funding commemorative projects, compiiing and maintaining nominal rolls, constructing and maintaining battle exploit memorials, war cemeteries and individual war graves in Australia and overseas, promoting community awareness of commemoration programs and events, and protection of the word 'Anzac'." ;
    skos:inScheme :conceptScheme: ;
    skos:prefLabel "Commemoration" .

:0104  a crs:Function, ra:Class,
        skos:Concept ;
    crs:isPerformedBy [ crs:hasAgent ca:2107 ] ;
    dct:source ras:2007-00025460 ;
    skos:definition "The function of providing assistance for home purchase and repairs, and house and contents insurance for eligible persons. Includes the design, construction and disposal of war service homes, the acquisition of houses and land, the development of land for housing construction and the granting of home loans." ;
    skos:inScheme :conceptScheme: ;
    skos:prefLabel "Housing Assistance" .

:0105  a crs:Function, ra:Class,
        skos:Concept ;
    crs:isPerformedBy [ crs:hasAgent ca:2107 ] ;
    dct:source ras:2007-00025460 ;
    skos:definition "The function of managing the appointment and terms and conditions of statutory appointees, such as the Director of War Graves. Includes the payment of allowances and remuneration, and the management of leave entitlements, travel arrangements and separation from office." ;
    skos:inScheme :conceptScheme: ;
    skos:prefLabel "Statutory Appointments" .

:0106  a crs:Function, ra:Class,
        skos:Concept ;
    crs:isPerformedBy [ crs:hasAgent ca:2141 ] ;
    dct:source ras:2004-00406090 ;
    skos:definition "The function of providing actuarial services to the Commonwealth Government and its agencies, international governments and private sector in relation to the management of financial risk. Includes provision of consultancy services, on a 'user pay' arrangement, relating to Commonwealth, civilian and defence superannuation schemes, military compensation schemes, long-term financial liabilities and risks including long service leave and workers compensation. Also includes provision of technical and related policy advice to support the prudential supervision of the financial services sector. " ;
    skos:inScheme :conceptScheme: ;
    skos:prefLabel "Actuarial Services" .

:0107  a crs:Function, ra:Class,
        skos:Concept ;
    crs:isPerformedBy [ crs:hasAgent ca:2141 ] ;
    dct:source ras:2004-00406090 ;
    skos:definition "The function of developing budget policies and framework, the assessment of Commonwealth budget position and outlook, and the preparation of budget and related documents. Includes review of Government expenditure and major Government programs, compliance with relevant legislation, forecasting of revenues and quality assurance of financial statements. " ;
    skos:inScheme :conceptScheme: ;
    skos:prefLabel "Commonwealth Budget" .

:0108  a crs:Function, ra:Class,
        skos:Concept ;
    crs:isPerformedBy [ crs:hasAgent ca:2141 ],
        [ crs:hasAgent ca:2141 ] ;
    dct:source ras:2004-00406090,
        ras:2009-00772254 ;
    skos:definition "The function of developing and implementing Commonwealth-State financial arrangements. Includes development of policy frameworks, provision of advice on various issues arising in a Commonwealth-State context, monitoring Commonwealth-State fiscal developments, development and implementation of inter-governmental agreements between the Commonwealth, States, and Territories and administration of the revenue payments to State and Territory governments. Includes regular meetings and liaison between Commonwealth and State officials on matters of mutual interest such as economic conditions, fiscal reporting, taxation and financial issues. " ;
    skos:inScheme :conceptScheme: ;
    skos:prefLabel "Commonwealth-State Financial Relations" .

:0109  a crs:Function, ra:Class,
        skos:Concept ;
    crs:isPerformedBy [ crs:hasAgent ca:2141 ] ;
    dct:source ras:2004-00406090 ;
    skos:definition "The function of formulating marcoeconomic policies (fiscal and monetary) and implementing Government decisions contributing to sound domestic economy including policy advice on social and labour markets issues. Includes monitoring and assessment of current and prospective Australian economic conditions and developments, analysis of their implications for general financial and economic policy, provision of macroeconomic forecasts to inform policy settings, and undertaking research and analysis of trends in the economy. Also includes extensive liaison with business, to assist in the monitoring and analysing of conditions and prospects, developing and maintaining economic models and reporting. " ;
    skos:inScheme :conceptScheme: ;
    skos:prefLabel "Domestic Economy" .

:0110  a crs:Function, ra:Class,
        skos:Concept ;
    crs:isPerformedBy [ crs:hasAgent ca:2141 ],
        [ crs:hasAgent ca:2141 ] ;
    dct:source ras:2004-00406090,
        ras:2009-00772254 ;
    skos:definition "The function of developing and implementing foreign investment policy, examination and approval of proposals by foreign interests for acquisitions and new investment projects in Australia. Includes advising Government on foreign investment generally, provision of guidance to foreign investors, monitoring and compliance with the foreign investment policy under the relevant legislation. " ;
    skos:inScheme :conceptScheme: ;
    skos:prefLabel "Foreign Investment" .

:0111  a crs:Function, ra:Class,
        skos:Concept ;
    crs:isPerformedBy [ crs:hasAgent ca:2141 ] ;
    dct:source ras:2004-00406090 ;
    skos:definition "The function of consulting, coordinating and developing industry and environment policies and projects. Includes provision of independent advice to the Treasurer, economic analysis of project proposals and their financing arrangements, and providing advice on alternative arrangements and the economic benefits and costs. Also includes input into reviews of existing projects and close collaboration with other agencies on progressing reforms in areas of industry, agriculture, regional development, small business and the environment. " ;
    skos:inScheme :conceptScheme: ;
    skos:prefLabel "Industry And Environmental Economics" .

:0112  a crs:Function, ra:Class,
        skos:Concept ;
    crs:isPerformedBy [ crs:hasAgent ca:2141 ] ;
    dct:source ras:2004-00406090 ;
    skos:definition "The function of development and implementation of policies relating to international economic arrangements. Includes provision of advice on international macroeconomic issues, forecasting, monitoring and analysing of developments in key global economies, Australia's major trading partners and other economies of interest and enhancing cooperation with economies in the region, active representation and participation in international financial institutions and other forums, provision of financial and technical assistance, and mutual recognition of standards and codes.  " ;
    skos:inScheme :conceptScheme: ;
    skos:prefLabel "International Economic Affairs" .

:0113  a crs:Function, ra:Class,
        skos:Concept ;
    crs:isPerformedBy [ crs:hasAgent ca:2141 ],
        [ crs:hasAgent ca:2141 ] ;
    dct:source ras:2004-00406090,
        ras:2009-00772254 ;
    skos:definition "The function of developing and implementing policies, strategies, legislative frameworks and reforms to ensure effective financial systems & markets and sound corporate practices. Includes activities associated with provision of advice to Government, Ministers and various government agencies on specific issues, including ministerial consent advice; consultations with stakeholders, liaison between the Department and State, Territory government agencies, industry, business, lobby groups, monitoring of the developments and trends in markets and financial systems and policy formulation in areas such as prudential supervision, corporate governance, competition and trade practices, reforms in key infrastructure sectors, industry self-regulation etc. Also includes provision of consumer information, raising the level of financial literacy, development and review of mandatory standards for general consumer products, licensing of smokeless tobacco, administration of product safety, resolving takeover disputes and provision of ad-hoc financial assistance to policyholders or members of failed insurance companies and superannuation funds.",
        "The function of developing and implementing policies, strategies, legislative frameworks and reforms to ensure effective financial systems and markets and sound corporate practices. Includes activities associated with provision of advice to Government, Ministers and various Government agencies on specific issues, including Ministerial consent advice, consultations with stakeholders, liaison between the Department and State and Territory Government agencies, industry, business, lobby groups, monitoring of the developments and trends in markets and financial systems and policy formulation in areas such as prudential supervision, corporate governance, competition and trade practices, reforms in key infrastructure sectors, industry self-regulation etc. Also includes provision of consumer information, development and review of mandatory standards for general consumer products, licensing of smokeless tobacco, administration of product safety, resolving takeover disputes and provision of ad hoc financial assistance to policyholders or members of failed insurance companies and superannuation funds. " ;
    skos:inScheme :conceptScheme: ;
    skos:prefLabel "Markets Regulation" .

:0114  a crs:Function, ra:Class,
        skos:Concept ;
    crs:isPerformedBy [ crs:hasAgent ca:2141 ],
        [ crs:hasAgent ca:2141 ] ;
    dct:source ras:2004-00406090,
        ras:2009-00772254 ;
    skos:definition "The function of supporting and coordinating governance arrangements of Treasury's portfolio bodies. Includes agreements on work arrangements, appointments, advice, accountability, performance and setting up reviews and coordination of budgets and levies. Also includes work planning, reporting and regular review of their operations. " ;
    skos:inScheme :conceptScheme: ;
    skos:prefLabel "Portfolio Governance" .

:0115  a crs:Function, ra:Class,
        skos:Concept ;
    crs:isPerformedBy [ crs:hasAgent ca:2141 ] ;
    dct:source ras:2004-00406090 ;
    skos:definition "The function of administering formal reviews and inquiries on behalf of the Government. Includes carrying out research, provision of advice, receiving submissions, consultations with stakeholders and issuing reports. Also includes coordination of appointments of members, advertising, relations with media and providing ongoing secretariat support. " ;
    skos:inScheme :conceptScheme: ;
    skos:prefLabel "Reviews And Inquiries Coordination" .

:0116  a crs:Function, ra:Class,
        skos:Concept ;
    crs:isPerformedBy [ crs:hasAgent ca:2141 ] ;
    dct:source ras:2009-00794784 ;
    skos:definition """The core business of managing the Standard Business Reporting (SBR) Program, a Commonwealth Government initiative, endorsed by the Council of Australian Governments (COAG) to simplify business-to-government reporting in Commonwealth, State and Territory jurisdictions.

Includes:
• establishing the program board, steering committee, business advisory forum and other taskforces, panels and committees
• establishing and implementing governance arrangements
• liaison, consultation and collaboration with internal and external stakeholders, software developers and consultants
• liaison, consultation and collaboration with other Commonwealth agencies as well as state, territory and international government agencies
• establishing agreements with other Commonwealth agencies as well as state, territory and international government agencies
• developing and applying broad systematic planning for the program
• managing the program to ensure objectives are met
• reviewing and reporting against program objectives and plans
• designing, developing, planning, testing and implementing solutions to meet program objectives
• providing and receiving advice regarding the program
• arranging and attending internal and external meetings
• delivering addresses and presentations and holding conferences regarding the program, and
• driving the take-up of SBR services through the accounting and business communities.""";
    skos:inScheme :conceptScheme: ;
    skos:prefLabel "Standardising Business Reporting" .

:0117  a crs:Function, ra:Class,
        skos:Concept ;
    crs:isPerformedBy [ crs:hasAgent ca:2141 ] ;
    dct:source ras:2004-00406090 ;
    skos:definition "The function of developing, designing and implementing legislation and policies relating to national and international taxation, retirement income systems and income support systems. Includes activities associated with provision of advice to Government, Ministers and other Government agencies on specific issues, analysis of taxation payments arrangements and key features of retirement income system, review and evaluation of business tax systems and international tax arrangements, monitoring the operation of business tax regimes, consultations with stakeholders, liaison between the Department and other Government agencies, industry and business, reporting of tax expenditures and negotiating tax treaties. Also includes economic modelling, revenue forecasting and management of ad hoc programs resulting from taxation reforms. " ;
    skos:inScheme :conceptScheme: ;
    skos:prefLabel "Taxation And Income Support" .

:0118  a crs:Function, ra:Class,
        skos:Concept ;
    crs:isPerformedBy [ crs:hasAgent ca:2260 ] ;
    dct:source ras:2001-04538412 ;
    skos:definition "The function of classifying against established criteria. Includes assessment and classification of children's programs by staff or consultants against the Children's Television Standards, determination of adult telephone services and issue of evidentiary certificates, opinions regarding licence categories and control opinions. Also includes plans, procedures and policies and reports regarding classification. " ;
    skos:inScheme :conceptScheme: ;
    skos:prefLabel "Classification" .

:0119  a crs:Function, ra:Class,
        skos:Concept ;
    crs:isPerformedBy [ crs:hasAgent ca:2260 ] ;
    dct:source ras:2001-04538412 ;
    skos:definition "The function of educating the community regarding broadcasting, datacasting or Internet issues. Includes the policies, procedures and plans supporting the education function." ;
    skos:inScheme :conceptScheme: ;
    skos:prefLabel "Education" .

:0120  a crs:Function, ra:Class,
        skos:Concept ;
    crs:isPerformedBy [ crs:hasAgent ca:2260 ] ;
    dct:source ras:2001-04538412 ;
    skos:definition "The function of monitoring broadcasting, datacasting and Internet trends and technologies, liaising with international bodies regarding trends and technologies, and reporting to the Minister." ;
    skos:inScheme :conceptScheme: ;
    skos:prefLabel "Industry Technology" .

:0121  a crs:Function, ra:Class,
        skos:Concept ;
    crs:isPerformedBy [ crs:hasAgent ca:2260 ] ;
    dct:source ras:2001-04538412 ;
    skos:definition "The function of allocating service and issuing apparatus licences for broadcasting and datacasting. Includes the allocation of temporary licences for community broadcasters where spectrum planning has not been completed, consultation, and hearings arranged by the Australian Broadcasting Authority regarding the allocation or issue of licences. Also includes procedures, policies and reports regarding the licensing function. " ;
    skos:inScheme :conceptScheme: ;
    skos:prefLabel "Licensing" .

:0122  a crs:Function, ra:Class,
        skos:Concept ;
    crs:isPerformedBy [ crs:hasAgent ca:2260 ] ;
    dct:source ras:2001-04538412 ;
    skos:definition "The function of monitoring and ensuring compliance with the broadcastingand Internet requirements outlined in broadcasting services legislation, licences and licence conditions, standards and codes of practice. Includes data and fee collection, consultation, determinations and declarations regarding monitoring and enforcement, rights management, complaints management breaches and investigations, licence monitoring, adding or varying licence conditions, and enforcing penalties. Also includes procedures, policies and reports regarding the monitoring and enforcement function. " ;
    skos:inScheme :conceptScheme: ;
    skos:prefLabel "Monitoring And Enforcement" .

:0123  a crs:Function, ra:Class,
        skos:Concept ;
    crs:isPerformedBy [ crs:hasAgent ca:2260 ] ;
    dct:source ras:2001-04538412 ;
    skos:definition "The function of developing, commenting on or reviewing major broadcasting, datacasting and Internet policy. Includes Ministerially directed policy reviews. Also includes procedures and reports regarding the policy projects function." ;
    skos:inScheme :conceptScheme: ;
    skos:prefLabel "Policy Projects" .

:0124  a crs:Function, ra:Class,
        skos:Concept ;
    crs:isPerformedBy [ crs:hasAgent ca:2260 ] ;
    dct:source ras:2001-04538412 ;
    skos:definition "The function of conducting or commissioning major research into broadcasting, datacasting or Internet issues. Includes attitudinal research, economic, industry and financial analysis and procedures, policies and reports regarding the research projects function." ;
    skos:inScheme :conceptScheme: ;
    skos:prefLabel "Research Projects" .

:0125  a crs:Function, ra:Class,
        skos:Concept ;
    crs:isPerformedBy [ crs:hasAgent ca:2260 ] ;
    dct:source ras:2001-04538412 ;
    skos:definition "The function of planning the availability of segments of the broadcasting service bands for analog radio and digital radio and television. Includes developing and consulting on frequency allotment plans, licence area plans, digital channel plans, technical/engineering plans and conversion schemes and the determination of licence areas, population and plan priorities. Also includes procedures, policies and reports regarding the planning function. " ;
    skos:inScheme :conceptScheme: ;
    skos:prefLabel "Spectrum Planning" .

:0126  a crs:Function, ra:Class,
        skos:Concept ;
    crs:isPerformedBy [ crs:hasAgent ca:2260 ] ;
    dct:source ras:2001-04538412 ;
    skos:definition "The function of managing standards and codes for broadcasting, datacasting and the Internet in Australia. Includes developing, consulting on and reviewing technical standards and standards covering issues like program content; assisting broadcasters in the development of codes of practice; registration of codes; and the development of standards where codes are not adequate. Also includes plans, procedures and reports regarding the standard management function. " ;
    skos:inScheme :conceptScheme: ;
    skos:prefLabel "Standards Management" .

:0127  a crs:Function, ra:Class,
        skos:Concept ;
    crs:isPerformedBy [ crs:hasAgent ca:2280 ] ;
    dct:source ras:2009-00922958 ;
    skos:definition """The business of managing the operations of the agency's aquarium. The aquarium is the educational centre of the Great Barrier Reef Marine Park Authority and raises awareness of the reef by developing and managing educational programs, collections and exhibits based around the world's largest living coral reef aquarium.

This work includes the specific tasks of:
•	awards presented to the Aquarium;
•	coordinating and managing customer service aspects of the aquarium;
•	receipt and processing of donations;
•	promoting, developing and implementing education programs;
•	research, development and coordination of core and permanent exhibitions;
•	managing functions, celebrations and commemorative events;
•	coordination and maintenance of living exhibits;
•	aquarium construction and maintenance;
•	marketing the aquarium to local, national and international customers; and
•	managing volunteering, sponsorship and membership programs and databases.

The performance of the business is supported by routine administrative tasks such as:
•	giving and receiving advice;
•	negotiating and establishing agreements;
•	receiving and responding to enquiries;
•	managing meetings; and
•	development of policies and procedures.""";
    skos:inScheme :conceptScheme: ;
    skos:prefLabel "Aquarium Operations" .

:0128  a crs:Function, ra:Class,
        skos:Concept ;
    crs:isPerformedBy [ crs:hasAgent ca:2280 ] ;
    dct:source ras:2009-00922958 ;
    skos:definition """The business of maintaining islands and sea-based areas of the natural environment within the Marine Park. Programs are developed to conserve plant and animal life; to enhance the sustainability of ecosystems; and to promote community awareness and participation in conservation activities.  The implementation of programs enhances the legislation and regulations protecting the Reef by increasing stakeholders' stewardship and awareness levels and enhances the social marketing ability of the agency.

This work includes the specific tasks of:
•	the management of joint ventures;
•	program management including development and implementation; and
•	research programs undertaken or funded by the Agency.

The performance of the business is supported by routine administrative tasks such as:
•	delivery of addresses to stakeholders;
•	giving and receiving advice;
•	negotiation and establishment of agreements;
•	establishment and management of committees;
•	receiving and responding to enquiries;
•	development of policies and procedures;
•	reporting requirements; and
•	reviewing programs or research projects.""";
    skos:inScheme :conceptScheme: ;
    skos:prefLabel "Marine Life Protection Programs" .

:0129  a crs:Function, ra:Class,
        skos:Concept ;
    crs:isPerformedBy [ crs:hasAgent ca:2280 ] ;
    dct:source ras:2009-00922958 ;
    skos:definition """The core business of establishing networks with the agency’s stakeholders and maintaining the organisation’s broad public profile.  Stakeholders refer to the Minister, government departments, businesses and groups (Australian and international) who have an interest in the Reef’s longevity.  This also includes individuals in the community who are not adequately represented by a stakeholder group.
This work includes the specific tasks of:
•	giving and receiving advice;
•	establishment and management of committees such as intergovernmental committees and round tables;
•	coordinating and managing customer service aspects;
•	exhibitions attendance and management;
•	joint ventures involving stakeholders;
•	marketing programs including sponsorship of events and social marketing;
•	media relations including original Agency press releases and media contacts;
•	agency staff appointed to representative roles or external appointments to Agency committees;
•	visits to the Agency by dignitaries or Agency staff visitations to lead stakeholders e.g. Agency staff providing assistance and knowledge to tsunami affected countries; and
•	international advisory committees and agreements including International Union for Conservation of Nature (IUCN) or World Heritage documentation.

The performance of the business is supported by routine administrative tasks such as:
•	delivery of addresses to stakeholders;
•	giving and receiving advice;
•	administrative arrangements to enable engagement;
•	establishment and management of committees;
•	organising agency sponsored conferences, staff attendance and speaking requests;
•	receiving and responding to enquiries;
•	managing meetings; and
•	development of procedures.""";
    skos:inScheme :conceptScheme: ;
    skos:prefLabel "Stakeholder Engagement" .

:0130  a crs:Function, ra:Class,
        skos:Concept ;
    crs:isPerformedBy [ crs:hasAgent ca:2280 ] ;
    dct:source ras:2009-00922958 ;
    skos:definition """The business of managing the Great Barrier Reef ecosystem using legislation, regulations and the subsequent standards, policies and permitting guidelines which are implemented for sustainable usage of the Marine Park. This work includes the specific tasks of:
•	advice regarding legislative requirements including:
o	development proposals;
•	compliance to legislation including:
o	enforcement;
o	field-based management;
o	illegal fishing activities;
o	marine pollution;
o	pre & post patrol reports; and
o	surveillance.
•	joint ventures with major stakeholders encompassing Codes of Conduct and operating procedures that have been agreed to by the agency and major stakeholders;
•	litigation of alleged breaches of Act;
•	marine park permits process involving granting, allocation, latency, tenure and compliance to the permit relating to research, tourism,  harvest/fishing;
•	marine park planning including the organisation’s mandate to create, implement and enforce zoning plans and plans of management for the protection of the Marine Park including:
o	aquaculture;
o	environmental management plans for scientific research zones;
o	plans of management;
o	ports;
o	recovery plans;
o	representative area program;
o	shipping;
o	site management plans and arrangements;
o	threat abatement plans;
o	Traditional Use of Marine Resources Agreements (TUMRAs) Accreditation; and
o	zoning plans.
•	legislatively required reporting processes e.g. Outlook Report;
•	stakeholder submissions inviting comments on proposed policies;
•	statutory reconsiderations;
•	user pays charge administration e.g. Environmental Management Charge (EMC); and
•	The performance of the business is supported by routine administrative tasks such as:
o	giving and receiving advice;
o	agreements;
o	Establishment and management of committees;
o	receiving and responding to enquiries;
o	development of policies and procedures; and
o	reviewing programs""";
    skos:inScheme :conceptScheme: ;
    skos:prefLabel "Statutory Obligations" .

:0131  a crs:Function, ra:Class,
        skos:Concept ;
    crs:isPerformedBy [ crs:hasAgent ca:2531 ] ;
    dct:source ras:2001-00000628 ;
    skos:definition "The function of establishing and changing the organisational structure of the agency. Includes reducing and increasing staffing levels and internal reorganisation." ;
    skos:inScheme :conceptScheme: ;
    skos:prefLabel "Agency Establishment" .

:0132  a crs:Function, ra:Class,
        skos:Concept ;
    crs:isPerformedBy [ crs:hasAgent ca:2531 ] ;
    dct:source ras:2001-00000628 ;
    skos:definition "The function of managing members and employees of the agency. Includes volunteer workers." ;
    skos:inScheme :conceptScheme: ;
    skos:prefLabel "Agency Personnel" .

:0133  a crs:Function, ra:Class,
        skos:Concept ;
    crs:isPerformedBy [ crs:hasAgent ca:2531 ] ;
    dct:source ras:2001-00000628 ;
    skos:definition "The function of managing the agency in compliance with its establishing legislation. Includes activities of the Board of Management and Full Commission, and any delegations by management committees or commissioners." ;
    skos:inScheme :conceptScheme: ;
    skos:prefLabel "Corporate Governance" .

:0134  a crs:Function, ra:Class,
        skos:Concept ;
    crs:isPerformedBy [ crs:hasAgent ca:2531 ] ;
    dct:source ras:2001-00000628 ;
    skos:definition "The function of conducting a law reform program in response to references given to the agency by the Attorney-General. Includes conducting research and consultation through a team on each reference to determine the need for reform, and to develop law reform recommendations." ;
    skos:inScheme :conceptScheme: ;
    skos:prefLabel "Law Reform" .

:0135  a crs:Function, ra:Class,
        skos:Concept ;
    crs:isPerformedBy [ crs:hasAgent ca:2922 ] ;
    dct:source ras:2009-00179026 ;
    skos:definition """The core business of developing and undertaking business activities on a commercial basis by the organisation. It includes content, airtime and merchandise sales, and the provision of language, pay television and production services.  Also includes:
• Managing requests and delivery of commercial goods and services
• Establishing agreements for the sale of products by the organisation
• The auditing of commercial activities
• Attending and hosting commercial functions and events
• Managing business ventures and independent commissioning companies
• Marketing commercial goods and services
• Establishing commercial policies and procedures, and determining prices for goods and services
• Reporting on commercial activities""";
    skos:inScheme :conceptScheme: ;
    skos:prefLabel "Commercial Activities" .

:0136  a crs:Function, ra:Class,
        skos:Concept ;
    crs:isPerformedBy [ crs:hasAgent ca:2922 ] ;
    dct:source ras:2009-00179026 ;
    skos:definition "The core business of managing the organisation's relationship with the broader multicultural community and its audiences.  Includes consultation with various multicultural groups, support for community advisory committees, the management of audience reaction to the organisation's broadcasting services, consultation with audience and potential audience members, and audience research.  Also includes receiving community awards, conducting audience competitions, developing the organisation's corporate brand, and participating in public events." ;
    skos:inScheme :conceptScheme: ;
    skos:prefLabel "Community And Audience Relations" .

:0137  a crs:Function, ra:Class,
        skos:Concept ;
    crs:isPerformedBy [ crs:hasAgent ca:2922 ] ;
    dct:source ras:2009-00179026 ;
    skos:definition """The core business of acquiring, producing, storing and delivering content for television, radio and online services.  Includes:
• Pre-production, production and post-production activities such as content proposals, production scheduling, arranging resources, obtaining any necessary approvals/permits, recording the content, evaluating and preparing content for broadcast.
• Marketing activities to promote content to the public.
• Bidding for broadcast and communication rights
• Managing rights agreements
• Attending and presenting at related conferences and similar events
• Providing and receiving production advice
• Commissioning productions
• Participating in related committees
• Complying with closed captioning requirements
• Maintaining the organisation’s program inventory/library
• Developing policies and procedures
• Scheduling and presenting content to audiences.""";
    skos:inScheme :conceptScheme: ;
    skos:prefLabel "Content Management" .

:0138  a crs:Function, ra:Class,
        skos:Concept ;
    crs:isPerformedBy [ crs:hasAgent ca:2922 ] ;
    dct:source ras:2009-00179026 ;
    skos:definition """The core business of developing and delivering accredited training to the organisation's staff and non-accredited training to external clients. Includes:
• Accreditation of the organisation (as a registered training organisation)
• Planning and building training programs
• Providing the training
• Assessing trainees
• Awarding of certificates and statements of attainment in relation to the training.
• Handling trainee grievances and appeals
• Promoting the training
• Developing and promulgating associated policies and procedures.""";
    skos:inScheme :conceptScheme: ;
    skos:prefLabel "Media Training" .

:0139  a crs:Function, ra:Class,
        skos:Concept ;
    crs:isPerformedBy [ crs:hasAgent ca:2922 ] ;
    dct:source ras:2009-00179026 ;
    skos:definition """The core business of planning, developing and managing network infrastructure to enable the transmission and distribution of the organisation's content. Includes:
• Managing relationships with external providers of infrastructure
• Monitoring network performance
• Reporting and rectifying network faults
• Planning and developing transmission sites and new broadcast technologies
• Acquiring and maintaining broadcast site licences, and
• Assisting local communities to establish transmitters.""";
    skos:inScheme :conceptScheme: ;
    skos:prefLabel "Transmission And Distribution Infrastructure" .

:0140  a crs:Function, ra:Class,
        skos:Concept ;
    crs:isPerformedBy [ crs:hasAgent ca:2965 ] ;
    dct:source ras:2009-00046614 ;
    skos:definition "The drafting of Bills and amendments to Bills for introduction into either House of the Commonwealth Parliament, arranging the introduction of Bills and amendments to Bills and the Royal Assent of legislation. Includes receiving instructions from agencies to draft legislation, clarifying policy issues with instructing agencies, drafting legislation and sending draft legislation to instructing agencies and other interested agencies for comment, receiving further instructions from instructing agencies and revising drafts according to those instructions, ensuring that legislation is within policy authority; providing advice and liaising with agencies to resolve legal issues that may arise, including advising the need to seek Australian Government Solicitor (AGS) advice, submitting drafts and authority memoranda for legislation approval process clearance, and arranging Royal Assent for legislation that has passed both Houses of Parliament." ;
    skos:inScheme :conceptScheme: ;
    skos:prefLabel "Legislative Drafting" .

:0141  a crs:Function, ra:Class,
        skos:Concept ;
    crs:isPerformedBy [ crs:hasAgent ca:2965 ] ;
    dct:source ras:2009-00046614 ;
    skos:definition "The training of drafters in legislative drafting to ensure the long-term viability of drafting resources and to maintain and improve drafting skills and knowledge. The conduct of legislation process courses for instructors to ensure potential instructors are trained in policy development and preparation of instructions. Includes team arrangements for drafters, the role of the Director of Drafter Training, the development of drafting skills through supervision and training, and organising and running legislation process courses." ;
    skos:inScheme :conceptScheme: ;
    skos:prefLabel "Legislative Drafting Capability" .

:0142  a crs:Function, ra:Class,
        skos:Concept ;
    crs:isPerformedBy [ crs:hasAgent ca:2965 ] ;
    dct:source ras:2009-00046614 ;
    skos:definition """Allocating drafting work and managing legislative projects to ensure optimum use of drafting resources in accordance with the priorities set by the Parliamentary Business Committee (PBC). Includes First Parliamentary Counsel attending PBC, allocation of drafting resources to drafting projects, monitoring the progress of legislative projects, and meetings with drafters.

Attendance at meetings of Parliamentary Counsel Committee (PCC), Board of Taxation, other bodies, reviews or enquiries in which FPC or other staff have involvement.
""";
    skos:inScheme :conceptScheme: ;
    skos:prefLabel "Program And Project Management " .

:0143  a crs:Function, ra:Class,
        skos:Concept ;
    crs:isPerformedBy [ crs:hasAgent ca:2965 ] ;
    dct:source ras:2009-00046614 ;
    skos:definition """The documentation and promulgation of OPC rules, standards and conventions for drafting.
The editorial checking of draft Bills and amendments to Bills, and the arranging of the publication of draft Bills before introduction into either House of the Parliament. Includes drafting directions, OPC rules, standards and conventions for drafting, completing internal quality control processes such as editorial checking, arranging for the printing of Bills and amendments, obtaining clearance to forward Bills and amendments to Parliament, updating and maintaining the internal database of the text of principal legislation, and monthly meetings of all drafters to discuss drafting issues that are of a general interest.""";
    skos:inScheme :conceptScheme: ;
    skos:prefLabel "Standardisation And Legislation Quality Control" .

:0144  a crs:Function, ra:Class,
        skos:Concept ;
    crs:isPerformedBy [ crs:hasAgent ca:2999 ] ;
    dct:source ras:2006-00446344 ;
    skos:definition "The function of collecting, collating, interpreting and disseminating data and other information on explosive incidents and related matters. Includes the provision of advice on explosives, explosives research, trial and evaluation of explosives and explosive devices, liaison with Australian and international police, security and intelligence agencies and organisations, and the conducting of bomb awareness training. Excludes responses to bomb threats." ;
    skos:inScheme :conceptScheme: ;
    skos:prefLabel "Bomb Data" .

:0145  a crs:Function, ra:Class,
        skos:Concept ;
    crs:isPerformedBy [ crs:hasAgent ca:2999 ] ;
    dct:source ras:2006-00446344 ;
    skos:definition "The function of managing and directing resources to identify, counter or otherwise investigate possible or actual breaches of law either reported or becoming known against a person or property, or the whereabouts of missing people, in the Australian Capital Territory or any Commonwealth Territory with which the agency has an agreement to provide these services. Includes developing potential targets as sources of information or evidence; obtaining warrants and collecting evidence; seizing and managing drugs and property to be used as evidence; the analysis of evidence, including forensic evidence; conducting surveillance and technical operations; conducting enquiries; research and analysis; and liaison with members of the public, government agencies, local and foreign governments." ;
    skos:inScheme :conceptScheme: ;
    skos:prefLabel "Community Investigations" .

:0146  a crs:Function, ra:Class,
        skos:Concept ;
    crs:isPerformedBy [ crs:hasAgent ca:2999 ] ;
    dct:source ras:2006-00446344 ;
    skos:definition "The function of keeping the peace and preserving safety in the Australian Capital Territory and any other Commonwealth Territory with which the agency has an agreement to provide these services. Includes crime prevention and community safety; diversionary conferencing; deterrence of crime; planning; development of policy; property administration; response policing; traffic management; and support to victims of crime services." ;
    skos:inScheme :conceptScheme: ;
    skos:prefLabel "Community Policing" .

:0147  a crs:Function, ra:Class,
        skos:Concept ;
    crs:isPerformedBy [ crs:hasAgent ca:2999 ] ;
    dct:source ras:2006-00446344 ;
    skos:definition "The function of recording the results of criminal prosecutions and providing details of, or extracts from, criminal records as appropriate to Australian government law enforcement agencies, both Federal and State, other government agencies, prosecution, judicial services, international law enforcement agencies and individuals." ;
    skos:inScheme :conceptScheme: ;
    skos:prefLabel "Criminal Records" .

:0148  a crs:Function, ra:Class,
        skos:Concept ;
    crs:isPerformedBy [ crs:hasAgent ca:2999 ] ;
    dct:source ras:2006-00446344 ;
    skos:definition "The function of managing and directing resources to identify, counter or otherwise investigate possible or actual breaches of law either reported or becoming known against a person or property either in Australia or overseas, or the whereabouts of missing people. Includes developing potential targets as sources of information or evidence; obtaining warrants and collecting evidence; seizing and managing drugs and property to be used as evidence; the analysis of evidence, including forensic evidence; conducting surveillance and technical operations; conducting enquiries; research and analysis; and liaison with members of the public, government agencies, local and foreign governments." ;
    skos:inScheme :conceptScheme: ;
    skos:prefLabel "Federal Investigations" .

:0149  a crs:Function, ra:Class,
        skos:Concept ;
    crs:isPerformedBy [ crs:hasAgent ca:2999 ] ;
    dct:source ras:2006-00446344 ;
    skos:definition "The function of managing firearm and prohibited weapon compliance, licensing and registration processes. Includes amnesties for prohibited firearms." ;
    skos:inScheme :conceptScheme: ;
    skos:prefLabel "Firearms And Weapons Control" .

:0150  a crs:Function, ra:Class,
        skos:Concept ;
    crs:isPerformedBy [ crs:hasAgent ca:2999 ] ;
    dct:source ras:2006-00446344 ;
    skos:definition "The function of receiving, registering, storing, and maintaining firearms that are not registered or managed as organisational assets.  Includes liaison with other government agencies, and the short-term lending of firearms in the collection for use as training aids or for other purposes.  Also includes the destruction of firearms that have been received by the organisation and are not included in the reference collection." ;
    skos:inScheme :conceptScheme: ;
    skos:prefLabel "Firearms Collection" .

:0151  a crs:Function, ra:Class,
        skos:Concept ;
    crs:isPerformedBy [ crs:hasAgent ca:2999 ] ;
    dct:source ras:2006-00446344 ;
    skos:definition "The function of collecting, interpreting, analysing and distributing intelligence information. Includes the identification and prioritisation of intelligence targets and the design and implementation of appropriate operational means to collect intelligence. Also includes the development of policies and procedures relating to intelligence programs; the monitoring, evaluation and reviewing of these programs; meeting with other government and non-government organisations, in Australia and overseas, and establishing agreements concerning intelligence activities." ;
    skos:inScheme :conceptScheme: ;
    skos:prefLabel "Intelligence" .

:0152  a crs:Function, ra:Class,
        skos:Concept ;
    crs:isPerformedBy [ crs:hasAgent ca:2999 ] ;
    dct:source ras:2006-00446344 ;
    skos:definition "The function of providing general policing assistance or support to United Nations peace operations, or other overseas operations as directed by Government. Includes the establishment of agreements for peace operations, deployments, liaison with Australian Government agencies and the United Nations, and visits to and from areas where peace operations are carried out." ;
    skos:inScheme :conceptScheme: ;
    skos:prefLabel "International Deployments" .

:0153  a crs:Function, ra:Class,
        skos:Concept ;
    crs:isPerformedBy [ crs:hasAgent ca:2999 ] ;
    dct:source ras:2006-00446344 ;
    skos:definition "The function of developing and maintaining international alliances with law enforcement and other relevant agencies, including Interpol and Europol. Includes liaison with other police forces, the conduct of police enquiries and policing assistance" ;
    skos:inScheme :conceptScheme: ;
    skos:prefLabel "International Policing" .

:0154  a crs:Function, ra:Class,
        skos:Concept ;
    crs:isPerformedBy [ crs:hasAgent ca:2999 ] ;
    dct:source ras:2006-00446344 ;
    skos:definition """The function of managing all employees, including volunteer workers, in the organisation employed under the federal police and other legislation. Includes review of actions, overtime, salaries, superannuation and working hours for individuals.  It also includes: recognition and awards; the conduct of internal investigations as part of professional standards; drug and alcohol testing; psychological services; and the management of undercover and covert operatives.
""";
    skos:inScheme :conceptScheme: ;
    skos:prefLabel "Law Enforcement Personnel" .

:0155  a crs:Function, ra:Class,
        skos:Concept ;
    crs:isPerformedBy [ crs:hasAgent ca:2999 ] ;
    dct:source ras:2006-00446344 ;
    skos:definition "The function of creating and providing, through the agency's own training centre, training programs related to law enforcement for staff and staff from other Government agencies. Includes the provision of accredited training, recruit training and ongoing enhancement of skills." ;
    skos:inScheme :conceptScheme: ;
    skos:prefLabel "Law Enforcement Training" .

:0156  a crs:Function, ra:Class,
        skos:Concept ;
    crs:isPerformedBy [ crs:hasAgent ca:2999 ] ;
    dct:source ras:2006-00446344 ;
    skos:definition "The function of collecting, storing and managing artefacts that document or relate to the history of the Australian Federal Police and interpreting and presenting this history for wider audiences. Includes developing and maintaining the Museum's collection and associated information, exhibitions, public programmes, loans, Friends organisation and marketing." ;
    skos:inScheme :conceptScheme: ;
    skos:prefLabel "Police Museum" .

:0157  a crs:Function, ra:Class,
        skos:Concept ;
    crs:isPerformedBy [ crs:hasAgent ca:2999 ] ;
    dct:source ras:2006-00446344 ;
    skos:definition "The function of bringing evidence and a person or persons before the courts for prosecution. Includes the provision of relevant briefing materials, evidence and witnesses as required. Also, includes: the processing and execution of orders, warrants and summons." ;
    skos:inScheme :conceptScheme: ;
    skos:prefLabel "Prosecution And Judicial Support" .

:0158  a crs:Function, ra:Class,
        skos:Concept ;
    crs:isPerformedBy [ crs:hasAgent ca:2999 ] ;
    dct:source ras:2006-00446344 ;
    skos:definition "The function of protecting and guarding the safety of high office holders, government officials, diplomats and diplomatic missions, guests of government, and other protected persons and witnesses through close personal protection, and the guarding of persons identified to be at risk. Includes the protection of establishments and assets such as aviation and defence facilities; Commonwealth, diplomatic and other premises; and sensitive, portable physical assets in transit. Also includes the provision of specially trained officers and the provision of measures as determined under established witness protection methodologies." ;
    skos:inScheme :conceptScheme: ;
    skos:prefLabel "Protective Security" .

:0159  a crs:Function, ra:Class,
        skos:Concept ;
    crs:isPerformedBy [ crs:hasAgent ca:3238 ] ;
    dct:source ras:2008-00422945 ;
    skos:definition """The business of investigating complaints made against Australian Government agencies. The work includes:
• Providing information to complainants about the role of the Commonwealth Ombudsman and a number of access channels
• Determining the complaints that will and will not be investigated, and referring out of jurisdiction complaints to alternative oversight bodies
• Developing, refining, promulgating and reviewing associated legislation and policy
• Investigating complaints
• Internal and external liaison to identify and achieve an appropriate resolution for the complainant
• Identifying areas / systems / policies for agency improvement
• Offering internal review of our decisions and mechanisms through which complainants can provide feedback about our service.
Explanatory Note: The approach categories 1-5 used in the class descriptions below are defined in the Commonwealth Ombudsman Work Practice Manual. Approaches are escalated through the categories
as their complexity increases. These may from time to time change in substance or detail. For the purposes of this records authority, the category of an approach on closure as described below determines the class to which it belongs.""";
    skos:inScheme :conceptScheme: ;
    skos:prefLabel "Complaint Investigations" .

:0160  a crs:Function, ra:Class,
        skos:Concept ;
    crs:isPerformedBy [ crs:hasAgent ca:3238 ] ;
    dct:source ras:2008-00422945 ;
    skos:definition """The business of conducting compliance audits into the use of intrusive powers by Australian Government agencies. Includes:
• The identification of an appropriate record sample
• Analysis of agency records and comparison with statutory, regulatory or policy requirements
• Preparation of a report that identifies areas of non-compliance and areas where there could be a closer alignment with best practice
• Drafting recommendations to help agencies achieve full compliance
• Following-up findings and recommendations in subsequent audits.""";
    skos:inScheme :conceptScheme: ;
    skos:prefLabel "Compliance Audits" .

:0161  a crs:Function, ra:Class,
        skos:Concept ;
    crs:isPerformedBy [ crs:hasAgent ca:3238 ] ;
    dct:source ras:2008-00422945 ;
    skos:definition """The business of improving the quality and performance of ombudsman offices in countries within the Asia-Pacific region. Includes:
• Developing and delivering programs in the Asia-Pacific region to reduce poverty and achieve sustainable development
• Supporting the development and implementation of ombudsman best practice
• Promoting good governance and building capacity in the Asia-Pacific region
• Sharing and transferring skills, values and competencies to strengthen ombudsman functions.""";
    skos:inScheme :conceptScheme: ;
    skos:prefLabel "International Programs" .

:0162  a crs:Function, ra:Class,
        skos:Concept ;
    crs:isPerformedBy [ crs:hasAgent ca:3238 ] ;
    dct:source ras:2008-00422945 ;
    skos:definition """The business of conducting an investigation into a major issue, on the Ombudsman’s own initiative (own motion), in response to a statutory requirement or at the request of an agency or Minister,
affecting one or more Australian Government agencies, and providing a written report on the findings. Includes:
• The identification of issues that should properly be the subject of such a report
• Scanning the environment to ensure all relevant agencies are included in the investigation and looking for cross agency issues
• Undertaking a thorough, fair and impartial investigation
• Preparing a report with recommendations and/or findings, negotiated with agencies where appropriate
• Following-up recommendations with the agency to test whether they have resulted in improved customer service, efficiency or compliance
• Research projects.""";
    skos:inScheme :conceptScheme: ;
    skos:prefLabel "Major Investigations And Reports" .

:0163  a crs:Function, ra:Class,
        skos:Concept ;
    crs:isPerformedBy [ crs:hasAgent ca:3589 ] ;
    dct:source ras:2005-00450552 ;
    skos:definition "The function of managing the organisation’s relationship with its audiences and stakeholders in any area.  Includes the management of audience reaction to the organisation and its services, feedback and consultation with audience and potential audience members, and audience research.  Also includes committees and councils, enquiries, audience complaints, awards, publicity, liaison and public events.  " ;
    skos:inScheme :conceptScheme: ;
    skos:prefLabel "Audience And Stakeholder Relations" .

:0164  a crs:Function, ra:Class,
        skos:Concept ;
    crs:isPerformedBy [ crs:hasAgent ca:3589 ] ;
    dct:source ras:2005-00450552 ;
    skos:definition "The function of managing the activities of the organisation’s governing body for which the organisation provides secretariat services. Includes the appointment and separation of board members, arrangements of members’ leave, remuneration, travel, insurance and meetings." ;
    skos:inScheme :conceptScheme: ;
    skos:prefLabel "Board Administration" .

:0165  a crs:Function, ra:Class,
        skos:Concept ;
    crs:isPerformedBy [ crs:hasAgent ca:3589 ] ;
    dct:source ras:2005-00450552 ;
    skos:definition "The function of undertaking commercial activities in relation to the organisation’s broadcast content.  Includes the sale of broadcast content, the development and sale of content-related products, in retail outlets and facilities hire.  Also includes the licensing and registration of business enterprises." ;
    skos:inScheme :conceptScheme: ;
    skos:prefLabel "Commercial Activities" .

:0166  a crs:Function, ra:Class,
        skos:Concept ;
    crs:isPerformedBy [ crs:hasAgent ca:3589 ] ;
    dct:source ras:2005-00450552 ;
    skos:definition "The function of producing content across all output media, including multimedia, television, radio, interactive and online, and providing physical and intellectual management of produced, co-produced, pre-purchased or acquired program material.  Includes producing, co-producing, pre-purchasing, acquiring, commissioning, captioning, classifying and scheduling content. Also includes identifying talent, designing, planning, managing and tracking productions, developing and receiving scripts, recording and filming content, and editing content." ;
    skos:inScheme :conceptScheme: ;
    skos:prefLabel "Content Management And Production" .

:0167  a crs:Function, ra:Class,
        skos:Concept ;
    crs:isPerformedBy [ crs:hasAgent ca:3589 ] ;
    dct:source ras:2005-00450552 ;
    skos:definition "The function of conserving the organisation’s audiovisual content and documenting the organisation’s history. Includes the production of audiovisual content where there is no intent to broadcast." ;
    skos:inScheme :conceptScheme: ;
    skos:prefLabel "Historical Information Management" .

:0168  a crs:Function, ra:Class,
        skos:Concept ;
    crs:isPerformedBy [ crs:hasAgent ca:3589 ] ;
    dct:source ras:2005-00450552 ;
    skos:definition """The function of developing and promoting the appreciation of orchestral music through the composition and performance of music. Includes concerts to schools and to paying audiences.  Also includes the development of artists and conductors, arrangement of orchestral tours, subscription services and ticket sales.

Note: The function does not cover records created after the date of corporatisation of individual orchestras or any support organisation, such as Symphony Australia. The dates of corporatisation are provided in the Application section of this Records Disposal Authority.""";
    skos:inScheme :conceptScheme: ;
    skos:prefLabel "Orchestras" .

:0169  a crs:Function, ra:Class,
        skos:Concept ;
    crs:isPerformedBy [ crs:hasAgent ca:3589 ] ;
    dct:source ras:2005-00450552 ;
    skos:definition "The function of establishing agreements, managing contracts, planning, setting standards and producing technical drawings for the organisation’s production, broadcast and office technology systems, applications and databases." ;
    skos:inScheme :conceptScheme: ;
    skos:prefLabel "Technology" .

:0170  a crs:Function, ra:Class,
        skos:Concept ;
    crs:isPerformedBy [ crs:hasAgent ca:3589 ] ;
    dct:source ras:2005-00450552 ;
    skos:definition "The function of developing and delivering training and consulting services for the organisation’s stakeholders, including international broadcasters.  Includes responding directly to requests from a national or international body, preparing and lodging bids for the provision of services, delivery of training and consultancy services, establishing funding for the services and reporting on the delivery of the services.  Also includes the organisation’s development and delivery of external and internal accredited training (for example as a registered training organisation) and the awarding of certificates and statements of attainment in relation to the accredited training." ;
    skos:inScheme :conceptScheme: ;
    skos:prefLabel "Training And Consultancy Services" .

:0171  a crs:Function, ra:Class,
        skos:Concept ;
    crs:isPerformedBy [ crs:hasAgent ca:3589 ] ;
    dct:source ras:2005-00450552 ;
    skos:definition "The function of delivering and transmitting broadcast content to audiences via a variety of technologies, such as satellite, telephone line and broadband technology. Includes acquiring and managing licenses and permissions of use for transmitters and spectrum, the management of tender projects, contracts with third party suppliers, fault management and the measurement of supplier performance. Also includes the collection of content produced, co-produced or pre-purchased by the organisation that is transmitted to the public." ;
    skos:inScheme :conceptScheme: ;
    skos:prefLabel "Transmission And Distribution" .

:0172  a crs:Function, ra:Class,
        skos:Concept ;
    crs:isPerformedBy [ crs:hasAgent ca:3854 ],
        [ crs:hasAgent ca:3854 ] ;
    dct:source ras:2005-00210284,
        ras:2008-00194021 ;
    skos:definition "The function of managing, conducting and assisting in local government, state, territory and federal elections, ballots, referendums and plebiscites. Includes by-elections, provision of elections for Aboriginal organisations and ballot votes for industrial organisations and various other bodies. Also includes the issue of writs, managing agreements to conduct elections for another party, planning the election process, managing nominations and declarations of candidates, developing rules and procedures for elections, organising polling arrangements, providing polling information, equipment and materials, conducting the elections, sorting and counting votes and reviewing and evaluating aspects of the election system. It also involves identifying non-voters and electoral fraud and challenges to the validity of any election." ;
    skos:inScheme :conceptScheme: ;
    skos:prefLabel "Elections, Ballots And Referendums" .

:0173  a crs:Function, ra:Class,
        skos:Concept ;
    crs:isPerformedBy [ crs:hasAgent ca:3854 ] ;
    dct:source ras:2005-00210284 ;
    skos:definition "The function of providing information and education programs to promote public awareness of electoral matters. Includes providing advice to education authorities on civics curriculum, researching and developing programs to meet the needs of specific target groups, conducting visits to schools and community groups, and the evaluation and review of these services. " ;
    skos:inScheme :conceptScheme: ;
    skos:prefLabel "Electoral Information And Education" .

:0174  a crs:Function, ra:Class,
        skos:Concept ;
    crs:isPerformedBy [ crs:hasAgent ca:3854 ] ;
    dct:source ras:2005-00210284 ;
    skos:definition "The function of administering the public funding of election campaigns and financial disclosure schemes. Includes providing advice on election funding and disclosure returns, conducting compliance audits to ensure parties and associated entities are complying with legislation, carrying out investigations into identified non-compliance cases and providing public access to funding and disclosure records. Also includes the administration of election funding payments and processing of disclosure returns, such as electoral expenditure and donations received. " ;
    skos:inScheme :conceptScheme: ;
    skos:prefLabel "Funding And Disclosure" .

:0175  a crs:Function, ra:Class,
        skos:Concept ;
    crs:isPerformedBy [ crs:hasAgent ca:3854 ] ;
    dct:source ras:2005-00210284 ;
    skos:definition "The function of providing assistance to foreign countries on electoral matters. Includes managing special purpose international assistance projects, such as participating in election observation missions and assisting in United Nations conducted elections. Also includes providing advice and answering enquiries about international electoral services, participating in international electoral conferences, developing, planning and conducting visitor programs and providing expert consultancy assistance. " ;
    skos:inScheme :conceptScheme: ;
    skos:prefLabel "International Electoral Services" .

:0176  a crs:Function, ra:Class,
        skos:Concept ;
    crs:isPerformedBy [ crs:hasAgent ca:3854 ] ;
    dct:source ras:2005-00210284 ;
    skos:definition "The function of registering and deregistering political parties at Federal level. Includes processing applications for registration, appeals against the refusal of the organisation to register a party, reviews of decisions regarding party registration, reviewing eligibility of party registration, and maintaining registers of political parties and agents and ensuring public access to the registers. " ;
    skos:inScheme :conceptScheme: ;
    skos:prefLabel "Party Registration " .

:0177  a crs:Function, ra:Class,
        skos:Concept ;
    crs:isPerformedBy [ crs:hasAgent ca:3854 ] ;
    dct:source ras:2005-00210284 ;
    skos:definition "The function of defining electoral divisions to ensure each State and Territory gains representation in the House of Representatives in proportion to their population. Includes the establishment and administration of committees responsible for receiving and considering submissions, development and dissemination of redistributions, receipt and management of objections and suggestions, holding of public hearings, and the determination and public announcement of electoral boundaries. " ;
    skos:inScheme :conceptScheme: ;
    skos:prefLabel "Redistribution" .

:0178  a crs:Function, ra:Class,
        skos:Concept ;
    crs:isPerformedBy [ crs:hasAgent ca:3854 ] ;
    dct:source ras:2005-00210284 ;
    skos:definition "The function of maintaining electoral rolls that ensures voter entitlements and provides the basis for the planning of electoral events and redistributions. Includes agreements in regards to sharing data to improve the integrity of the electoral roll, processing enrolment forms including changes of details, handling objections to enrolments, appeals and reviews of decisions, producing and supplying roll products, and maintaining joint roll arrangements with the States and Territories. " ;
    skos:inScheme :conceptScheme: ;
    skos:prefLabel "Roll Management" .

:0179  a crs:Function, ra:Class,
        skos:Concept ;
    crs:isPerformedBy [ crs:hasAgent ca:4416 ] ;
    dct:source ras:2001-00000630 ;
    skos:definition "The function of patrolling coastal and offshore areas for the purpose of detecting illegal activity and coordinating interception. Includes the making of agreements and ongoing liaison with other agencies; coordination, conduct and review of air and sea surveillance and interception operations; referral of information from the community at large about suspect illegal activity; the use and control of defensive armaments or weapons; and provision of education and training. " ;
    skos:inScheme :conceptScheme: ;
    skos:prefLabel "Civil Maritime Surveillance And Response" .

:0180  a crs:Function, ra:Class,
        skos:Concept ;
    crs:isPerformedBy [ crs:hasAgent ca:4416 ] ;
    dct:source ras:2001-00000630 ;
    skos:definition "The function of acquiring and breeding dogs for the detection of drugs and other prohibited or restricted imports carried or concealed on persons, and in baggage, parcels, cargo containers, vessels, aircraft and premises. Includes the conduct and support of breeding programs; the sale, donation or giving away of dogs to other agencies and organisations, or individuals; the deployment of dogs and handlers to assist in search operations conducted by Customs and other agencies; the training of dogs and handlers; the kennelling of dogs, including general care and upkeep; the selection of dogs to be trained and used for detection purposes. " ;
    skos:inScheme :conceptScheme: ;
    skos:prefLabel "Detector Dogs" .

:0181  a crs:Function, ra:Class,
        skos:Concept ;
    crs:isPerformedBy [ crs:hasAgent ca:4416 ] ;
    dct:source ras:2001-00000630 ;
    skos:definition "The function of providing advice and assistance to industry through the delivery of concession schemes (eg Policy By-law Scheme, Project By-law Scheme, Tariff Concession Scheme), dumping investigations (including application of anti-dumping and countervailing duties), import tariff quotas, duty drawback schemes, bounty schemes, and other programs and measures. Includes the case management of the provision of particular benefits and entitlements to clients, client training and education, representations from industry representative groups, formal review of decisions, etc. " ;
    skos:inScheme :conceptScheme: ;
    skos:prefLabel "Industry Schemes And Trade Measures" .

:0182  a crs:Function, ra:Class,
        skos:Concept ;
    crs:isPerformedBy [ crs:hasAgent ca:4416 ] ;
    dct:source ras:2001-00000630 ;
    skos:definition "The function of collecting, analysing and distributing value-added, strategic information to meet the organisation's compliance objectives. Includes making of agreements and liaison with other agencies, organisations and governments; development of case files or dossiers; development of intelligence product; tasking or allocation of intelligence product development work; joint ventures with other agencies involved in intelligence gathering; and provision of training to external clients etc." ;
    skos:inScheme :conceptScheme: ;
    skos:prefLabel "Intelligence" .

:0183  a crs:Function, ra:Class,
        skos:Concept ;
    crs:isPerformedBy [ crs:hasAgent ca:4416 ] ;
    dct:source ras:2001-00000630 ;
    skos:definition "The function of facilitating liaison and cooperation with other customs agencies, and international or regional organisations. This includes advising or briefing of agency and other organisations on issues, trends, policies, programs, etc; involvement in the making of international treaties. Memoranda of Understanding and other agreements; holding of bilateral meetings; facilitation of agency participation on international committees; conference facilitation and attendance; international policy agenda development; coordination of the provision of technical assistance to other customs administrations; hosting of visits by officials from other customs administrations and organisations. " ;
    skos:inScheme :conceptScheme: ;
    skos:prefLabel "International Relations" .

:0184  a crs:Function, ra:Class,
        skos:Concept ;
    crs:isPerformedBy [ crs:hasAgent ca:4416 ] ;
    dct:source ras:2001-00000630 ;
    skos:definition "The function of investigating breaches of legislation administered by Customs that have been referred for special enquiries. Includes conduct of case matters involving the initiation, planning, assessment, reporting and review of operations; the interview, search, detention and arrest of persons; surveillance of selected premises and people; securing of crime scenes; seizure of goods; collection and securing of evidence; making of enquiries; making of recommendations and decisions as to whether a case should be prosecuted, terminated or settled out of court. Also includes the preparation of briefs of evidence, obtaining of warrants etc preceding litigation. " ;
    skos:inScheme :conceptScheme: ;
    skos:prefLabel "Investigation" .

:0185  a crs:Function, ra:Class,
        skos:Concept ;
    crs:isPerformedBy [ crs:hasAgent ca:4416 ] ;
    dct:source ras:2001-00000630 ;
    skos:definition "The function of receiving and paying monies in the form of duties, taxes, penalties, drawbacks, refunds, reimbursements, securities, levies, remissions, rebates, bounties, damaged/missing goods claims etc. Includes collection of monies on behalf of other agencies, and the keeping of statistics.  " ;
    skos:inScheme :conceptScheme: ;
    skos:prefLabel "Revenue Management" .

:0186  a crs:Function, ra:Class,
        skos:Concept ;
    crs:isPerformedBy [ crs:hasAgent ca:4416 ] ;
    dct:source ras:2001-00000630 ;
    skos:definition "The function of controlling and facilitating the movement of commercial consignments of goods, including postal items, in and out of Australia. Includes provision of advice relating to tariff classification, goods valuation, and rules of origin; referral of matters to other agencies; making of agreements with clients and agencies (including copyright and trade mark 'objections'); handling of appeals; the clearance of goods for import and export; the control of goods (including withholding) for the purposes of examination, treatment etc; the reporting of cargoes by carriers; the provision of education and training programmes; the enforcement of regulatory requirements relating to payment of duties and taxes, import/export prohibitions and restrictions etc; the handling of matters referred by industry for enquiry; the licensing of brokers and warehouse operators (including monitoring and control of licensee operations); formal review of decisions, the audit and checking of the commercial records of importers, exporters, brokers, carriers and warehouse operators. " ;
    skos:inScheme :conceptScheme: ;
    skos:prefLabel "Trade Facilitation And Compliance" .

:0187  a crs:Function, ra:Class,
        skos:Concept ;
    crs:isPerformedBy [ crs:hasAgent ca:4416 ] ;
    dct:source ras:2001-00000630 ;
    skos:definition "The function of processing passengers, crews and their belongings, and the detection and interception of suspect illegal activity, at the border. Includes referral of matters (eg quarantine, immigration, permit requirements) to other agencies; making of agreements (eg carrier access to Customs computer systems); ship and aircraft arrival/departure reporting; authorisation, including ship and aircraft movement and docking/landing approvals, appointment of ports, airports, wharves and boarding stations; enforcement, including detention and search of passengers; goods control; processing of passengers and non-dutiable belongings through Customs gateways. " ;
    skos:inScheme :conceptScheme: ;
    skos:prefLabel "Travel Facilitation And Compliance" .

:0188  a crs:Function, ra:Class,
        skos:Concept ;
    crs:isPerformedBy [ crs:hasAgent ca:4435 ] ;
    dct:source ras:2009-00822408 ;
    skos:definition """The core business of developing, implementing, managing and evaluating public, education, outreach and exhibition programs, services and resources aimed at engaging national and international audiences to foster awareness and understanding of Australia’s history, culture and society. Audiences are people who make up the organisation's public including visitors, researchers, volunteers, the media, donors, sponsors, other cultural institutions and all consumers or users of organisational products. Includes:
• Establishing policies and principles which guide the core business of audience development;
• Presenting addresses at openings of major exhibitions and new permanent galleries;
• Conducting market research to target potential sponsors and philanthropy donors;
• Managing philanthropic and unsolicited donations of money to the organisation;
• Administering funding to external service providers and non-government organisations for research into practices of interpretation and visitor experiences for public and outreach programs;
• Organising, managing and hosting public programs and corporate functions for the purposes of launching new programs to strengthen existing audiences and attract new audiences;
• Negotiating and establishing agreements with historians, story-tellers, writers, photographers, artists, authors etc to produce works for the organisation;
• Partnering and collaborating with educational organisations in audience development related programs;
• Undertaking research into visitor experiences and practices of interpretation;
• Developing public, educational and outreach programs relating to the organisation’s collections, galleries, research and exhibitions;
• Consulting  stakeholders to obtain authoritative advice, and feedback on the development of audience related programs, services and resources;
• Maintaining general contact between the organisation and Friends of the Museum, international High Commissions and Embassies;
• Arranging and managing visits and guided tours of school groups, young children, families, adults and access groups; and
• Administrative activities such as conduct of meetings and committees, authorising and delegation, compliance, auditing and reporting.

""";
    skos:inScheme :conceptScheme: ;
    skos:prefLabel "Audience Development" .

:0189  a crs:Function, ra:Class,
        skos:Concept ;
    crs:isPerformedBy [ crs:hasAgent ca:4435 ] ;
    dct:source ras:2009-00822408 ;
    skos:definition """The core business of developing and maintaining a national collection of objects and associated materials that represents Australia’s history and cultural heritage. Includes:
• Acquiring, assessing significance, studying, registering, classifying, digitising, researching, de-accessioning, disposal and other activities regarding the management of items and materials forming the agency's collections;
• Planning for and maintaining the collection through preventative conservation and development projects;
• Developing and/or implementing policies, standards and guidelines for the development and management of the Museum's collection;
• Evaluating, reviewing, giving advice on and preparing submissions to support agency collection program and services;
• Management of access to the Museum's collection;
• Promoting the Museum's collection through liaison with other institutions, indigenous groups, the public and other stakeholders;
• Repatriation of indigenous ancestral remains and sacred objects;
• Administrative activities such as conduct of meetings and committees, authorising and delegation, compliance, auditing and reporting.

""";
    skos:inScheme :conceptScheme: ;
    skos:prefLabel """Collection Development And Management
""".

:0190  a crs:Function, ra:Class,
        skos:Concept ;
    crs:isPerformedBy [ crs:hasAgent ca:4435 ] ;
    dct:source ras:2009-00822408 ;
    skos:definition """The core business of providing on a commercial basis, retail services and merchandise sales to the public which are inspired by the organisation’s building, exhibitions and public programs. Includes:
• Arranging and coordinating bookings for hiring out the organisation’s facilities to external parties for corporate and private social events including liaison with the convention industry and other cultural bodies
• Promoting, pricing and forecasting merchandise sales
• Disseminating and distributing agency publications purchased by mail order or online
• Carrying out customer surveys to support the planning and development of customer service initiatives
• Processing reproduction requests for use of images or objects where copyright is invested in the agency
• Counting and valuing of merchandise to identify missing items and determine the condition of existing items; and
• Administrative activities such as conduct of meetings and committees, authorising and delegation, compliance, auditing and reporting""";
    skos:inScheme :conceptScheme: ;
    skos:prefLabel "Commercial Services" .

:0191  a crs:Function, ra:Class,
        skos:Concept ;
    crs:isPerformedBy [ crs:hasAgent ca:4435 ] ;
    dct:source ras:2009-00822408 ;
    skos:definition """The core business of managing permanent, temporary and travelling exhibitions of the agency’s collection throughout Australia and overseas with the aim of widening public knowledge of Australian history and historical experience developed around interrelated
thematic interests of Aboriginal and Torres Strait Islander cultures and histories, Australia’s history and society since European settlement in 1788, and the interaction of people with the environment.
Includes:
• Establishing policy to guide the development of the agency’s permanent galleries, and temporary and travelling exhibition program;
• Planning, developing and maintaining forward schedules for refreshment and renewal of gallery exhibitions;
• Developing exhibition content and design;
• Installing and demounting exhibitions;
• Constructing exhibitory and packing collection objects;
• Developing exhibition programs and services;
• Collaboration on exhibition projects with other cultural institutions and hosting buy-in exhibitions;
• Fit-outs and refurbishment of exhibition galleries and spaces;
• Administration of inwards and outwards loans of exhibition materials;
• Conducting marketing research to target potential sponsorships for exhibitions;
• Evaluation testing exhibition programs and services either prior to or during their development, and/or after an exhibition has opened;
• Consulting stakeholders;
• Contributing to relevant international debates and scholarship on exhibition-making within the field of museology;
• Exhibition research and studies on exhibition-making;
• Obtaining advice and feedback on the development of exhibition-related programs, services and resources;
• Development of concepts for exhibitions based on a specific theme;
• Joint ventures between other cultural and educational organisations and the agency;
• Assessing requests for sponsorship of exhibitions;
• Negotiating and establishing agreements;
• Project management processes and controls;
• Implementing agency and industry standards to support exhibitions;
• Reporting on the performance of exhibitions;
• Presentations made by agency staff to promote exhibitions;
• Development of procedure manuals and guidelines;
• Liaison activities with other cultural institutions, authorities and the private sector;
• Maintenance of exhibitions and display materials;
• Inspections of exhibitions against design documentation;
• Enquiries from the public about agency exhibition program and services; and
• Administrative activities such as conduct of meetings and committees, authorising and delegation, compliance, auditing and reporting.

""";
    skos:inScheme :conceptScheme: ;
    skos:prefLabel """Exhibition Management
""".

:0192  a crs:Function, ra:Class,
        skos:Concept ;
    crs:isPerformedBy [ crs:hasAgent ca:4435 ] ;
    dct:source ras:2009-00822408 ;
    skos:definition """The core business of developing and implementing programs of research in Australian history, museum studies and material culture to underpin the agency’s exhibitions, national collection, publications and other related activities.
Includes:
• Managing and developing research and scholarship projects and programs;
• Writing and editing historical manuscripts, chapters for scholarly compilations and historical interpretation reports;
• Partnering and collaborating with academic and institutional research organisations;
• Attending and hosting conferences, symposiums, forums, seminars and lectures to disseminate research initiatives and outcomes;
• Assessing applications made to the agency for research grant funding;
• Undertaking field trips to research a specific subject or area of interest in order to discover facts, principles etc;
• Managing intellectual property (copyright, royalties etc) owned by the agency;
• Maintaining informal contact with various individuals and institutions in related fields of research;
• Arranging and carrying out research guided tours with members of the public;
• Developing and implementing policies;
• Administrative activities such as conduct of meetings and committees, authorising and delegation, compliance, auditing and reporting.
""";
    skos:inScheme :conceptScheme: ;
    skos:prefLabel "Historical Research" .

:0193  a crs:Function, ra:Class,
        skos:Concept ;
    crs:isPerformedBy [ crs:hasAgent ca:4474 ] ;
    dct:source ras:2003-00258141 ;
    skos:definition "The function of managing the appointments and ongoing arrangements of Commissioners (including the Chairman).  This includes activities associated with notification of processing and payment of salaries and allowances, provision of leave entitlements, management of resignation, suspension or presented by Commissioners at external events." ;
    skos:inScheme :conceptScheme: ;
    skos:prefLabel "Commissioner Administration" .

:0194  a crs:Function, ra:Class,
        skos:Concept ;
    crs:isPerformedBy [ crs:hasAgent ca:4474 ] ;
    dct:source ras:2003-00258141 ;
    skos:definition "The function of conducting inquiries and reviews under Terms of Reference issued by the government and providing advice and recommendations. This includes research, inviting and considering submissions from the States and interested parties, taking evidence at formal hearings, conducting meeetings, engaging consultants, reviewing methodology and reporting to the Minister." ;
    skos:inScheme :conceptScheme: ;
    skos:prefLabel "Grants Inquiries" .

:0195  a crs:Function, ra:Class,
        skos:Concept ;
    crs:isPerformedBy [ crs:hasAgent ca:4485 ] ;
    dct:source ras:2003-00113511 ;
    skos:definition "The function of providing audit services to the Commonwealth to promote improvement in public sector performance and to provide independent assurance of public sector accountability. Includes audit planning; performance and assurance auditing; evaluation and monitoring; benchmarking; peer veview and audit education. Also includes audit guidance, research and representation in the Australian and international formulation and application of auditing standards and processes." ;
    skos:inScheme :conceptScheme: ;
    skos:prefLabel "Audit Services" .

:0196  a crs:Function, ra:Class,
        skos:Concept ;
    crs:isPerformedBy [ crs:hasAgent ca:5374 ] ;
    dct:source ras:2007-00268370 ;
    skos:definition """The function of administering the operations of the agency's board. Includes providing reports to the Minister and Parliament, taking of board minutes and processes involved in authorising the agency's
charter of corporate governance, corporate and business plans and audited financial statements. Also includes processing board nominations and appointments and managing board committees, arranging
board travel, accommodation and remuneration.""";
    skos:inScheme :conceptScheme: ;
    skos:prefLabel "Board Administration" .

:0197  a crs:Function, ra:Class,
        skos:Concept ;
    crs:isPerformedBy [ crs:hasAgent ca:5374 ] ;
    dct:source ras:2007-00268370 ;
    skos:definition "The function of managing the national data collections and data sets documenting health, housing and community programs and services in government and non-government sectors. Includes the activities involved in collecting and analysing data and information, complying with legal confidentiality provisions, maintaining the quality of data sets and dictionaries, obtaining opinions from external referees, and responding to requests for access to the agency's national data holdings. Also includes responding to requests for tender, providing consultancy services for which remuneration is paid, providing external training services and reporting on the outcomes of the analysis and research activities to inform community debate and public policy making." ;
    skos:inScheme :conceptScheme: ;
    skos:prefLabel "Data Collection Management" .

:0198  a crs:Function, ra:Class,
        skos:Concept ;
    crs:isPerformedBy [ crs:hasAgent ca:5374 ] ;
    dct:source ras:2007-00268370 ;
    skos:definition """The function of developing infrastructure for the collection of national health, housing and community-services related statistics from government and non-government sectors. Includes developing
specialised standards and classifications aimed to collect consistent data and information, negotiating and formalising agreements, the management of national and/or internal committees responsible for developing national performance indicators and providing support to agency projects. Also includes managing joint ventures with external bodies or persons, arranging and attending conferences, giving presentations for professional and promotional purposes, providing advice, liaison activities, and responding to public enquiries.""";
    skos:inScheme :conceptScheme: ;
    skos:prefLabel "Statistical Infrastructure Development" .

:0199  a crs:Function, ra:Class,
        skos:Concept ;
    crs:isPerformedBy [ crs:hasAgent ca:5554 ] ;
    dct:source ras:2005-00077921 ;
    skos:definition "The function of appointing and managing the advisory board, monitoring its performance and managing separations. Includes ongoing administrative activities such as arranging travel and paying travel allowances.  " ;
    skos:inScheme :conceptScheme: ;
    skos:prefLabel "Advisory Board Management" .

:0200  a crs:Function, ra:Class,
        skos:Concept ;
    crs:isPerformedBy [ crs:hasAgent ca:5554 ] ;
    dct:source ras:2005-00077921 ;
    skos:definition "The function of identifying and winning clients by researching and responding to business opportunities. Includes marketing activities such as service development, conducting market research, preparing marketing strategies, tendering to undertake work for prospective clients, contracting to deliver services to clients, coordinating public relations activities and the management of client relationships. Also includes entering partnerships with other parties to bid for work. " ;
    skos:inScheme :conceptScheme: ;
    skos:prefLabel "Business Development" .

:0201  a crs:Function, ra:Class,
        skos:Concept ;
    crs:isPerformedBy [ crs:hasAgent ca:5554 ] ;
    dct:source ras:2005-00077921 ;
    skos:definition "The function of providing legal and law-related services to Government, Commonwealth, State and Territory governments, government bodies, office holders and employees. Includes legal and related services to bodies and persons determined by the Attorney-General or the chief executive officer for any purpose for which the Commonwealth can make laws. Includes the provision of legal advice, the drafting of legislation and legal contracts, the registration of intellectual property and representing clients in dispute resolution processes such as mediation and litigation and the development, delivery and review of administrative law training to clients.  " ;
    skos:inScheme :conceptScheme: ;
    skos:prefLabel "Legal Services To Government" .

:0202  a crs:Function, ra:Class,
        skos:Concept ;
    crs:isPerformedBy [ crs:hasAgent ca:5987 ] ;
    dct:source ras:2003-00622439 ;
    skos:definition "The function of managing the activities of foundations, councils and institutes where the Department provides secretariat services. Includes the appointment and separation of board members, remuneration, board meetings, committees established by boards, and arrangements for board members to travel on board business." ;
    skos:inScheme :conceptScheme: ;
    skos:prefLabel "Board Administration" .

:0203  a crs:Function, ra:Class,
        skos:Concept ;
    crs:isPerformedBy [ crs:hasAgent ca:5987 ] ;
    dct:source ras:2003-00622439 ;
    skos:definition "The function of managing cases involving personal emergencies experienced by individual Australians travelling or residing overseas. Emergencies could include hospitalisation, robbery, arrest or death." ;
    skos:inScheme :conceptScheme: ;
    skos:prefLabel "Consular Case Management" .

:0204  a crs:Function, ra:Class,
        skos:Concept ;
    crs:isPerformedBy [ crs:hasAgent ca:5987 ] ;
    dct:source ras:2003-00622439 ;
    skos:definition "The function of assisting and protecting the interests of Australians overseas in accordance with international law. Includes handling notarial acts, co-ordination of claims for United Nations compensation, registration of Australians travelling or residing overseas, provision of travel advice, monitoring situations and co-operative consular arrangements. " ;
    skos:inScheme :conceptScheme: ;
    skos:prefLabel "Consular Services" .

:0205  a crs:Function, ra:Class,
        skos:Concept ;
    crs:isPerformedBy [ crs:hasAgent ca:5987 ] ;
    dct:source ras:2003-00622439 ;
    skos:definition "The function of providing protection and assistance to Australians and other approved nationals in the event of civil emergencies, disasters (e.g. earthquake) or acts of terrorism, requiring integrated and coordinated action by mission staff and Canberra. Includes assessing risks, developing contingency plans, maintaining the warden network system, providing advice and the convening of task forces to manage the crisis. " ;
    skos:inScheme :conceptScheme: ;
    skos:prefLabel "Crisis Management" .

:0206  a crs:Function, ra:Class,
        skos:Concept ;
    crs:isPerformedBy [ crs:hasAgent ca:5987 ] ;
    dct:source ras:2003-00622439 ;
    skos:definition "The function of managing the organisation's historical resources. Includes agreements regarding access to historical resources, conducting reference enquiries for clients, maintaining information on overseas posts and personnel, producing and maintaining guidelines outlining potential current sensitivities and the preparation for publication of scholarly volumes of diplomatic documents." ;
    skos:inScheme :conceptScheme: ;
    skos:prefLabel "Historical Records Management" .

:0207  a crs:Function, ra:Class,
        skos:Concept ;
    crs:isPerformedBy [ crs:hasAgent ca:5987 ] ;
    dct:source ras:2003-00622439 ;
    skos:definition "The function of monitoring, advising and developing strategies, agreements and policy advice in regards to international issues such as the environment, human rights and democratic principles. Includes providing financial assistance to other countries and international organisations; conducting consultations and maintaining relationships with foreign countries and international organisations; participation and support for international treaties/agreements; establishment of diplomatic posts and management of international visits to and from Australia. " ;
    skos:inScheme :conceptScheme: ;
    skos:prefLabel "International Relations" .

:0208  a crs:Function, ra:Class,
        skos:Concept ;
    crs:isPerformedBy [ crs:hasAgent ca:5987 ] ;
    dct:source ras:2003-00622439 ;
    skos:definition "The function of protecting and advancing Australia's security interests through contributions to international security. Includes providing advice, negotiating agreements, participating in conferences and defence/security exercises, undertaking consultations and outreach programs regarding security issues, and monitoring international security situations. " ;
    skos:inScheme :conceptScheme: ;
    skos:prefLabel "International Security" .

:0209  a crs:Function, ra:Class,
        skos:Concept ;
    crs:isPerformedBy [ crs:hasAgent ca:5987 ] ;
    dct:source ras:2003-00622439 ;
    skos:definition "The function of regulating and monitoring peaceful use of nuclear, chemical, biological and radiological materials and facilities. Includes implementation of obligations under various legislation, treaties, arrangements and agreements; granting permits to use, import and export materials, information and facilities; and inspections." ;
    skos:inScheme :conceptScheme: ;
    skos:prefLabel "Non Proliferation And Safeguards" .

:0210  a crs:Function, ra:Class,
        skos:Concept ;
    crs:isPerformedBy [ crs:hasAgent ca:5987 ] ;
    dct:source ras:2003-00622439 ;
    skos:definition "The function of issuing Australian travel identification documents in accordance with international standards. Includes provision of passports, documents of identity and convention travel documents and investigating suspected travel document fraud." ;
    skos:inScheme :conceptScheme: ;
    skos:prefLabel "Passport Services" .

:0211  a crs:Function, ra:Class,
        skos:Concept ;
    crs:isPerformedBy [ crs:hasAgent ca:5987 ] ;
    dct:source ras:2003-00622439 ;
    skos:definition "The function of managing employees and volunteers working overseas for the organisation and not covered by the Public Service Act. Overseas employees include locally engaged staff, house staff or heads of mission, honorary consuls and spouses and family of consular staff. " ;
    skos:inScheme :conceptScheme: ;
    skos:prefLabel "Personnel Overseas" .

:0212  a crs:Function, ra:Class,
        skos:Concept ;
    crs:isPerformedBy [ crs:hasAgent ca:5987 ] ;
    dct:source ras:2003-00622439 ;
    skos:definition "The function of providing services to the foreign diplomatic and consular community. Includes co-ordinating diplomatic accreditation, facilitating the transition of diplomats and their families into Australia and the consular community, authorisation of concessions, ensuring diplomatic privileges and immunities, processing award nominations and organising diplomatic functions." ;
    skos:inScheme :conceptScheme: ;
    skos:prefLabel "Protocol" .

:0213  a crs:Function, ra:Class,
        skos:Concept ;
    crs:isPerformedBy [ crs:hasAgent ca:5987 ] ;
    dct:source ras:2003-00622439 ;
    skos:definition "The function of projecting a positive and accurate image of Australia. Includes developing and maintaining links (such as cultural, sporting and academic) between Australia and other countries, financial assistance for projects and programs to promote awareness and understanding between Australia and other countries, identifying and responding to contentious issues concerning Australia, and facilitating visits by international media and cultural representatives. " ;
    skos:inScheme :conceptScheme: ;
    skos:prefLabel "Public Diplomacy" .

:0214  a crs:Function, ra:Class,
        skos:Concept ;
    crs:isPerformedBy [ crs:hasAgent ca:5987 ] ;
    dct:source ras:2003-00622439 ;
    skos:definition "The function of participating in international trade negotiations and overseeing the implementation of trade rules/agreements according to the international trading system. Includes participation in trade negotiation committees and conferences, and in the consultation, dispute and accession processes. Also includes providing trade negotiation policy advice and outreach services and monitoring trade negotiation activities of Australia's trading partners." ;
    skos:inScheme :conceptScheme: ;
    skos:prefLabel "Trade Negotiations" .

:0215  a crs:Function, ra:Class,
        skos:Concept ;
    crs:isPerformedBy [ crs:hasAgent ca:5987 ] ;
    dct:source ras:2003-00622439 ;
    skos:definition "The function of advancing Australian trade and investment interests through commercial diplomacy, forums, the provision of information and assistance to Australian companies, and initiatives to support and strengthen the multilateral trading system. Includes policy advice to the government and the Australian business community. " ;
    skos:inScheme :conceptScheme: ;
    skos:prefLabel "Trade Policy And Development" .

:0216  a crs:Function, ra:Class,
        skos:Concept ;
    crs:isPerformedBy [ crs:hasAgent ca:6326 ] ;
    dct:source ras:2003-00211156 ;
    skos:definition "The function of inquiring into and, where possible, conciliating complaints of alleged discrimination and breaches of human rights. Includes amicus curiae, investigation and reporting to the Federal Parliament." ;
    skos:inScheme :conceptScheme: ;
    skos:prefLabel "Complaints Handling" .

:0217  a crs:Function, ra:Class,
        skos:Concept ;
    crs:isPerformedBy [ crs:hasAgent ca:6326 ] ;
    dct:source ras:2003-00211156 ;
    skos:definition "The function of monitoring and inquiring into compliance with human rights and equal opportunity legislation administered by the agency. Includes intervention into legal proceedings, public inquiries, developing guidelines, examining acts of Parliament in order to determine whether they comply with provisions of the Universal Declaration of Human Rights, and examining any relevant international instruments that Australia is considering adopting, to identify any inconsistencies with existing human rights treaties." ;
    skos:inScheme :conceptScheme: ;
    skos:prefLabel "Human Rights Compliance" .

:0218  a crs:Function, ra:Class,
        skos:Concept ;
    crs:isPerformedBy [ crs:hasAgent ca:6326 ] ;
    dct:source ras:2003-00327877 ;
    skos:definition "The function of promoting human rights principles and the objects of human rights and equal opportunity legislation. Includes conducting education and awards programs and providing technical assistance in the establishment and delivery of human rights services, both nationally and internationally. " ;
    skos:inScheme :conceptScheme: ;
    skos:prefLabel "Public Awareness And Education" .

:0219  a crs:Function, ra:Class,
        skos:Concept ;
    crs:isPerformedBy [ crs:hasAgent ca:6669 ] ;
    dct:source ras:2009-00714202 ;
    skos:definition """The core business of establishing relationships, usually through agreements, and working with ally and partner organisations such as professional firms, chambers of commerce and industry associations, as well as federal, state and local government agencies and regional development organisations, to promote exporting of Australian products to overseas markets.  Includes commercial relationships established under the Tradestart Scheme.
The tasks associated with ally and partner management include:
• establishing, maintaining, reviewing and negotiating agreements with allies and partners to act as agents for agency and/or to promote exporting
• managing contact, including meetings, between the agency and allies and partners
• auditing the agency’s events, processes or business relating to allies and partners
• developing policies and procedures to provide guidance to the agency in its dealings with allies and partners
• all aspects of training provided to allies and partners, including developing training programs and material, and conducting and evaluating training programs
• managing compliments and complaints relating to allies and partners
• monitoring the work performances of allies and partners so that specific goals and objectives are achieved
• developing, implementing and monitoring programs relating to allies and partners
• developing internal periodic and statistical reports.""";
    skos:inScheme :conceptScheme: ;
    skos:prefLabel "Ally And Partner Management" .

:0220  a crs:Function, ra:Class,
        skos:Concept ;
    crs:isPerformedBy [ crs:hasAgent ca:6669 ] ;
    dct:source ras:2009-00714202 ;
    skos:definition """The core business of assisting potential, new and established Australian exporters (clients) to achieve export sales.
The tasks associated with client services include:
• sourcing, contacting and recruiting new clients
• managing client accounts
• negotiating, establishing and maintaining formal service agreements with clients, and joint ventures with external industry groups
• managing internal and external committees relating to client services, such as industry committees
• establishing and maintaining contact between the agency and other organisations and agencies, such as regional and industry groups and professional allies such as freighters, finance specialist, lawyers and accountants
• managing appeals against rejection of program applications, to higher authorities such as tribunals or courts
• conducting audits of operational records and activities
• assessing applications for tax exemptions from Australian companies bidding for overseas work
• answering enquiries about services available to clients
• managing complaints and compliments relating to client services
• providing and receiving advice relating to client services
• providing coaching and mentoring to new and irregular exporters
• developing and establishing policies and procedures to provide guidance to the agency in regards to client services
• reviewing operations, procedures and policies
• developing, implementing and monitoring programs to assist Australian businesses to achieve set objectives
• conducting research and evaluations to gauge agency performance and determine client expectations relating to client services
• reporting on the activities associated with client services, including statistical and periodic reports
• developing programs to assist Australian businesses access international markets and
• providing general and tailored services,including training, to assist clients achieve successful export outcomes.""";
    skos:inScheme :conceptScheme: ;
    skos:prefLabel "Client Services" .

:0221  a crs:Function, ra:Class,
        skos:Concept ;
    crs:isPerformedBy [ crs:hasAgent ca:6669 ] ;
    dct:source ras:2009-00714202 ;
    skos:definition """The core business of identifying and working with overseas companies (customers) wishing to purchase Australian products and services, to achieve international business outcomes for Australian businesses.
The tasks associated with customer management include:
• conducting audits of operations, processes or business relating to customer management
• identifying, acquiring, and maintaining contact with customers as potential purchasers of Australian products and services
• managing overseas visits and appointments by agency representatives and clients to customers
• managing visits and appointments for customers visiting Australia
• development and establishing procedures to provide guidance to the agency in regards to customer management
• reporting on the activities associated with customer management, including statistical and periodic reports
• reviewing operations, processes and procedures relating to customer management
• handling complaints and compliments received from customers.""";
    skos:inScheme :conceptScheme: ;
    skos:prefLabel "Customer Management" .

:0222  a crs:Function, ra:Class,
        skos:Concept ;
    crs:isPerformedBy [ crs:hasAgent ca:6669 ] ;
    dct:source ras:2009-00714202 ;
    skos:definition """The core business of co-ordinating or participating in international events, which provide a way for clients to promote their products and services internationally, and domestic events, which provide Australian companies with current information about international markets and also potentially involve visiting international buyers.
The tasks associated with event and visit management include:
• providing and receiving advice relating to the management of events and visits
• negotiating, establishing and maintaining agreements, including memoranda of understanding, relating to event and visit management, such as agreements with states and territories to participate in export awards
• conducting audits of operational records and activities
• planning and managing the Australian export awards process and ceremony
• managing complaints and compliments relating to event and visit management
• planning, marketing and managing domestic and off-shore events and visits, including exhibitions and missions
• developing and establishing policies and procedures to provide guidance to the agency in regards to event and visit management
• developing, implementing and monitoring programs designed to assist Australian businesses to access and secure international markets and services, such as Business Club Australia Program
• reporting on activities associated with event and visit management, and
• securing or providing sponsorship for events and evaluating and reporting on the arrangements.""";
    skos:inScheme :conceptScheme: ;
    skos:prefLabel "Event And Visit Management" .

:0223  a crs:Function, ra:Class,
        skos:Concept ;
    crs:isPerformedBy [ crs:hasAgent ca:6669 ] ;
    dct:source ras:2009-00714202 ;
    skos:definition """The core business of developing and managing financial assistance programs and schemes to assist Australian companies seeking to establish or expand overseas markets for Australian products.
The tasks associated with financial assistance include:
• establishing, maintaining, reviewing and negotiating agreements, including memorandum of understanding, with other agencies to provide services or information relating to financial services, such as Australian Customs Service who provides the agency with travel details of financial assistance applicants
• managing contact and consultations between the agency and stakeholders such as applicants, police agencies, grant consultants and allies
• providing and receiving advice and guidance relating to financial assistance
• receiving and assessing applications for financial assistance from Australian businesses
• managing appeals to higher authorities, such as tribunals and courts, against the rejection of financial assistance applications
• planning and conducting audits of the operations, processes and procedures relating to financial assistance
• developing policies and procedures to provide guidance to the agency in regards to financial assistance
• developing, conducting and evaluating training provided to external stakeholders and relating to financial assistance
• managing complaints and compliments relating to financial assistance
• investigating suspected fraudulent claims for financial assistance and taking further legal action if required
• developing formal, periodic and statistical reports relating to financial assistance
• conducting and reporting on research relating to financial assistance, such as surveys of financial assistance recipients
• reviewing operations, processes and procedures relating to financial assistance
• developing, establishing, managing and monitoring financial assistance programs and schemes
• managing internal and external committees relating to financial assistance.
•	managing internal and external committees relating to financial assistance.
""";
    skos:inScheme :conceptScheme: ;
    skos:prefLabel "Financial Assistance" .

:0224  a crs:Function, ra:Class,
        skos:Concept ;
    crs:isPerformedBy [ crs:hasAgent ca:6669 ] ;
    dct:source ras:2009-00714202 ;
    skos:definition """The core business of assisting Australian private organisations to compete for contracts with overseas development projects so as to encourage the export of Australian goods and services. All extant records at the time of issue of this Records Authority were created by the Australian Overseas Projects Corporation, abolished in 1986. It includes:
• identifying overseas development project opportunities for Australian organisations
• providing information and advice to stakeholders
• assisting in negotiations with overseas entities
• facilitating stakeholder meetings and liaison
• developing policies and procedures in relation to the agency’s involvement in overseas development projects
• entering into arrangement to jointly carry out the overseas development project""";
    skos:inScheme :conceptScheme: ;
    skos:prefLabel "International Development Projects" .

:0225  a crs:Function, ra:Class,
        skos:Concept ;
    crs:isPerformedBy [ crs:hasAgent ca:6669 ] ;
    dct:source ras:2009-00714202 ;
    skos:definition """The core business of monitoring, analysing and advising on current and future domestic and international  trends, markets, opportunities, issues and conditions relating to trade and the economy. Includes preparing country and industry profiles and establishing and managing industry networks.
The tasks associated with trade and economic analysis include:
• analysing and reporting on international trade and economic opportunities
• researching and reporting on trade and economic issues and trends
• facilitating stakeholder meetings and liaison
• contributing to the negotiations and establishment of bilateral or multilateral trade agreements
• developing industry and country economic profiles
• presentations on international trade and economic issues presented at public events
• receiving and providing advice to government and industry on trade and economic trends and issues
• participation on committees relating to trade and economy""";
    skos:inScheme :conceptScheme: ;
    skos:prefLabel "Trade And Economic Analysis" .

:0226  a crs:Function, ra:Class,
        skos:Concept ;
    crs:isPerformedBy [ crs:hasAgent ca:6679 ],
        [ crs:hasAgent ca:6679 ],
        [ crs:hasAgent ca:6679 ],
        [ crs:hasAgent ca:6679 ],
        [ crs:hasAgent ca:6679 ],
        [ crs:hasAgent ca:6679 ] ;
    dct:source ras:2001-00000625,
        ras:2004-00679116 ;
    skos:definition "The function of designing and constructing architectural and engineering works of any kind including fitouts, refurbishments and extensions and conservation of such works. Includes preparing drawings and specifications, surveying, tendering, managing and overseeing of construction activities by internal or contracted labour and liaison with clients." ;
    skos:inScheme :conceptScheme: ;
    skos:prefLabel "Capital Works" .

:0227  a crs:Function, ra:Class,
        skos:Concept ;
    crs:isPerformedBy [ crs:hasAgent ca:6679 ] ;
    dct:source ras:2004-00679116 ;
    skos:definition "The function of managing, including on a commercial basis, non-Defence-related properties and places owned by the Commonwealth within Australia, or leased by the Commonwealth. Includes managing and monitoring contract performance against cost and service standards relating to those properties, acquiring, selling, transferring, divesting or otherwise disposing of properties owned by the Commonwealth, implementing commercial leasing arrangements for all users of Commonwealth property, developing and implementing property management strategies and refining commercial arrangements for Commonwealth office buildings. Also includes matters relating to the development and application of the Commonwealth property framework, the Commonwealth construction procurement policy and matters relating to the administration of the legislation such as Public Works Act 1969." ;
    skos:inScheme :conceptScheme: ;
    skos:prefLabel "Commonwealth Property Management" .

:0228  a crs:Function, ra:Class,
        skos:Concept ;
    crs:isPerformedBy [ crs:hasAgent ca:6679 ] ;
    dct:source ras:2002-04651164 ;
    skos:definition "The function of providing independent advice to the Minister for Foreign Affairs and Trade on current and future issues relating to Australia’s overseas aid program. Includes arranging Council meetings and member travelling arrangements, formulating agendas and taking of minutes, and maintaining a record of member appointments and resignations." ;
    skos:inScheme :conceptScheme: ;
    skos:prefLabel "Overseas Aid Advice" .

:0229  a crs:Function, ra:Class,
        skos:Concept ;
    crs:isPerformedBy [ crs:hasAgent ca:6679 ] ;
    dct:source ras:2002-04650377 ;
    skos:definition "The function of developing policies and strategies to support and enhance Australia’s aid projects and programs to overseas countries. Includes identifying and assessing overseas development needs and priorities through reviews, research and investigations; and fostering links between Australian community organisations and the people of developing countries through agreements, joint ventures and visits. Also includes managing and processing funding submissions from non-government organisations for their aid development activities and providing policy advice, briefings and support to the Minister on development issues." ;
    skos:inScheme :conceptScheme: ;
    skos:prefLabel "Overseas Aid Development" .

:0230  a crs:Function, ra:Class,
        skos:Concept ;
    crs:isPerformedBy [ crs:hasAgent ca:6679 ],
        [ crs:hasAgent ca:6679 ] ;
    dct:source ras:2002-04650377,
        ras:2009-00689250 ;
    skos:definition "The function of managing the delivery of Australia’s aid programs and projects to overseas countries. Includes engaging with a range of international organisations and the private sector through the development of agreements and the undertaking of contractual arrangements, allocation of funds and monitoring and evaluating the implementation of projects and programs. Also includes managing the provision of scholarship assistance to students from developing countries." ;
    skos:inScheme :conceptScheme: ;
    skos:prefLabel "Overseas Aid Management" .

:0231  a crs:Function, ra:Class,
        skos:Concept ;
    crs:isPerformedBy [ crs:hasAgent ca:7126 ] ;
    dct:source ras:2009-00589493 ;
    skos:definition "The function of establishing and maintaining ongoing relationships with domestic agencies and international counterparts. Includes the provision of intelligence access and services to domestic agencies and the exchange of information with international counterparts to assist in the combat against money laundering, the financing of terrorism, and other major crimes. Also includes agreements with agencies and countries governing access and exchange of financial intelligence, participation in international bodies, and the provision of training and technical assistance." ;
    skos:inScheme :conceptScheme: ;
    skos:prefLabel "Domestic And International Relations" .

:0232  a crs:Function, ra:Class,
        skos:Concept ;
    crs:isPerformedBy [ crs:hasAgent ca:7126 ] ;
    dct:source ras:2009-00589493 ;
    skos:definition "The function of collecting, interpreting, analysing, and distributing intelligence information to partner agencies and international counterparts. Includes the identification and prioritisation of intelligence targets and the design and implementation of appropriate operational means to collect intelligence. Also includes the development of policies and procedures relating to intelligence programs, and the monitoring, evaluation and reviewing of these programs." ;
    skos:inScheme :conceptScheme: ;
    skos:prefLabel "Intelligence" .

:0233  a crs:Function, ra:Class,
        skos:Concept ;
    crs:isPerformedBy [ crs:hasAgent ca:7126 ] ;
    dct:source ras:2009-00589493 ;
    skos:definition "The function of collecting financial transaction reports and ensuring the regulated community complies with legislation. Includes identifying new and existing reporting entities, providing education services, and managing action relating to identified or suspected non-compliance with legislated obligations, including those defined in the Anti-Money Laundering and Counter-Terrorism Financing Act 2006. Includes investigations and actions relating to the regulated community, members of the public undertaking cross border movements of currency or carrying bearer negotiable instruments, and other persons, whether regulated or not, for events covered by the agency’s enforcement powers provided in legislation." ;
    skos:inScheme :conceptScheme: ;
    skos:prefLabel "Regulatory Compliance" .

:0234  a crs:Function, ra:Class,
        skos:Concept ;
    crs:isPerformedBy [ crs:hasAgent ca:7126 ],
        [ crs:hasAgent ca:7126 ] ;
    dct:source ras:2009-00589493 ;
    skos:definition "The function of developing, implementing, and maintenance of Australia’s anti-money laundering and counter-terrorist financing framework. Includes the setting of policy, rules, and guidelines that constitute the statutory framework and the development and management of associated legislation." ;
    skos:inScheme :conceptScheme: ;
    skos:prefLabel "Regulatory Policy" .

:0235  a crs:Function, ra:Class,
        skos:Concept ;
    crs:isPerformedBy [ crs:hasAgent ca:7235 ] ;
    dct:source ras:2007-00232293 ;
    skos:definition "The function of protecting the marine environment from pollution from ships and other environmental damage.  Includes management of a national plan to combat sea pollution, managing the national emergency towage program, coordination of training for national plan and emergency towage participants, responding to marine pollution incidents, and investigating apparent breaches of compliance with environment protection legislation.  Also includes promoting community awareness of maritime pollution through education programs." ;
    skos:inScheme :conceptScheme: ;
    skos:prefLabel "Marine Environment Protection" .

:0236  a crs:Function, ra:Class,
        skos:Concept ;
    crs:isPerformedBy [ crs:hasAgent ca:7235 ] ;
    dct:source ras:2007-00232293 ;
    skos:definition "The function of providing a national search and rescue service by detecting, locating and rescuing persons in maritime and aviation distress situations. Includes the receipt and evaluation of requests for assistance through a rescue coordination centre, coordinating responses and assessing outcomes.  Also includes administering Australia’s ship reporting system, developing education programs and providing training services." ;
    skos:inScheme :conceptScheme: ;
    skos:prefLabel "Maritime And Aviation Search And Rescue" .

:0237  a crs:Function, ra:Class,
        skos:Concept ;
    crs:isPerformedBy [ crs:hasAgent ca:7235 ] ;
    dct:source ras:2007-00232293 ;
    skos:definition "The function of developing Australia's maritime regulatory framework for maritime safety and marine environmental protection through formulating legislation such as marine orders and regulations.  Includes assessing and certification of seafarer qualifications and maritime training, and administering the licensing system for all coastal pilots.  Includes managing the Australian register of ships through activities such as registering and establishing ownership of relevant ships.  Also includes enforcing operational standards for ships in Australian waters by conducting ship inspections and marine investigations under relevant legislation." ;
    skos:inScheme :conceptScheme: ;
    skos:prefLabel "Maritime Regulation" .

:0238  a crs:Function, ra:Class,
        skos:Concept ;
    crs:isPerformedBy [ crs:hasAgent ca:7235 ] ;
    dct:source ras:2007-00232293 ;
    skos:definition """The function of promoting maritime safety by minimising the risk of shipping incidents.
Includes managing the national network of marine aids to navigation and safety communications and developing operational standards.  Also includes managing heritage issues associated with the organisation's marine aids to navigation sites and promoting a safety culture in the maritime industry through education programs.
""";
    skos:inScheme :conceptScheme: ;
    skos:prefLabel "Maritime Safety" .

:0239  a crs:Function, ra:Class,
        skos:Concept ;
    crs:isPerformedBy [ crs:hasAgent ca:7486 ] ;
    dct:source ras:2007-00204327 ;
    skos:definition "The function of managing the appointments and ongoing arrangements of board members. Includes processing and payment of salaries and allowances, provision of leave entitlements, management of separations and arrangements for travel and equipment. Also includes providing executive secretarial support to the board in the conduct of its work." ;
    skos:inScheme :conceptScheme: ;
    skos:prefLabel "Board Administration" .

:0240  a crs:Function, ra:Class,
        skos:Concept ;
    crs:isPerformedBy [ crs:hasAgent ca:7486 ] ;
    dct:source ras:2007-00204327 ;
    skos:definition """The function of managing national fisheries resources on behalf of the Australian community and key stakeholders. Includes establishing agreements with external parties, inspecting fishing vessels and
equipment, apprehending and disposing of illegal fishing vessels, and auctioning fishing rights. Also includes licensing activities, monitoring compliance, handling infringements and breaches of fisheries regulations, maintaining registers of fishing rights and training national fisheries personnel.""";
    skos:inScheme :conceptScheme: ;
    skos:prefLabel "Fisheries Resources Management" .

:0241  a crs:Function, ra:Class,
        skos:Concept ;
    crs:isPerformedBy [ crs:hasAgent ca:7605 ] ;
    dct:source ras:2005-00233013 ;
    skos:definition "The function of determining onshore and offshore boundaries. Includes preparation of technical case and supporting information to enable the submission of the outer limit of Australia's continental shelf to the United Nations Commission on the Limits of the Continental Shelf under current international laws and conventions and determining the location of Australia's Territorial Sea Baseline and other various maritime zone limits. Also includes providing advice to interested parties on cadastral issues, offshore State and Federal jurisdictions, marine resources, environment and use of the ocean issues." ;
    skos:inScheme :conceptScheme: ;
    skos:prefLabel "Boundary Determination" .

:0242  a crs:Function, ra:Class,
        skos:Concept ;
    crs:isPerformedBy [ crs:hasAgent ca:7605 ] ;
    dct:source ras:2005-00233013 ;
    skos:definition "The function of selling commercial surveying services, customised maps and data, geographic information and facilities management products, and consultancies. Includes cadastral, engineering and project surveys, and the development of products for fee paying clients." ;
    skos:inScheme :conceptScheme: ;
    skos:prefLabel "Commercial Services" .

:0243  a crs:Function, ra:Class,
        skos:Concept ;
    crs:isPerformedBy [ crs:hasAgent ca:7605 ] ;
    dct:source ras:2005-00233013 ;
    skos:definition "The function of managing all specific scientific data held in the organisation's corporate stores in all formats, including cores, samples, data received under Commonwealth legislation, currently the Petroleum (Submerged Lands) Act 1967, and spatial data which can be manipulated to form specific data sets. Includes the activities relating to the data acquired in the remote sensing program, including managing and maintaining the national archive of satellite remote sensing data; and the national archive of primary geodetic survey marks. " ;
    skos:inScheme :conceptScheme: ;
    skos:prefLabel "Data Management" .

:0244  a crs:Function, ra:Class,
        skos:Concept ;
    crs:isPerformedBy [ crs:hasAgent ca:7605 ] ;
    dct:source ras:2005-00233013 ;
    skos:definition """The function of maintaining the fundamental geodetic framework for all spatial activities in Australia and its offshore territories. To maintain this framework and ensure that it is appropriate for emerging applications, this involves monitoring the horizontal and vertical motion of the Australian landmass, contributing data to the global scientific community's effort to monitor the Earth's changing shape and motion, to provide a uniform, accurate basis for all spatial data in Australia and its offshore territories.

Includes data acquisition, geodetic computation and the provision of advice to government, industry, States, researchers, communities and international organisations.""";
    skos:inScheme :conceptScheme: ;
    skos:prefLabel "Geodetic Management" .

:0245  a crs:Function, ra:Class,
        skos:Concept ;
    crs:isPerformedBy [ crs:hasAgent ca:7605 ] ;
    dct:source ras:2005-00233013 ;
    skos:definition "The function of ongoing data collection and monitoring of geophysical and nuclear hazards and providing risk assessment information. Includes research, provision of advice and risk/hazard information to government, industry, States, researchers, communities and international aid organisations, data acquisition and analysis, media relations and joint ventures. " ;
    skos:inScheme :conceptScheme: ;
    skos:prefLabel "Geohazard Monitoring And Risk Assessment" .

:0246  a crs:Function, ra:Class,
        skos:Concept ;
    crs:isPerformedBy [ crs:hasAgent ca:7605 ] ;
    dct:source ras:2005-00233013 ;
    skos:definition "The function of establishing rapport with the community and raising and maintaining the organisation's broad profile. Includes alerting school students and teachers to the contribution of scientific research to our community, and role that the organisation plays in Australia's geoscientific development. Includes teacher development and interaction with students within the organisation's facilities. Includes marketing, advertising, media liaison, exhibitions, celebrations, official representation at functions, and participating in community activities. Also includes the handling of customer services, handling reactions to those services, customer consultation and feedback. " ;
    skos:inScheme :conceptScheme: ;
    skos:prefLabel "Geoscience Awareness" .

:0247  a crs:Function, ra:Class,
        skos:Concept ;
    crs:isPerformedBy [ crs:hasAgent ca:7605 ],
        [ crs:hasAgent ca:7605 ] ;
    dct:source ras:2005-00233013,
        ras:2008-00521423 ;
    skos:definition """The business of creating and providing geoscience information publications, irrespective of format, issued for sale or distribution internally and externally. Includes the developing of products from specification to drafting and manual or electronic production (design, layout, printers, proofs, negatives, printing etc.). Also includes the marketing, customer service, supply and sales of products by the organisation.
Includes packaged products available through the product catalogues, including vector and raster digital map data, digital elevation models, satellite image data, printed topographic and geological maps, geodetic and geological datasets. Also includes multi media publications, CD-ROM and on-line information services.""";
    skos:inScheme :conceptScheme: ;
    skos:prefLabel "Geoscience Information Products" .

:0248  a crs:Function, ra:Class,
        skos:Concept ;
    crs:isPerformedBy [ crs:hasAgent ca:7605 ] ;
    dct:source ras:2005-00233013 ;
    skos:definition "The function of conducting research on the geoscientific character of Australia's marine jurisdiction to underpin effective environmental management of the oceans and coastal areas. " ;
    skos:inScheme :conceptScheme: ;
    skos:prefLabel "Marine Zone Geoscience" .

:0249  a crs:Function, ra:Class,
        skos:Concept ;
    crs:isPerformedBy [ crs:hasAgent ca:7605 ] ;
    dct:source ras:2005-00233013 ;
    skos:definition "The function of researching, promoting and providing advice and information relating to mineral exploration and mining. Includes promotion of mineral prospectivity, science case development and presentation, industry monitoring and liaison, assessment of exploration activities, and advice to government, industry and the investment community. Also includes reporting discoveries of uranium under Commonwealth legislation, currently the Atomic Energy Act 1953." ;
    skos:inScheme :conceptScheme: ;
    skos:prefLabel "Minerals And Mining Management" .

:0250  a crs:Function, ra:Class,
        skos:Concept ;
    crs:isPerformedBy [ crs:hasAgent ca:7605 ] ;
    dct:source ras:2005-00233013 ;
    skos:definition "The function of researching, marketing and providing advice relating to petroleum exploration and development. Includes promotion of petroleum prospectivity. Includes advice under Commonwealth legislation, currently the Petroleum (Submerged Lands) Act 1967, advice on annual acreage release, advice on award and administration of permits, advice on granting of production licences, retention leases, pipeline and infrastructure licences. Also industry activity monitoring and advice to government, industry and the investment community." ;
    skos:inScheme :conceptScheme: ;
    skos:prefLabel "Petroleum Management" .

:0251  a crs:Function, ra:Class,
        skos:Concept ;
    crs:isPerformedBy [ crs:hasAgent ca:7605 ] ;
    dct:source ras:2005-00233013 ;
    skos:definition "The function of participating in activities with other organisations to foster professional research, personal development and information sharing in geoscience and the activities that support the delivery of geoscience outputs. This includes membership of associations, involvement with joint committees, providing the secretariat for committees, providing expert advice on standards committees, providing assistance with conferences, seminars and workshops and attending conferences.  " ;
    skos:inScheme :conceptScheme: ;
    skos:prefLabel "Professional Relations" .

:0252  a crs:Function, ra:Class,
        skos:Concept ;
    crs:isPerformedBy [ crs:hasAgent ca:7605 ] ;
    dct:source ras:2005-00233013 ;
    skos:definition "The function of managing mechancial, technical and electronic equipment designed specifically to support geoscientific research. Such equipment may be designed and constructed inhouse, bought, acquired or leased through collaborative arrangements with other bodies to support projects and research areas. Includes acquisiton, compliance, consultancy, design and construction, installation, joint ventures, etc. Includes equipment specifically designed to manage geoscience data and arrangements for national research facilities and seismic vessels. " ;
    skos:inScheme :conceptScheme: ;
    skos:prefLabel "Research Equipment Management" .

:0253  a crs:Function, ra:Class,
        skos:Concept ;
    crs:isPerformedBy [ crs:hasAgent ca:7605 ] ;
    dct:source ras:2005-00233013 ;
    skos:definition "The function of establishing and managing research undertaken by the organisation or in collaboration with other partners. This includes the establishment, funding, priorities, submissions for research programs, monitoring progress and the reporting associated with managing research outcomes." ;
    skos:inScheme :conceptScheme: ;
    skos:prefLabel "Research Management" .

:0254  a crs:Function, ra:Class,
        skos:Concept ;
    crs:isPerformedBy [ crs:hasAgent ca:7605 ] ;
    dct:source ras:2005-00233013 ;
    skos:definition "The function of establishing whole of government and industry-wide infrastructure for the benchmarking and referencing of land and geographic information. Includes the process of establishing policy and administrative arrangements, technical standards to support fundamental datasets facilitating and promoting the sharing of spatial data across all agencies, and improving the coordination of surveying and mapping. Also includes establishing the responsibility for revision and maintenance of spatial data standards through out all levels of government, and the community. " ;
    skos:inScheme :conceptScheme: ;
    skos:prefLabel "Spatial Data Infrastructure" .

:0255  a crs:Function, ra:Class,
        skos:Concept ;
    crs:isPerformedBy [ crs:hasAgent ca:7605 ] ;
    dct:source ras:2005-00233013 ;
    skos:definition "The function of managing the organisation's special buildings and specialised housings constructed to house geoscience specific equipment in the field which have unique or specialised design features. Includes observatories, laboratories, cold store and rock store. " ;
    skos:inScheme :conceptScheme: ;
    skos:prefLabel "Specialist Property Management" .

:0256  a crs:Function, ra:Class,
        skos:Concept ;
    crs:isPerformedBy [ crs:hasAgent ca:7842 ] ;
    dct:source ras:2002-05152314 ;
    skos:definition "The function of consulting with members of the community and their representatives on agricultural and veterinary chemical issues and the operation of the national registration scheme for agricultural and veterinary chemicals. Includes activities relating to the provision of secretariat support to consultative groups such as the community consultative committee and payment of members’ allowances and remuneration." ;
    skos:inScheme :conceptScheme: ;
    skos:prefLabel "Community Liaison" .

:0257  a crs:Function, ra:Class,
        skos:Concept ;
    crs:isPerformedBy [ crs:hasAgent ca:7842 ] ;
    dct:source ras:2002-05152314 ;
    skos:definition "The function of determining focus and strategic direction of the agency. Includes activities associated with providing secretariat support to the board of directors in the conduct of its meetings, and administrative support to board members including arranging travel and remuneration of allowances. Also includes activities associated with the delegation of authority." ;
    skos:inScheme :conceptScheme: ;
    skos:prefLabel "Corporate Governance" .

:0258  a crs:Function, ra:Class,
        skos:Concept ;
    crs:isPerformedBy [ crs:hasAgent ca:7842 ] ;
    dct:source ras:2002-05152314 ;
    skos:definition "The function of Commonwealth coordination of the evaluation of agricultural and veterinary chemical products including active constituents and the issue of clearance certificates to enable the States to proceed to registration for sale in Australia. Includes the activities of developing operational policy, setting and reviewing standards and guidelines, and liaison with industry and community groups." ;
    skos:inScheme :conceptScheme: ;
    skos:prefLabel "Product Clearance" .

:0259  a crs:Function, ra:Class,
        skos:Concept ;
    crs:isPerformedBy [ crs:hasAgent ca:7842 ] ;
    dct:source ras:2002-05152314 ;
    skos:definition "The function of registering agricultural and veterinary chemicals and products that are effective for their intended purpose and satisfy safety requirements. Includes the activities of evaluating applications, authorising products and active constituents for registration, determining maximum residue limits (MRLs), setting standards and guidelines for data required to support registration applications, liaison, and fostering international harmonisation of regulatory processes and requirements.  Also includes determining proprietary rights in registration data." ;
    skos:inScheme :conceptScheme: ;
    skos:prefLabel "Product Registration" .

:0260  a crs:Function, ra:Class,
        skos:Concept ;
    crs:isPerformedBy [ crs:hasAgent ca:7842 ] ;
    dct:source ras:2002-05152314 ;
    skos:definition "The function of achieving compliance with legislation and relevant standards through product review, quality assurance, enforcement programs and licensing activities. Includes the activities which ensure chemicals meet contemporary standards through licensing of manufacturers, monitoring of adverse reactions and periodic review of chemicals of concern. Also includes control of distribution of hormonal growth promotants." ;
    skos:inScheme :conceptScheme: ;
    skos:prefLabel "Quality Assurance" .

:0261  a crs:Function, ra:Class,
        skos:Concept ;
    crs:isPerformedBy [ crs:hasAgent ca:7842 ] ;
    dct:source ras:2002-05152314 ;
    skos:definition "The function of administering the operation of the national registration scheme for agricultural and veterinary chemicals. Includes activities which facilitate collaborative arrangements between scheme participants (States and Territories) and industry, such as putting into place formal agreements and providing secretariat support to committees supporting collaborations." ;
    skos:inScheme :conceptScheme: ;
    skos:prefLabel "Scheme Administration" .

:0262  a crs:Function, ra:Class,
        skos:Concept ;
    crs:isPerformedBy [ crs:hasAgent ca:7919 ] ;
    dct:source ras:2009-00106625 ;
    skos:definition """The core business of developing and managing the national maritime collection which has the focus areas of indigenous communities, exploration and European settlement, convicts, migrants and refugees, Australian naval history, shipping and trade, environment and industry, maritime technology, maritime archaeology, sport and lifestyle, and Australian/American maritime experience.  Also includes the management of other material, such as historical vessels, large objects and replicas, related to the maritime focus of the organisation.

Processes associated with this core business include:
• acquiring historical material through purchase (from private individuals, dealers, at auction), donation/bequest, gift as part of the Commonwealth Cultural Gifts Program or equivalent, field surveys, or as a transfer of assets from other Commonwealth, state and local government agencies
• researching, registering and documenting details of the material
• conserving and restoring historical material
• de-accessioning and disposing of historical material that is no longer required
• obtaining licences, permits, approvals and certification to undertake particular action, such as holding and discharging firearms
• providing loans of the material to other organisations
• developing policies and procedures for the management of the collection and other historical material
• taking inventory and valuing collection objects and other historical material.""";
    skos:inScheme :conceptScheme: ;
    skos:prefLabel "Collection Management" .

:0263  a crs:Function, ra:Class,
        skos:Concept ;
    crs:isPerformedBy [ crs:hasAgent ca:7919 ] ;
    dct:source ras:2009-00106625 ;
    skos:definition """The core business of promoting the activities undertaken by the Museum, seeking and receiving sponsorship and donations and undertaking business activities for a commercial purpose. Includes:
• promoting exhibitions, events and public programs
• arranging sponsorship of events and activities conducted by the organisation
• receiving public financial donations in support of core functions
• development and retail sales of merchandise through the store
• managing food and beverage services that are provided through the organisation’s café and kiosk
outlets
• venue hire and catering in relation to the use of the organisation’s premises for short-term purposes,
such as weddings and parties
• visitor ticketing
• managing visitor services feedback
• undertaking market research
• providing statistical reports in relation to commercial activities, such as sales
• undertaking and participating in activities with other organisations to encourage tourism and broad
commercial improvements for the area
• establishing and operating commercial business entities.""";
    skos:inScheme :conceptScheme: ;
    skos:prefLabel "Commerical Services" .

:0264  a crs:Function, ra:Class,
        skos:Concept ;
    crs:isPerformedBy [ crs:hasAgent ca:7919 ] ;
    dct:source ras:2009-00106625 ;
    skos:definition """The core business of managing and delivering cultural and associated programs that draw upon material in the national maritime collection or otherwise in the possession of the Museum, and that disseminate
information about Australian maritime history to the public and maritime heritage stakeholders. Includes:
• managing core gallery, traveling and temporary exhibitions by means such as production scheduling,
budgeting, preparation of exhibition content lists, label texts, exhibition design and construction, liaison and receipt of loans from external sources of material for exhibition and/or design elements, agreements for terms of loan, arranging secure transportation of material, assessment, conservation/treatment and reporting on the condition of material for exhibition, preparation
commissioning, development of audiovisual and interactive content and negotiating copyright arrangements
• developing, receiving submissions, and approving concepts for exhibitions, major events, and commemorations, including those that take place exclusively online
• securing grants and other funds, excluding sponsorships, and entering into agreements with external sources in relation to cultural programs
• supporting exhibitions and major events by providing adult, school, family and infant education programs, visitor events and the members program
• providing ongoing adult, school, family, infant and member education programs and visitor events that are not linked to specific exhibitions/events
• promoting and assisting with the development of maritime heritage through involvement in assistance programs, such as the Maritime Museums of Australia Project Support Scheme (MMAPSS)
• managing and facilitating access to information about surviving vessels of significance to Australia's maritime heritage, including details of historic boats, their designers, builders and owners, through programs such as the Australian Register of Historical Vessels
• managing commemorative programs, such as the Welcome Wall
• operating historical vessels and replicas, such as the HMB Endeavour
• conducting and assisting with research into matters relating to Australian maritime history, including the scientific study of underwater cultural heritage and related land-based sites, and providing expert advice and assistance to designated Australian government and overseas agencies with site management, assessment, documentation, conservation and interpretation through programs such as the Maritime Archaeology Program
• managing professional relations and providing submissions concerning the organisation’s core business, programs and role as a collecting and cultural institution.""";
    skos:inScheme :conceptScheme: ;
    skos:prefLabel "Program Management" .

:0265  a crs:Function, ra:Class,
        skos:Concept ;
    crs:isPerformedBy [ crs:hasAgent ca:8058 ] ;
    dct:source ras:2006-00408296 ;
    skos:definition "The function of administering the activities of the organisation's board. Includes authorising the funding of fisheries research and development projects, providing advice and conducting board meetings." ;
    skos:inScheme :conceptScheme: ;
    skos:prefLabel "Board Administration" .

:0266  a crs:Function, ra:Class,
        skos:Concept ;
    crs:isPerformedBy [ crs:hasAgent ca:8058 ] ;
    dct:source ras:2006-00408296 ;
    skos:definition "The function of managing fisheries research and development throughout Australia. Includes the activities of planning to achieve outcomes and benefits for stakeholders, negotiating and establishing agreements with research providers, and liaising with stakeholders through fisheries research advisory bodies. Also includes evaluating research and development applications from research providers, issuing, receiving and assessing tenders, and managing the performance of external service provider(s)." ;
    skos:inScheme :conceptScheme: ;
    skos:prefLabel "Fisheries Research And Development Management" .

:0267  a crs:Function, ra:Class,
        skos:Concept ;
    crs:isPerformedBy [ crs:hasAgent ca:8137 ] ;
    dct:source ras:2002-05214604 ;
    skos:definition "The function of determining the objectives, strategies and policies of the organisation and undertaking activities to ensure that the organisation carries out its functions properly, efficiently and effectively. Includes activities associated with providing secretariat support to the Board in the conduct of its work and administrative support to Board members including arranging travel and remunerations for duties performed." ;
    skos:inScheme :conceptScheme: ;
    skos:prefLabel "Corporate Governance" .

:0268  a crs:Function, ra:Class,
        skos:Concept ;
    crs:isPerformedBy [ crs:hasAgent ca:8137 ] ;
    dct:source ras:2002-05214604 ;
    skos:definition "The function of issuing and renewing licences, approvals, certificates, registrations, authorisations and permissions to enable participation in aviation activities or the aviation industry. Includes entry and exit management." ;
    skos:inScheme :conceptScheme: ;
    skos:prefLabel "Entry Control" .

:0269  a crs:Function, ra:Class,
        skos:Concept ;
    crs:isPerformedBy [ crs:hasAgent ca:8137 ] ;
    dct:source ras:2002-05214604 ;
    skos:definition "The function of coordinating international activities of the agency and coordinating Australia’s position on matters considered by international civil aviation organisations. Includes liaison with overseas organisations and assessing overseas developments" ;
    skos:inScheme :conceptScheme: ;
    skos:prefLabel "International Relations" .

:0270  a crs:Function, ra:Class,
        skos:Concept ;
    crs:isPerformedBy [ crs:hasAgent ca:8137 ] ;
    dct:source ras:2002-05214604 ;
    skos:definition "The function of ensuring people, aircraft, industry, facilities, etc. comply with aviation regulations and standards through surveillance activities. Includes the handling of complaints in regards to aviation related activities or issues, investigations into alleged incidents or accidents, notification of aerodrome hazards and obstructions. Also includes ensuring compliance with building control regulations and controlling activities that could affect aviation safety." ;
    skos:inScheme :conceptScheme: ;
    skos:prefLabel "Safety Compliance" .

:0271  a crs:Function, ra:Class,
        skos:Concept ;
    crs:isPerformedBy [ crs:hasAgent ca:8137 ] ;
    dct:source ras:2002-05214604 ;
    skos:definition "The function of promoting safety awareness to the public and industry to encourage a greater acceptance of its obligations to maintain high safety standards. Also includes research into aviation safety issues, monitoring aviation industry activities and collecting, analysing and evaluating information to develop strategies to prevent risks." ;
    skos:inScheme :conceptScheme: ;
    skos:prefLabel "Safety Promotion " .

:0272  a crs:Function, ra:Class,
        skos:Concept ;
    crs:isPerformedBy [ crs:hasAgent ca:8137 ] ;
    dct:source ras:2002-05214604 ;
    skos:definition "The function of developing legislative instruments. Includes developing aviation standards, regulations, civil aviation orders, rules and procedures to define aviation safety requirements. Also includes the publication and promulgation of legislative instruments and guidance material. Excludes the processes involved in supporting the passage of the agency's legislation through Parliament." ;
    skos:inScheme :conceptScheme: ;
    skos:prefLabel "Standards Development" .

:0273  a crs:Function, ra:Class,
        skos:Concept ;
    crs:isPerformedBy [ crs:hasAgent ca:8138 ] ;
    dct:source ras:2009-00546397 ;
    skos:definition """The core business of managing air traffic in airspace, or operating on the manoeuvring area of an aerodrome, to prevent aircraft collisions, maintain an orderly flow of air traffic, provide advice and information useful for the safe and efficient conduct of flights and notify organisations regarding aircraft in need of search and rescue aid. The associated tasks include:
• the negotiation, establishment, maintenance and review of agreements such as memoranda of understanding for regional cooperation on air traffic operations and agreements for the exchange of information;
• the planning and conduct of internal and external audits;
• seeking approval from the regulatory authority to provide or make changes to air traffic services;
• providing commercial air traffic services to external clients;
• management of internal and external committees and task forces;
• complying with legislative, regulatory and voluntary standards or requirements;
• planning and conducting exercises and drills to test the proficiency of the air traffic management system and personnel;
• the reporting and investigation of aviation related incidents;
• liaison and meetings with stakeholders;
• managing operational information necessary for the safe and efficient movement of air traffic;
• recording operational communications, navigation, surveillance and flight data;
• developing plans such as air traffic control strategic plans and airport long term operating plans;
• developing and reviewing policies and procedures, guidelines and instructions;
• the planning and management of projects;
• the development of internal and external reports;
• the development and implementation of industry or agency standards.""";
    skos:inScheme :conceptScheme: ;
    skos:prefLabel "Air Traffic Management" .

:0274  a crs:Function, ra:Class,
        skos:Concept ;
    crs:isPerformedBy [ crs:hasAgent ca:8138 ] ;
    dct:source ras:2009-00546397 ;
    skos:definition """The core business of establishing and maintaining relationships with aviation industry stakeholders (such as other national and international civil aviation authorities and organisations, representative groups and airport owners) in order to share information and consult on aviation issues and advances in aviation technology, global aviation safety standards, and similar matters. The tasks associated with aviation industry relations include:
• the negotiation, establishment, maintenance and review of agreements, such as cooperative arrangements and agreements for the exchange of information;
• the management of internal and external committees and task forces;
• arranging or attending conferences relating to the aviation industry;
• presenting at aviation industry related events;
• assistance provided to participants in the aviation and aerospace industry to develop and market products or services;
• consultations, meetings and liaison with aviation industry stakeholders regarding aviation industry issues;
• developing plans such as strategic regional plans relating to the aviation industry;
• the planning and management of projects relating to aviation industry relations;
• the conduct of general research into aviation industry issues;
• providing comments and feedback to external agencies developing standards relating to the aviation industry;
• the receipt of industry awards for the agency’s outstanding achievements.""";
    skos:inScheme :conceptScheme: ;
    skos:prefLabel "Aviation Industry Relations" .

:0275  a crs:Function, ra:Class,
        skos:Concept ;
    crs:isPerformedBy [ crs:hasAgent ca:8138 ] ;
    dct:source ras:2009-00546397 ;
    skos:definition """The core business of prospecting and identifying commercial business opportunities for the agency to provide services, such as air traffic management, to external domestic and international stakeholders. Includes facilitating regional engagement and business collaboration with air navigation service providers to improve safety, efficiency, services and technologies. The tasks associated with business development include:
• speeches and addresses presented to support business development activities;
• the negotiation, establishment, maintenance and review of agreements, such as memoranda of understanding with external agencies or organisations relating to commercial or strategic business alliances;
• identifying business opportunities;
• bidding and negotiating for the agency to provide commercial services to other organisations or governments;
• the management of internal and external committees and task forces;
• liaison and meetings with stakeholders;
• marketing the agency’s commercial services and activities;
• the development of internal reports;
• the planning and management of projects.""";
    skos:inScheme :conceptScheme: ;
    skos:prefLabel "Business Development" .

:0276  a crs:Function, ra:Class,
        skos:Concept ;
    crs:isPerformedBy [ crs:hasAgent ca:8138 ] ;
    dct:source ras:2009-00546397 ;
    skos:definition """The core business of protecting the environment from the effects of or effects associated with the aviation industry. Includes, reducing the organisation's environmental footprint by minimising the impact of operations with respect to greenhouse gas emissions, energy and water use, heritage, biodiversity, resource usage and waste generation, and reviewing airport development plans and development activities. The associated tasks include:
• the negotiation, establishment, maintenance and review of agreements, such as memoranda of understanding with external agencies or organisations for sharing or accessing information;
• the planning and conduct of internal and external audits, including environmental and noise abatement audits;
• the management of certificates and permits such as aircraft noise certificates;
• the management of and participation in internal and external committees and task forces, and supporting international initiatives;
• the management of complaints and enquiries relating to environmental matters such as wake turbulence and aircraft noise;
• the management of compliance with legislative, regulatory and voluntary standards or requirements;
• Environmental Management System development, maintenance, implementation and certification;
• providing commercial environmental management services to clients;
• the conduct of environmental assessments;
• the reporting and investigation of environmental incidents;
• liaison and meetings with stakeholders;
• monitoring environmental compliance relating to aircraft noise and flight paths, including by Ministerial Direction;
• developing plans such as environmental management plans and strategies;
• developing and reviewing policies and procedures, guidelines and instructions;
• reviews and appeals against agency decisions;
• the planning and management of projects;
• the development of internal and external reports;
• the conduct of research;
• the development and implementation of industry or agency standards;
• the development and implementation of environmental awareness and communication programs.""";
    skos:inScheme :conceptScheme: ;
    skos:prefLabel "Environmental Management" .

:0277  a crs:Function, ra:Class,
        skos:Concept ;
    crs:isPerformedBy [ crs:hasAgent ca:8138 ] ;
    dct:source ras:2009-00546397 ;
    skos:definition """The core business of managing statutory determination charges for the provision of services and facilities to aviation operators.  It includes the right for the agency to impose a statutory lien on aircraft where charges are not paid by the due date, and if the debt remains unpaid, to seize and sell aircraft.  The associated tasks include:
• maintaining a register of statutory liens
• seizure and sale of aircraft
• managing reviews of agency decisions.""";
    skos:inScheme :conceptScheme: ;
    skos:prefLabel "Financial Management (Statutory Liens)" .

:0278  a crs:Function, ra:Class,
        skos:Concept ;
    crs:isPerformedBy [ crs:hasAgent ca:8138 ] ;
    dct:source ras:2009-00546397 ;
    skos:definition """The core business of managing the agency’s operational infrastructure. Includes purpose-built maintenance buildings, fire stations, radar towers and air traffic control towers. The associated tasks include:
• the design, maintenance and decommissioning of operational infrastructure
• the negotiation, establishment, maintenance and review of agreements such as agreements or memoranda of understanding for the development and management of infrastructure
• seeking and managing approvals from the regulatory authority to make changes to operational infrastructure
• the management of internal and external committees
• developing plans for operational infrastructure
• the planning and management of projects.""";
    skos:inScheme :conceptScheme: ;
    skos:prefLabel "Operational Infrastructure" .

:0279  a crs:Function, ra:Class,
        skos:Concept ;
    crs:isPerformedBy [ crs:hasAgent ca:8138 ] ;
    dct:source ras:2009-00546397 ;
    skos:definition """The core business of managing operational systems and equipment, including navigation, communication and surveillance equipment and the air traffic management system (CNS/ATM) which assists in the management of air traffic, and specialised equipment used by rescue and fire fighting personnel. The associated tasks include:
• the provision of commercial services relating to the management of navigation, communication and surveillance equipment to external stakeholders;
• the provision of advice relating to service interruptions;
• the negotiation, establishment, maintenance and review of agreements such as interface agreements or memoranda of understanding for the sharing of information;
• the planning and conduct of internal and external audits;
• seeking and managing approvals from the regulatory authority to make changes to operational equipment and systems;
• the management of internal and external committees;
• the planning and conduct of flight inspections to test accuracy and performance of operational equipment;
• liaison and meetings with stakeholders;
• the design, installation, testing, commissioning, routine operation, maintenance, modification, repair and decommissioning of operational equipment and systems;
• help desk operations;
• developing plans such as facility maintenance plans;
• developing and reviewing policies, procedures, guidelines, and instructions;
• the planning and management of projects;
• the development of internal and external reports;
• the management of research relating to operational equipment and systems;
• security arrangements for operational equipment and systems;
• the development and implementation of industry or agency standards;
• reference and technical information.""";
    skos:inScheme :conceptScheme: ;
    skos:prefLabel "Operational Systems & Equipment" .

:0280  a crs:Function, ra:Class,
        skos:Concept ;
    crs:isPerformedBy [ crs:hasAgent ca:8138 ] ;
    dct:source ras:2009-00546397 ;
    skos:definition """The core business of planning, providing, managing and evaluating training in specialised operational aspects of the organisation, such as air traffic movement and rescue and fire fighting, and training in the use and maintenance of operational equipment and systems, and maintaining records of qualifications and competencies. Includes nationally accredited training and authorised training at training colleges and on the job training. The associated tasks include:
• the provision and receipt of advice to regulatory authorities relating to operational training;
• the negotiation, establishment, maintenance and review of training agreements;
• the management of internal and external committees and task forces;
• developing plans such as strategic operational training plans;
• arrangements for the delivery of operational training programs;
• assessing student competencies through examinations, tests and exercises and maintaining records of the assessments, including recognition of prior learning/current competency assessments;
• the planning and conduct of internal and external audits relating to operational training;
• seeking approval from regulatory authorities to provide operational training;
• managing clients’ training requirements;
• the process of accrediting the agency’s training college as a recognised training organisation;
• the design, development, delivery and maintenance of the curricula and syllabi;
• the licensing, certification and monitoring of personnel to perform specialised aviation-related work;
• developing and reviewing policies, procedures, guidelines and instruction relating to operational training;
• the development of internal and external reports;
• the development and implementation of industry or agency standards;
• the planning and management of projects;
• addresses presented to promote operational training;
• recording and maintaining case files of personnel’s operational training history.""";
    skos:inScheme :conceptScheme: ;
    skos:prefLabel "Operational Training" .

:0281  a crs:Function, ra:Class,
        skos:Concept ;
    crs:isPerformedBy [ crs:hasAgent ca:8138 ] ;
    dct:source ras:2009-00546397 ;
    skos:definition """The core business of providing rescue and fire fighting services to the aviation industry at specified locations and to established standards. The associated tasks include:
• the negotiation, establishment, maintenance and review of agreements, such as for the provision of services;
• the planning and conduct of internal and external audits;
• the process of seeking approval to provide rescue and fire fighting services to specific aerodromes;
• the management of internal and external committees;
• providing commercial rescue and fire fighting services to external clients;
• planning and conducting exercises and drills to test the proficiency of the rescue and fire fighting systems and personnel;
• the reporting and investigation of aviation, fire or hazard incidents;
• the conduct of fire safety inspections of buildings to ensure compliance with agreed standards;
• liaison and meetings with stakeholders;
• managing operational notifications of new or changed services, procedures or hazards;
• recording communications in the course of rescue and fire fighting operations;
• developing plans, such as airport contingency plans and tactical plans relating to rescue and fire fighting services;
• developing and reviewing policies, procedures, guidelines and instructions;
• the planning and management of projects;
• the development of internal and external reports;
• the development and implementation of industry or agency standards.""";
    skos:inScheme :conceptScheme: ;
    skos:prefLabel "Rescue & Fire Fighting Services" .

:0282  a crs:Function, ra:Class,
        skos:Concept ;
    crs:isPerformedBy [ crs:hasAgent ca:8138 ] ;
    dct:source ras:2009-00546397 ;
    skos:definition """The core business of managing the organisation’s safety resources, systems and processes. Includes safety audits and reviews, safety approval processes and procedures, and safety documentation and reporting systems. Excludes occupational health. The associated tasks include:
• maintaining a Safety Management System (SMS) in accordance with civil aviation safety regulations;
• the negotiation, establishment, maintenance and review of agreements, such as agreements with airport operators to monitor airport safety;
• the planning and conduct of internal and external audits;
• complying with legislative, regulatory and voluntary standards or requirements;
• the evaluation of safety management programs and services;
• the reporting and investigation of safety-related incidents;
• advising, liaising and meetings with stakeholders;
• developing plans, such as disaster plans;
• developing and reviewing policies, procedures, guidelines and instructions;
• the development of internal and external reports;
• the identification and management of risks relating to operational functions of the agency;
• the development and implementation of industry or agency standards.""";
    skos:inScheme :conceptScheme: ;
    skos:prefLabel "Safety Management" .

:0283  a crs:Function, ra:Class,
        skos:Concept ;
    crs:isPerformedBy [ crs:hasAgent ca:8138 ] ;
    dct:source ras:2009-00546397 ;
    skos:definition """The core business of managing regulatory matters relating to the establishment and maintenance of the agency’s corporate entities.  The tasks include:
• Establishing and winding-up corporate entities;
• Developing an entity’s Memorandum and Articles of Association (bylaws) and corporate seal;
• Registration, certification and licensing of corporate entities.""";
    skos:inScheme :conceptScheme: ;
    skos:prefLabel "Strategic Management (Corporate Entities)" .

:0284  a crs:Function, ra:Class,
        skos:Concept ;
    crs:isPerformedBy [ crs:hasAgent ca:8155 ] ;
    dct:source ras:2009-00121658 ;
    skos:definition """The processing of future act application cases under native title legislation. Future acts are acts done in relation to land and/or waters that either validly affect native title rights and interests or are invalid because of native title.
The future act process managed by the Tribunal generally allows native title claimants and project proponents to negotiate an agreement in relation to the doing of certain future acts (mining and petroleum tenement grants and some compulsory acquisitions).  Future act applications may be resolved through mediation between the parties in those cases where the claimant has the right to negotiate under native title legislation. Where mediation is not successful, one or more of the parties may apply to have the matter arbitrated by the Tribunal. The Tribunal will determine whether the act should or should not be done and, if done, under what conditions.

The tasks associated with this function include;
• receiving future act applications and allocating resources;
• assessing requests and providing assistance in the preparation of applications (including assistance pre lodgement);
• notifying negotiation parties when a future act application has been lodged;
• undertaking preliminary assessments of applications and advising parties of the assessment outcome;
• assessing whether a native title party has the right to negotiate;
• providing geospatial analysis and research assistance to parties and internal stakeholders in respect to applications (including s 29 notices);
• monitoring progress of applications;
• providing mediation services to support future act negotiations (including conferences and hearings under s 31(1)(b), s 31 (3) and s 150);
• providing legal services support;
• conducting inquiries (arbitration) and making determinations, where parties cannot reach agreement (e.g. under s 35);
• formally notifying parties, stakeholders and the general public of the outcome of the application process;
• providing feedback to parties on the application process;
• receiving and recording Agreements; (e.g. under s 31(1)(b) and s 41A); and
• finalising applications by means other than reaching agreement or arbitration (i.e. invalid applications, lack of jurisdiction to deal with applications etc).

Excludes future act negotiations handled at the State and Territory level and reviews of Tribunal determinations considered by the Federal Court.""";
    skos:inScheme :conceptScheme: ;
    skos:prefLabel "Future Act Application Management" .

:0285  a crs:Function, ra:Class,
        skos:Concept ;
    crs:isPerformedBy [ crs:hasAgent ca:8155 ] ;
    dct:source ras:2009-00121658 ;
    skos:definition """The processes associated with providing support and assistance for developing indigenous land use agreements (ILUAs) and processing applications for the registration of such agreements in accordance with native title legislation.

ILUAs are agreements about the use and management of land and waters made between parties who hold, or claim to hold, native title in an area and other parties who have, or wish to gain, an interest in that area. If the parties agree, they may seek to register an agreement in accordance with native title legislation, at which point the terms of the ILUA become binding on all parties (if not already bound) and all the people who hold native title in relation to the agreement area, regardless of whether or not they are a party to the agreement.

An ILUA may be developed as part of the settlement of a native title determination application or it may be developed on a separate native title related issue or issues. ILUAs may be negotiated before or, if native title is found to exist after a determination of native title.

The tasks associated with ILUA application management include:
• providing pre-lodgement information and assistance;
• receiving and processing applications for mediation assistance from parties who wish to negotiate an ILUA;
• providing technical information and assistance with agreement negotiations, including mediation services, facilitation and chairing of meetings, and project management services;
• providing geospatial analysis, background research and mapping services;
• providing legal services support;
• reviewing agreements that have been lodged and testing them to ensure compliance with relevant native title legislation and eligibility for registration;
• providing feedback on draft agreements and supporting documents prior to lodgement;
• notifying interested parties/prescribed persons and the general public of the application to register the ILUA;
• processing any objections or bars to the registration of the ILUA including holding a Tribunal inquiry into whether or not it would be fair and reasonable to register an alternative procedure agreement; and
• deciding whether or not the ILUA should be registered (including registration minutes).""";
    skos:inScheme :conceptScheme: ;
    skos:prefLabel "Indigenous Land Use Agreement (Ilua) Application Management" .

:0286  a crs:Function, ra:Class,
        skos:Concept ;
    crs:isPerformedBy [ crs:hasAgent ca:8155 ] ;
    dct:source ras:2009-00121658 ;
    skos:definition """The processing of Native Title Determination Applications (NTDA) in accordance with native title legislation.

Native title describes the rights and interests of Aboriginal and Torres Strait Islander people in land and waters, according to their traditional laws and customs, which are recognised under Australian law. A native title determination is a decision by a court or recognised State or Territory body that native title does or does not exist in an area of land or sea. Where the existence of native title is recognised the determination identifies the native title holders and describes their native title rights and interests.

There are four kinds of applications under native title legislation: a ‘claimant’ application made by Indigenous Australians seeking a determination recognising that native title exists; a ‘non claimant’ application, where a non Indigenous person seeks a determination that native title does not exist; an application to revise or revoke an existing determination; and, an application for compensation for loss or impairment of native title.

The tasks associated with NTDA management include:
• receiving and assessing requests from interested parties for assistance in preparing applications, and if warranted providing such assistance;
• receiving referrals of NTDAs for mediation i.e. case referrals from the courts, or other recognised State and Territory bodies and allocating resources to these mediations;
• notifying interested parties and the general public of the NTDA and giving them an opportunity to be joined as a party to the proceedings;
• considering new and amended applications for registration and advising parties and the Federal Court of the outcome;
• providing geospatial analysis and historical, linguistic and anthropological research assistance to parties and internal stakeholders;
• providing mediation services to support the resolution of NTDAs;
• providing legal services support;
• monitoring the progress of NTDA mediation and providing the Federal Court with periodic progress reports including making recommendations to the Court about actions that the Court should consider ordering;
• referral of questions of fact or law to the courts;
• conducting a review on the existence of native title rights and interests;
• conducting an inquiry in relation to matters or issues relevant to the determination of native title;
• formally notifying relevant people and organisations of the outcome of the registration process;
• reporting to the Federal Court in relation to applications, including advising the court of those matters in which agreement cannot be reached; and
• where outcomes are appealed, providing the necessary documents and assistance to the court of review.""";
    skos:inScheme :conceptScheme: ;
    skos:prefLabel "Native Title Determination Application Management" .

:0287  a crs:Function, ra:Class,
        skos:Concept ;
    crs:isPerformedBy [ crs:hasAgent ca:8155 ] ;
    dct:source ras:2009-00121658 ;
    skos:definition """The processes related to establishing, maintaining and updating statutory registers in accordance with native title legislation and other registers as required in respect to native title. Includes matters relating to the robustness and authenticity of the registers and ensuring registry entries endure over time.

The tasks associated with register management include:
• establishing, maintaining and updating registers;
• establishing and maintaining adequate security and quality control processes to ensure the accuracy, integrity and reliability of register content;
• ensuring compliance with native title legislation;
• providing access to registers for internal and external stakeholders and creating register extracts;
• receiving and providing advice in relation to the administration and operation of registers and reporting to internal and external stakeholders;
• establishing and managing internal committees relating to register management;
• negotiating agreements and contracts relating to register management;
• developing and implementing policies, procedures and plans for the administration and operation of registers;
• maintaining statutory register content, such as registering agreements, consolidated records of updates and amendments to content; and
• periodically auditing and reviewing the administration and operation of registers. """;
    skos:inScheme :conceptScheme: ;
    skos:prefLabel "Register Management" .

:0288  a crs:Function, ra:Class,
        skos:Concept ;
    crs:isPerformedBy [ crs:hasAgent ca:8155 ] ;
    dct:source ras:2009-00121658 ;
    skos:definition """The processes associated with supporting and facilitating the effective and efficient conduct of the agency’s core business activities and responsibilities as outlined under native title legislation, including the provision of support for the management and processing of native title determination applications, future act applications and indigenous land use agreement (ILUA) applications.

The tasks associated with supporting service delivery management include:
• receiving and providing general information on native title processes (where the request does not relate to a specific application case), liaising with other bodies, and undertaking media monitoring and environmental scanning;
• marketing and promoting agency services, through seminars, workshops, conferences and the production of guidelines, brochures and other publications;
• advertising notifications in accordance with native title legislation and managing the agency’s relationship with the media;
• conducting training courses and workshops for parties to native title applications;
• arranging and attending celebrations/ceremonies/events (e.g. celebrations of claim outcomes);
• arranging travel and accommodation for agency staff;
• establishing and managing committees to oversight service delivery management;
• developing and implementing policies, procedures and plans and change management and risk management programs;
• managing application case load flows and ensuring appropriate allocation of resources are allocated to support them (e.g. National Case Flow Management Scheme);
• establishing and maintaining agreements to support service delivery, including joint-venture and inter-governmental agreements;
• researching matters relating to native title (e.g. cultural and regional indigenous matters, practices in respect to native title in other jurisdictions), not specific to any one case;
• providing historical, anthropological and linguistic research, and geospatial analysis undertaken in relation to specific application cases;
• reporting to internal and external stakeholders, including the courts, the portfolio Department and the Minister; and
• monitoring, evaluating, auditing and periodically reviewing service delivery programs and operations.
Excludes the processing of individual native title determination applications, future act applications and indigenous land use agreement (ILUA) applications, and the management of registers in accordance with native title legislation.""";
    skos:inScheme :conceptScheme: ;
    skos:prefLabel "Service Delivery Management" .

:0289  a crs:Function, ra:Class,
        skos:Concept ;
    crs:isPerformedBy [ crs:hasAgent ca:8155 ] ;
    dct:source ras:2009-00121658 ;
    skos:definition """The processes associated with establishing and managing the administration and operations of the Tribunal, including the appointment of the President, the Registrar and Members of the Tribunal. Members of the Tribunal are appointed by the Governor General under native title legislation. The Governor General also appoints a President as head of the Tribunal.

The tasks associated with the management of individual Members of the Tribunal include:
• establishment and composition of Tribunal membership, including  appointments, agreements, conditions and separations; and
• administering remuneration and allowances, leave, disclosures of interest, training and professional development and travel and accommodation.
The Tribunal performs valuable roles in relation to native title claim mediation, indigenous land use agreement negotiations and future act mediations, hearings and processes, as well as providing information to parties involved in the native title process.
The tasks associated with the establishment, administration and operation of the Tribunal include:
• development and implementation of policies, procedures and plans;
• receiving or providing advice, liaising with and visiting other bodies, and delivering addresses and presentations;
• meetings and provision of secretariat support; and
• monitoring, auditing, reviewing and reporting on Tribunal administration and operations.
Excludes matters in respect to the Members’ activities in relation to specific native title claims or cases. """;
    skos:inScheme :conceptScheme: ;
    skos:prefLabel "Tribunal President And Member Management" .

:0290  a crs:Function, ra:Class,
        skos:Concept ;
    crs:isPerformedBy [ crs:hasAgent ca:8199 ],
        [ crs:hasAgent ca:8199 ],
        [ crs:hasAgent ca:8199 ] ;
    dct:source ras:2003-00349230,
        ras:2007-00493159 ;
    skos:definition "The function of ensuring that businesses have access to the services of essential infrastructure facilities including gas pipelines, electricity transmission wires, rail tracks and some airport facilities. Includes developing access codes and responding to appeals lodged to a higher authority. Also includes participation in various consultative groups, advising on access principles, seeking of public submissions, assessing and accepting undertakings and making determinations." ;
    skos:inScheme :conceptScheme: ;
    skos:prefLabel "Access Regulation" .

:0291  a crs:Function, ra:Class,
        skos:Concept ;
    crs:isPerformedBy [ crs:hasAgent ca:8199 ] ;
    dct:source ras:2003-00349230 ;
    skos:definition "The function of managing the appointments and ongoing personnel arrangements of commissioners, including the chairman and associate members of the commission. Includes salaries and leave arrangements, travel arrangements and allowances and all separation arrangements. Also includes secretariat services to the commission. " ;
    skos:inScheme :conceptScheme: ;
    skos:prefLabel "Commission Administration" .

:0292  a crs:Function, ra:Class,
        skos:Concept ;
    crs:isPerformedBy [ crs:hasAgent ca:8199 ],
        [ crs:hasAgent ca:8199 ],
        [ crs:hasAgent ca:8199 ] ;
    dct:source ras:2003-00349230,
        ras:2007-00493159 ;
    skos:definition "The function of protecting consumers (household and business) from anti-competitive and unfair market practice, by ensuring industry compliance with trade practices legislation and associated state or territory legislation. Includes management of mergers, acquisitions, authorisations and notifications, monitoring of product safety, prices (including price exploitation relating to tax initiatives), and false, misleading or deceptive conduct (including misleading advertising). " ;
    skos:inScheme :conceptScheme: ;
    skos:prefLabel "Competition And Consumer Protection",
        "Competition And Consumer Protection " .

:0293  a crs:Function, ra:Class,
        skos:Concept ;
    crs:isPerformedBy [ crs:hasAgent ca:8199 ],
        [ crs:hasAgent ca:8199 ] ;
    dct:source ras:2003-00349230 ;
    skos:definition "The function of providing trade practices information and guidance to the general community and persons engaged in trade or commerce with the purpose of minimising the need for enforcement and litigation. Includes programs and activities to increase the knowledge of rights and obligations under legislation (including the Trade Practices Act 1974), programs and activities to increase public understanding of the commission's role, policies, and procedures, as well as promoting public awareness of competition and consumer protection law and utility regulation issues. " ;
    skos:inScheme :conceptScheme: ;
    skos:prefLabel "Education And Information Services" .

:0294  a crs:Function, ra:Class,
        skos:Concept ;
    crs:isPerformedBy [ crs:hasAgent ca:8199 ],
        [ crs:hasAgent ca:8199 ] ;
    dct:source ras:2003-00349230 ;
    skos:definition "The function of facilitating agreements between countries, liaison and cooperation with international agencies (including Asia-Pacific Economic Cooperation group, World Trade Organization, and the Organisation for Economic Co-operation and Development), technical assistance, training and support in development of legislation, engagement in competition and consumer protection matters, bilateral agreements, international trading seminars, consultancies in capacity building, involvement in development of a common set of competition principles and effective competition regimes. " ;
    skos:inScheme :conceptScheme: ;
    skos:prefLabel "International Relations" .

:0295  a crs:Function, ra:Class,
        skos:Concept ;
    crs:isPerformedBy [ crs:hasAgent ca:8199 ],
        [ crs:hasAgent ca:8199 ] ;
    dct:source ras:2003-00349230 ;
    skos:definition "The function of investigating alleged breaches of legislation, breaches of conduct and breaches of undertakings. Includes receiving and assessing complaints and inquiries, research, obtaining information by conducting hearings and carrying out interviews and inspections on the premises. Includes briefing, and reporting, for the commission to litigate. Also includes initiating proceedings for legal enforcement and briefing counsel. " ;
    skos:inScheme :conceptScheme: ;
    skos:prefLabel "Investigation And Legal Enforcement" .

:0296  a crs:Function, ra:Class,
        skos:Concept ;
    crs:isPerformedBy [ crs:hasAgent ca:8199 ],
        [ crs:hasAgent ca:8199 ] ;
    dct:source ras:2003-00349230 ;
    skos:definition "The function of examining critically the laws in force relatinig to trade practices and consumer protection and other matters referred from the Minister, and reporting to the Minister. Includes research and consultation to determine the need for reform in response to matters referred by the Minister or the National Competition Council, or review instigated by the commission, and to make recommendations. " ;
    skos:inScheme :conceptScheme: ;
    skos:prefLabel "Law Reform And Research" .

:0297  a crs:Function, ra:Class,
        skos:Concept ;
    crs:isPerformedBy [ crs:hasAgent ca:8376 ],
        [ crs:hasAgent ca:8376 ] ;
    dct:source ras:2003-00218091,
        ras:2007-00263775 ;
    skos:definition "The function of assessing the quality of practices in child care services and awarding accreditation in compliance with standards. Includes registration of services as part of eligibility for financial assistance. Also includes resolving complaints about child care services; the development, evaluation and promotion of accreditation programs and policies eg. the Quality Improvement and Accreditation System and Family Day Care Quality Assurance; and advice and liaison on quality child care matters. " ;
    skos:inScheme :conceptScheme: ;
    skos:prefLabel "Accreditation" .

:0298  a crs:Function, ra:Class,
        skos:Concept ;
    crs:isPerformedBy [ crs:hasAgent ca:8376 ] ;
    dct:source ras:2009-00831189 ;
    skos:definition """The business of selecting, training, endorsing and offering continuing support to individuals as National Childcare Accreditation Council (NCAC) Endorsed Quality Assurance (QA) Trainers who can deliver training to child care services on the processes associated with the 5 Steps of Child Care Quality Assurance (CCQA).
Includes:
• Receiving applications and selecting those who meet the selection criteria for Trainers, processing applications for re-endorsement
• Developing policies and procedures
• Promoting the program and availability of QA Trainers
• Conducting training sessions
• Developing training materials to train the QA Trainers
• Developing a NCAC Endorsed Training Kit or similar material that the QA Trainers can use to deliver training to child care services
• Offering continuing support to QA Trainers
• Conducting regular meetings to work with other teams within NCAC and within the team itself to support QA Trainers and evaluate the program
• Developing new methods and resources to support services to meet the Child Care Quality Assurance standards.""";
    skos:inScheme :conceptScheme: ;
    skos:prefLabel "Child Care Quality Assurance Training And Support" .

:0299  a crs:Function, ra:Class,
        skos:Concept ;
    crs:isPerformedBy [ crs:hasAgent ca:8376 ] ;
    dct:source ras:2003-00218091 ;
    skos:definition "The function of appointing, training, assessing and managing accreditation examiners eg. validators and moderators." ;
    skos:inScheme :conceptScheme: ;
    skos:prefLabel "Examiners" .

:0300  a crs:Function, ra:Class,
        skos:Concept ;
    crs:isPerformedBy [ crs:hasAgent ca:8376 ] ;
    dct:source ras:2003-00218091 ;
    skos:definition "The function of administering and managing the Council and its appointed members. The Chairperson and the Council members are appointed by the Commonwealth Minister responsible for child care services. Includes managing Council Meetings and the Annual General Meeting and complying with statutory regulations in relation to incorporation. " ;
    skos:inScheme :conceptScheme: ;
    skos:prefLabel "Governance" .

:0301  a crs:Function, ra:Class,
        skos:Concept ;
    crs:isPerformedBy [ crs:hasAgent ca:8460 ] ;
    dct:source ras:2005-00474525 ;
    skos:definition "The function of classifying against established criteria. Includes assessment and classification of children’s programs by staff and consultants against the Children’s Television Standards, determination of adult telephone services and issue of evidentiary certificates, opinions regarding licence categories and control opinions. Also includes plans, procedures and policies and reports regarding classification." ;
    skos:inScheme :conceptScheme: ;
    skos:prefLabel "Classification" .

:0302  a crs:Function, ra:Class,
        skos:Concept ;
    crs:isPerformedBy [ crs:hasAgent ca:8460 ] ;
    dct:source ras:2003-00677339 ;
    skos:definition "The function of protecting the interests of communications consumers by ensuring consumers are well-informed about their rights and industry issues through advice and consumer awareness and information programs. Includes liaison with other regulators, including those currently known as the Australian Competition and Consumer Commission (ACCC) and the Telecommunications Industry Ombudsman, and formal consultative arrangements. Includes the development of codes and standards, registration of codes, monitoring industry performance and compliance with codes and standards and undertaking investigations to address consumer protection issues. Also includes the development, application, and administration of what are currently known as the Customer Services Guarantee (CSG) Standard and Universal Service Obligation (USO) and National Relay Service (NRS) regime requirements." ;
    skos:inScheme :conceptScheme: ;
    skos:prefLabel "Consumer Interests" .

:0303  a crs:Function, ra:Class,
        skos:Concept ;
    crs:isPerformedBy [ crs:hasAgent ca:8460 ] ;
    dct:source ras:2003-00677339 ;
    skos:definition "The function of managing the corporate framework established by the agency's governing body. Includes managing the agency's governing body, which is responsible for setting and approving the overall corporate direction and establishing and complying with rules and procedures for corporate operations. Includes those activities associated with providing secretariat support to the Board in the conduct of its work and administrative support to the Board members including arranging for travel and remuneration for duties performed." ;
    skos:inScheme :conceptScheme: ;
    skos:prefLabel "Corporate Governance" .

:0304  a crs:Function, ra:Class,
        skos:Concept ;
    crs:isPerformedBy [ crs:hasAgent ca:8460 ] ;
    dct:source ras:2003-00677339 ;
    skos:definition "The function of testing radiocommunications and telecommunications equipment against mandatory standards, equipment compliance requirements, overseas equipment performance arrangements, arrangements specified in licences, or other specified requirements. Includes maintaining the agency's accreditation as a recognised testing authority.  " ;
    skos:inScheme :conceptScheme: ;
    skos:prefLabel "Equipment Assessment" .

:0305  a crs:Function, ra:Class,
        skos:Concept ;
    crs:isPerformedBy [ crs:hasAgent ca:8460 ] ;
    dct:source ras:2003-00677339 ;
    skos:definition "The function of providing high-level technical advice to the Minister on specific issues of importance that relate to the unique functions of the organisation. The advice is provided by boards, councils, committees, and advisory bodies formally established by the agency for which the agency provides secretariat services. Includes authorisation, appointments, and remuneration for appointed individuals, members of councils, committees, and advisory bodies, and the provision of other administrative services. " ;
    skos:inScheme :conceptScheme: ;
    skos:prefLabel "Industry Relations" .

:0306  a crs:Function, ra:Class,
        skos:Concept ;
    crs:isPerformedBy [ crs:hasAgent ca:8460 ] ;
    dct:source ras:2003-00677339 ;
    skos:definition "The function of managing the radiofrequency spectrum in accordance with the objectives and requirements of radiocommunications and associated legislation. Includes the activities of planning, pricing, allocation, frequency assignment, licensing, compliance, and regulation. Includes participating in industry processes to develop standards, determine industry standards, and make radiocommunications standards. Includes representing Australia's radiocommunications position and interests in the regional and international areas. " ;
    skos:inScheme :conceptScheme: ;
    skos:prefLabel "Radiocommunications Regulation" .

:0307  a crs:Function, ra:Class,
        skos:Concept ;
    crs:isPerformedBy [ crs:hasAgent ca:8460 ] ;
    dct:source ras:2003-00677339 ;
    skos:definition "The function of regulating telecommunications activities, including administering the telecommunications numbering plan and regulating telecommunications infrastructure and facilities establishment, maintenance, operation, and access. Includes issuing and administering licences, nominated carrier declarations, and trial certificates, developing and monitoring compliance with licence conditions, service provider rules, and other requirements under the telecommunications legislation. Includes registering industry codes, participating in industry processes to develop codes and standards, determine industry standards, and make technical standards. Includes monitoring and undertaking investigations into industry performance and enforcing compliance with codes and standards. Includes regulation of peremium rate services including the development of service provider rules and monitoring for compliance. Includes representing Australia's communications position and interests in the regional and international arenas and the activities of number allocation, information programs and permissions. " ;
    skos:inScheme :conceptScheme: ;
    skos:prefLabel "Telecommunications Regulation" .

:0308  a crs:Function, ra:Class,
        skos:Concept ;
    crs:isPerformedBy [ crs:hasAgent ca:8480 ] ;
    dct:source ras:2004-00136572 ;
    skos:definition "The function of managing the sale of major Government business assets. Includes scoping studies to determine the viability or otherwise of the sale and the sale method; the provision of advice; preparation of the asset for sale either as a trade sale or sale by the public offering; marketing and advertising; the engagement of specialist advisers and consultants; the preparation of sale documents; including requests for tender; management of the sale process; including evaluation of tender bids and receipt of applications; and sale finalisation, including contract negotiations. Also includes evaluation and oversight of the sale of minor Government business assets carried out by other agencies." ;
    skos:inScheme :conceptScheme: ;
    skos:prefLabel "Asset Sales" .

:0309  a crs:Function, ra:Class,
        skos:Concept ;
    crs:isPerformedBy [ crs:hasAgent ca:8480 ] ;
    dct:source ras:2005-00627309 ;
    skos:definition "The function of designing and constructing architectural and engineering works of any kind including fitouts, refurbishments and extensions and conservation of such works. Includes preparing drawings and specifications, surveying, tendering, managing and overseeing of construction activities by internal or contracted labour and liaison with clients." ;
    skos:inScheme :conceptScheme: ;
    skos:prefLabel "Capital Works" .

:0310  a crs:Function, ra:Class,
        skos:Concept ;
    crs:isPerformedBy [ crs:hasAgent ca:8480 ] ;
    dct:source ras:2004-00136572 ;
    skos:definition """The function of providing car with driver transportation services within Australia to individuals approved by Government, including the Prime Minister, Senators, Members of Parliament, the Governor General, overseas guests of government and other officials. Includes leasing of vehicles, vehicle allocation, and driver training.
""";
    skos:inScheme :conceptScheme: ;
    skos:prefLabel "Car With Driver Services" .

:0311  a crs:Function, ra:Class,
        skos:Concept ;
    crs:isPerformedBy [ crs:hasAgent ca:8480 ] ;
    dct:source ras:2004-00136572 ;
    skos:definition "The function of managing the Commonwealth’s annual budget process. Includes developing policies in relation to the budget; planning, developing and coordinating processes required to produce the budget, developing and distributing advice; briefings, guidelines and reporting on the budget; budget processes or budget estimates; developing statements of proposed expenditure; collecting, collating, interpreting and analysing financial information relating to the budget; liaising and exchanging information with other Government agencies; providing advice on longer term budgetary issues; preparing and drafting Appropriation Bills." ;
    skos:inScheme :conceptScheme: ;
    skos:prefLabel "Commonwealth Budget Management" .

:0312  a crs:Function, ra:Class,
        skos:Concept ;
    crs:isPerformedBy [ crs:hasAgent ca:8480 ] ;
    dct:source ras:2004-00136572 ;
    skos:definition "The function of managing the Commonwealth’s financial resources. Includes developing policy on the management of finances in the Commonwealth; providing advice on economic conditions; analysing the overall financial position of the Commonwealth over time; including movements in balance sheets and capital investment proposals; establishing, operating and maintaining accounting systems for the Commonwealth; liaising with other agencies; advising Commonwealth agencies on alternative financing arrangements; advising the Minister on financial management issues facing Government, providing Government with a comprehensive overview of financial performance; financial reporting (including annual financial statements and reporting on agencies' effectiveness and efficiency); developing and/or implementing financial policies, procedures, systems and other services." ;
    skos:inScheme :conceptScheme: ;
    skos:prefLabel "Commonwealth Financial Management" .

:0313  a crs:Function, ra:Class,
        skos:Concept ;
    crs:isPerformedBy [ crs:hasAgent ca:8480 ] ;
    dct:source ras:2004-00136572 ;
    skos:definition "The function of identifying, quantifying and managing future financial risks to the Commonwealth through the analysis and calculation of costs; and promoting the use of the Commonwealth’s fund for insurable risks. Includes the administration and management of insurance claims made by Commonwealth agencies." ;
    skos:inScheme :conceptScheme: ;
    skos:prefLabel "Commonwealth Insurance" .

:0314  a crs:Function, ra:Class,
        skos:Concept ;
    crs:isPerformedBy [ crs:hasAgent ca:8480 ] ;
    dct:source ras:2005-00627309 ;
    skos:definition "The function of managing, including on a commercial basis, non-Defence-related properties and places owned by the Commonwealth within Australia, or leased by the Commonwealth. Includes managing and monitoring contract performance against cost and service standards relating to those properties, acquiring, selling, transferring, divesting or otherwise disposing of properties owned by the Commonwealth, implementing commercial leasing arrangements for all users of Commonwealth property, developing and implementing property management strategies and refining commercial arrangements for Commonwealth office buildings. Also includes matters relating to the development and application of the Commonwealth property framework, the Commonwealth construction procurement policy and matters relating to the administration of the legislation such as Public Works Act 1969." ;
    skos:inScheme :conceptScheme: ;
    skos:prefLabel "Commonwealth Property Management" .

:0315  a crs:Function, ra:Class,
        skos:Concept ;
    crs:isPerformedBy [ crs:hasAgent ca:8480 ] ;
    dct:source ras:2004-00136572 ;
    skos:definition "The function of fostering the use of risk management techniques and methodologies by Commonwealth departments and agencies in their activities and business practices; managing contracts to deliver risk management services to those agencies; and promoting a risk management culture within the Commonwealth" ;
    skos:inScheme :conceptScheme: ;
    skos:prefLabel "Commonwealth Risk Management" .

:0316  a crs:Function, ra:Class,
        skos:Concept ;
    crs:isPerformedBy [ crs:hasAgent ca:8480 ] ;
    dct:source ras:2004-00136572 ;
    skos:definition "The function of examining and managing special types of requests made to the Commonwealth for financial assistance, when such requests would not form part of normal administrative procedures. Includes the consideration and management of requests for compensation from persons who may have been unfairly disadvantaged by the Commonwealth Government but who have no right of legal claim; the payment of amounts owed a person by the Commonwealth, sought between the time of death and the granting of probate; and the waiving of the recovery of amounts of money owing to the Commonwealth, thereby expunging the Commonwealth’s legal right to that money. Also the development of policy and procedures to manage such requests; the constitution of an advisory committee when requests are in excess of a given amount; reporting on these activities and the development of advice in relation to these matters." ;
    skos:inScheme :conceptScheme: ;
    skos:prefLabel "Financial Redress" .

:0317  a crs:Function, ra:Class,
        skos:Concept ;
    crs:isPerformedBy [ crs:hasAgent ca:8480 ] ;
    dct:source ras:2004-00136572 ;
    skos:definition "The function of providing non-repayable funding to non-government and community organisations in the form of grants to support designated community activities and to achieve aims and objectives that are consistent with Government policy. Includes the examination of a request for grant funding; decision making as to the appropriate authority for establishing and managing grants; liaison and communication with requestors for grants and other stakeholders as required; determining the amount of the grant and the accountability requirements and approvals." ;
    skos:inScheme :conceptScheme: ;
    skos:prefLabel "Grants Administration" .

:0318  a crs:Function, ra:Class,
        skos:Concept ;
    crs:isPerformedBy [ crs:hasAgent ca:8480 ] ;
    dct:source ras:2007-00172603 ;
    skos:definition "The function of providing evaluations and audits of relevant indigenous-specific programs administered by Australian Government bodies and of activities of individual or organisation that has recieved funding or a guarantee, or other property under any relevant program.  Includes liaising with goverment and non-government organisations and preparing responses to questions raised by Ministers or in Parliament." ;
    skos:inScheme :conceptScheme: ;
    skos:prefLabel "Indigenous Programs Evaluation And Audit" .

:0319  a crs:Function, ra:Class,
        skos:Concept ;
    crs:isPerformedBy [ crs:hasAgent ca:8480 ] ;
    dct:source ras:2004-00136572 ;
    skos:definition "The function of managing the consolidation and outsourcing of the Commonwealth’s information technology infrastructure. Includes initial scoping studies; definition of requirements specifications in consultation with agencies; the development of project documentation, templates, and tender documents; due diligence; management of the tender process, including evaluation of the corporate, technical, industry development and financial worth of each tenderer; and negotiation and finalisation of contracts." ;
    skos:inScheme :conceptScheme: ;
    skos:prefLabel "Information Technology Outsourcing" .

:0320  a crs:Function, ra:Class,
        skos:Concept ;
    crs:isPerformedBy [ crs:hasAgent ca:8480 ] ;
    dct:source ras:2004-00136572 ;
    skos:definition "The function of overseeing the governance and financial performance of Government authorities and companies that the Commonwealth has a controlling interest in. Includes collecting, receiving, researching and analysing information on, or relating to, the performance of Government Business Enterprises that are either wholly or partially owned by the Commonwealth, or are in the process of being sold; and advising the delegated representative or shareholder of the Commonwealth. Includes setting policy guidelines for Commonwealth statutory authorities." ;
    skos:inScheme :conceptScheme: ;
    skos:prefLabel "Oversight Of Government Businesses" .

:0321  a crs:Function, ra:Class,
        skos:Concept ;
    crs:isPerformedBy [ crs:hasAgent ca:8480 ] ;
    dct:source ras:2004-00136572 ;
    skos:definition "The function of administering, managing, and paying allowances and additional benefits for Senators and Members of Parliament and certain office-holders, salaries for Ministers of State and superannuation for certain types of office holders including Senators and Members of Parliament." ;
    skos:inScheme :conceptScheme: ;
    skos:prefLabel "Parliamentary Entitlements" .

:0322  a crs:Function, ra:Class,
        skos:Concept ;
    crs:isPerformedBy [ crs:hasAgent ca:8480 ] ;
    dct:source ras:2004-00136572 ;
    skos:definition "The function of administering a superannuation scheme to provide superannuation benefits for Senators and Members of Parliament, and their beneficiaries. Includes calculation and assessment of superannuation benefits; the production of regular statements; advice to and liaison with Senators and Members of Parliament and their beneficiaries, secretariat support for the Trust; and the development of policy and procedures." ;
    skos:inScheme :conceptScheme: ;
    skos:prefLabel "Parliamentary Superannuation" .

:0323  a crs:Function, ra:Class,
        skos:Concept ;
    crs:isPerformedBy [ crs:hasAgent ca:8480 ] ;
    dct:source ras:2004-00136572 ;
    skos:definition "The function of arranging visits and exchange programs on behalf of the Australian Political Exchange Council for members of political parties from Australia and other countries, and sponsoring participation in individual study tours and international forums overseas. Includes the establishment of agreements, advice and reporting, and other secretariat support for the Australian Political Exchange Council." ;
    skos:inScheme :conceptScheme: ;
    skos:prefLabel "Political Exchange Program" .

:0324  a crs:Function, ra:Class,
        skos:Concept ;
    crs:isPerformedBy [ crs:hasAgent ca:8480 ] ;
    dct:source ras:2004-00136572 ;
    skos:definition """The function of assisting Commonwealth departments and agencies with the procurement of goods and services through the development of policies, guidelines, best practice advice, standard contract clauses, and other means; and promoting the development of Australian industry. Includes the development and running of workshops and seminars; the development of draft tender and contract documentation, and costing models; the pre-qualification of Australian businesses to supply certain classes of goods and services to the Commonwealth; the collection and dissemination of information on potential suppliers of goods and services; the facilitation of access to small business to the Commonwealth market; assisting Commonwealth departments and agencies to cost and market test their activities; providing a means by which individuals or
businesses can complain about Government purchasing; and participating in international forums and negotiations on Government procurement activity.""";
    skos:inScheme :conceptScheme: ;
    skos:prefLabel "Procurement Management" .

:0325  a crs:Function, ra:Class,
        skos:Concept ;
    crs:isPerformedBy [ crs:hasAgent ca:8480 ] ;
    dct:source ras:2004-00136572 ;
    skos:definition "The function of developing and providing policy and advice in Commonwealth superannuation issues. Includes preparing amendments to superannuation legislation, monitoring the employer costs of superannuation and unfunded liabilities; communicating proposed changes to superannuation to agencies (as employers); managing contracts for actuarial services; managing superannuation issues relating to former Commonwealth employees, including former Australian overseas territories and managing the processes involved in appointing individuals to Commonwealth superannuation boards. " ;
    skos:inScheme :conceptScheme: ;
    skos:prefLabel "Public Sector Superannuation" .

:0326  a crs:Function, ra:Class,
        skos:Concept ;
    crs:isPerformedBy [ crs:hasAgent ca:8480 ] ;
    dct:source ras:2007-00172603 ;
    skos:definition "The function of facilitating and providing access to government information and services. Includes access through online services, directory services, government domain administration, promotion of information and technical interoperability. Also includes development and management of Whole of Government web sites and directories." ;
    skos:inScheme :conceptScheme: ;
    skos:prefLabel "Whole Of Government Information And Services Facilitation" .

:0327  a crs:Function, ra:Class,
        skos:Concept ;
    crs:isPerformedBy [ crs:hasAgent ca:8480 ] ;
    dct:source ras:2007-00172603 ;
    skos:definition "The function of developing and promoting whole of government Information and Communications Technology (ICT) management policies to inform the design and implementation of government programs.  Includes the provision of assistance, guidance and better practice advice to agencies applying ICT to government operations; and fosters the efficient and effective use of ICT by Australian Government departments and agencies.  Also includes working with government and other bodies at the local, national and international level to develop and maintain Australia's position as a world leader in e-government." ;
    skos:inScheme :conceptScheme: ;
    skos:prefLabel "Whole Of Government Information Management Policy And Guidance" .

:0328  a crs:Function, ra:Class,
        skos:Concept ;
    crs:isPerformedBy [ crs:hasAgent ca:8550 ] ;
    dct:source ras:2007-00576124 ;
    skos:definition """The function of communicating Archives’ role, collection and unique business to external audiences for the purposes of promotion, professional leadership, collaboration and collection interpretation. Includes raising awareness and facilitating engagement through events, functions, conferences, addresses (presentations), joint ventures, scholarships, marketing, media and visits. Also includes providing leadership and support in Australia and overseas in matters of professional interest and facilitating
learning and accessibility through programs which interpret the collection, such as exhibitions and education initiatives. Also includes the promotion of the core business of Archives and managing
organisation-wide interaction with key stakeholder groups (such as Consultative Forums). Also includes hosting visits from representatives of other organisations and members of the archival profession and Archives staff visiting other archival organisations. Excludes specific liaison with stakeholders for the purpose of developing, implementing and supporting unique business programs. Also excludes the production of publications aimed at promoting the collection and activities of the Archives.""";
    skos:inScheme :conceptScheme: ;
    skos:prefLabel "Archives External Communications" .

:0329  a crs:Function, ra:Class,
        skos:Concept ;
    crs:isPerformedBy [ crs:hasAgent ca:8550 ] ;
    dct:source ras:2007-00576124 ;
    skos:definition """The function of developing information standards, including recordkeeping standards, for use by Commonwealth agencies. Includes developing internal, and endorsing external, standards, procedures,
codes of best practice and guidelines covering creation, capture and management of records and business information. Also includes providing guidance and advice to agencies to assist the adoption of
these standards, including the provision of training and compliance activities.""";
    skos:inScheme :conceptScheme: ;
    skos:prefLabel "Information Management Standards & Operations" .

:0330  a crs:Function, ra:Class,
        skos:Concept ;
    crs:isPerformedBy [ crs:hasAgent ca:8550 ] ;
    dct:source ras:2007-00576124 ;
    skos:definition "The function of providing public and official access to records of the Commonwealth. Includes providing a range of services to facilitate access such as the handling of reference enquiries, copying of archival records, examining records prior to release, and managing the appeals process." ;
    skos:inScheme :conceptScheme: ;
    skos:prefLabel "Records Access Management " .

:0331  a crs:Function, ra:Class,
        skos:Concept ;
    crs:isPerformedBy [ crs:hasAgent ca:8550 ] ;
    dct:source ras:2007-00576124 ;
    skos:definition "The function of managing the physical control of records irrespective of their location. Includes transfer of records to the custody of the Archives, the management of their location and storage, and lending and withdrawal activities. Also includes the negotiation of agreements establishing custody arrangements to allow Commonwealth archival records to be stored outside of the Archives." ;
    skos:inScheme :conceptScheme: ;
    skos:prefLabel "Records Custody & Storage" .

:0332  a crs:Function, ra:Class,
        skos:Concept ;
    crs:isPerformedBy [ crs:hasAgent ca:8550 ] ;
    dct:source ras:2007-00576124 ;
    skos:definition """The function of managing the disposition of Commonwealth records. Includes analysing the business activities of government with the aim of identifying the need for records taking into account stakeholder requirements, risks, benefits and costs. Includes the development of disposal authorities authorising the disposal of records, formulating policies and procedures and providing advice on the implementing disposal actions. Includes applying disposal actions to records held in archival care, and monitoring sentencing activities carried out by agencies or contractors. Also includes activities involved in the transfer of custody and ownership of records following the privatisation or sale of a government entity,
or its shares in an entity, and the imposition of disposal freezes.""";
    skos:inScheme :conceptScheme: ;
    skos:prefLabel "Records Evaluation & Disposal " .

:0333  a crs:Function, ra:Class,
        skos:Concept ;
    crs:isPerformedBy [ crs:hasAgent ca:8550 ] ;
    dct:source ras:2007-00576124 ;
    skos:definition "The function of controlling records and documenting their provenance through registration, arrangement and description. Includes monitoring administrative change to maintain the accuracy of the intellectual control framework. Also includes developing, maintaining and reviewing the Commonwealth Record Series (CRS) system used by the Archives." ;
    skos:inScheme :conceptScheme: ;
    skos:prefLabel "Records Intellectual Control" .

:0334  a crs:Function, ra:Class,
        skos:Concept ;
    crs:isPerformedBy [ crs:hasAgent ca:8550 ] ;
    dct:source ras:2007-00576124 ;
    skos:definition "The function of devising strategies and implementing techniques to preserve the ongoing integrity and useability of records in any format. Includes the application of conservation measures to treat records under threat, or prevent further deterioration. Also includes providing advice on preservation matters, developing strategies and policy to guide the application of preservation processes, undertaking preservation techniques such as copying and conversion, managing preservation processes relating to the loan of archival records, undertaking research and development of new preservation techniques and approaches, surveying records, and setting standards to support preservation processes." ;
    skos:inScheme :conceptScheme: ;
    skos:prefLabel "Records Preservation Management" .

:0335  a crs:Function, ra:Class,
        skos:Concept ;
    crs:isPerformedBy [ crs:hasAgent ca:8551 ],
        [ crs:hasAgent ca:8551 ] ;
    dct:source ras:2007-00122077,
        ras:2008-00658152 ;
    skos:definition "The function of registrating patent and trade marks attorneys. Includes accrediting courses and units of study, approving qualifications and conducting examinations and maintaining a register of patent and trademarks attorneys. Also includes the establishment of standards for the professional conduct of attorneys, handling complaints, conducting disciplinary hearings and imposing penalties." ;
    skos:inScheme :conceptScheme: ;
    skos:prefLabel "Attorney Registration" .

:0336  a crs:Function, ra:Class,
        skos:Concept ;
    crs:isPerformedBy [ crs:hasAgent ca:8551 ] ;
    dct:source ras:2004-00068493 ;
    skos:definition "The function of processing applications for the registration of designs including Olympic designs. Includes reviewing and deciding disputed matters relating to the granting or refusal of design rights; maintaining the Register of Designs and the Register of Olympic Designs; providing advice on the application of design legistlation, World Intellectual Property Organization matters pertaining to designs, and on other international and bilateral design matters." ;
    skos:inScheme :conceptScheme: ;
    skos:prefLabel "Design Rights Management" .

:0337  a crs:Function, ra:Class,
        skos:Concept ;
    crs:isPerformedBy [ crs:hasAgent ca:8551 ] ;
    dct:source ras:2004-00068493 ;
    skos:definition "The function of creating and implementing strategies and programs that aim to raise the awareness of Australians about the Australian intellectual property system and related issues. Includes conducting market research; preparing marketing and promotion strategies; promoting services at exhibitions and expos; developing editorial programs for tertiary institutions, business advisers such as accountants and small business; delivering information sessions to professional bodies in Australian States and Territories; and coordinating public relations activities. Also includes the management of customer services; handling reactions about the Australian intellectual property system such as non-enforcement issues; customer consultation and feedback." ;
    skos:inScheme :conceptScheme: ;
    skos:prefLabel "Intellectual Property Awareness" .

:0338  a crs:Function, ra:Class,
        skos:Concept ;
    crs:isPerformedBy [ crs:hasAgent ca:8551 ] ;
    dct:source ras:2004-00068493 ;
    skos:definition "The function of developing the intellectual property system. Includes developing policies, strategies and programs; preparing amendments for existing intellectual property legislation or developing new legislation to implement new policies; and conducting research and analysis on intellectual property and how it affects the Australian economy. Also includes influencing the development of the international intellectual property system to ensure Australian innovators are able to seek protection for their intellectual property throughout the world. This includes delivering training to international bodies; presenting papers at meetings and conferences; tendering with external organisations for international projects; and negotiating and entering into arrangements with other countries’ intellectual property offices to conduct patent searches and examination services on their behalf. " ;
    skos:inScheme :conceptScheme: ;
    skos:prefLabel "Intellectual Property Development" .

:0339  a crs:Function, ra:Class,
        skos:Concept ;
    crs:isPerformedBy [ crs:hasAgent ca:8551 ] ;
    dct:source ras:2004-00068493 ;
    skos:definition "The function of processing applications for the granting of patents. Includes reviewing and deciding disputed matters relating to the granting or refusal of patent rights; maintaining a register of patents; providing advice on the application of patents legislation, World Intellectual Property Organization matters pertaining to patents, and on other international and bilateral patent matters. Also includes activities of processing Patent Cooperation Treaty applications such as Receiving Office, International Searching Authority and International Preliminary Examination Authority activities; examining patent applications and undertaking international searches on behalf of other countries and undertaking commercial searches." ;
    skos:inScheme :conceptScheme: ;
    skos:prefLabel "Patent Rights Management" .

:0340  a crs:Function, ra:Class,
        skos:Concept ;
    crs:isPerformedBy [ crs:hasAgent ca:8551 ] ;
    dct:source ras:2006-00587410 ;
    skos:definition "The function of processing applications for the registration of proprietary rights for breeders of new plant, algae and fungi varieties. Includes reviewing and deciding on disputed matters relating to the granting, revocation or refusal of rights, maintaining the register of plant varieties, and providing advice on the application of rights legislation, matters pertaining to breeder's rights, and on other international and bilateral breeder's rights matters especially those relating to international agreements for the protection of new plant varieties. Also includes administration of the Plant Breeder's Rights Advisory Committee, consultation with the public and the registration of technical consultants." ;
    skos:inScheme :conceptScheme: ;
    skos:prefLabel "Plant Breeder'S Rights Management" .

:0341  a crs:Function, ra:Class,
        skos:Concept ;
    crs:isPerformedBy [ crs:hasAgent ca:8551 ] ;
    dct:source ras:2004-00068493 ;
    skos:definition "The function of processing applications for the registration of trade marks. Includes considering and deciding disputed matters relating to the granting or refusal of trade mark rights; maintaining the Register of Trade Marks; providing advice on application of the trade markds legistlation, World Intellectual Property organization matters pertaining to trade marks, and on other international and bilateral trade mark matters." ;
    skos:inScheme :conceptScheme: ;
    skos:prefLabel "Trade Mark Rights Management" .

:0342  a crs:Function, ra:Class,
        skos:Concept ;
    crs:isPerformedBy [ crs:hasAgent ca:8571 ] ;
    dct:source ras:2007-00211258 ;
    skos:definition "The function of providing services to the public, agencies, organisations and other business areas. Includes developing new business opportunities and providing commercial services such as document imaging." ;
    skos:inScheme :conceptScheme: ;
    skos:prefLabel "Commercial Services" .

:0343  a crs:Function, ra:Class,
        skos:Concept ;
    crs:isPerformedBy [ crs:hasAgent ca:8571 ] ;
    dct:source ras:2007-00211258 ;
    skos:definition "The function of supervising the regulated corporate and finance sectors to ensure participants are complying with legislation.  Includes the provision of advice, liaising with and monitoring industry participants, conducting surveillance of industry participants and referring cases to other business units or regulators for further action if issues are identified." ;
    skos:inScheme :conceptScheme: ;
    skos:prefLabel "Compliance Management" .

:0344  a crs:Function, ra:Class,
        skos:Concept ;
    crs:isPerformedBy [ crs:hasAgent ca:8571 ] ;
    dct:source ras:2007-00211258 ;
    skos:definition "The function of ensuring protection for consumers of insurance, superannuation and banking services and the corporate and finance sectors. Includes the receipt and assessment of complaints by the public of suspected corporate and financial services misconduct, conducting investigations into complaints to determine if further action is required, providing consumer education programs, issuing public warnings on issues such as financial scams and illegal investment offers and handling general enquiries regarding consumer issues. " ;
    skos:inScheme :conceptScheme: ;
    skos:prefLabel "Consumer Protection" .

:0345  a crs:Function, ra:Class,
        skos:Concept ;
    crs:isPerformedBy [ crs:hasAgent ca:8571 ] ;
    dct:source ras:2007-00211258 ;
    skos:definition "The function of regulating entry to the corporate and finance sector. Includes managing the lodgement of annual returns, licensing of financial services, financial markets and clearing and settlement facilities, registration of managed investment schemes, auditors, liquidators and authorised audit companies, approval of participants such as dispute resolution schemes and authorised assessors, and processing changes of licence, registration and participants' details. Also includes managing applications for exemptions, education and information programs and policy development." ;
    skos:inScheme :conceptScheme: ;
    skos:prefLabel "Corporate And Finance Regulation" .

:0346  a crs:Function, ra:Class,
        skos:Concept ;
    crs:isPerformedBy [ crs:hasAgent ca:8571 ] ;
    dct:source ras:2007-00211258 ;
    skos:definition "The function of managing the outstanding interests in deregistered company property. Includes managing requests from stakeholders to deal with property, provision of advice and maintaining the register of property vested in the agency." ;
    skos:inScheme :conceptScheme: ;
    skos:prefLabel "Deregistered Company Property" .

:0347  a crs:Function, ra:Class,
        skos:Concept ;
    crs:isPerformedBy [ crs:hasAgent ca:8571 ] ;
    dct:source ras:2007-00211258 ;
    skos:definition "The function of managing funds received from financial institutions and companies and classified as unclaimed. Includes money from inactive bank, credit union and building society accounts and compulsory acquisition of shares resulting from takeovers, and unclaimed money from insurance policies where an owner cannot be located.  " ;
    skos:inScheme :conceptScheme: ;
    skos:prefLabel "Financial Management (Unclaimed Money)" .

:0348  a crs:Function, ra:Class,
        skos:Concept ;
    crs:isPerformedBy [ crs:hasAgent ca:8571 ] ;
    dct:source ras:2007-00211258 ;
    skos:definition "The function of establishing relationships with overseas regulatory counterparts. Includes requesting and providing information and evidence for investigations, contributing to the development of cross-border standards and providing training opportunities for overseas regulators and agencies." ;
    skos:inScheme :conceptScheme: ;
    skos:prefLabel "International Relations" .

:0349  a crs:Function, ra:Class,
        skos:Concept ;
    crs:isPerformedBy [ crs:hasAgent ca:8571 ] ;
    dct:source ras:2007-00211258 ;
    skos:definition "The function of conducting formal investigations into organisations and individuals associated with serious corporate crime and civil misconduct and misleading and deceptive conduct relating to superannuation, insurance, managed funds, deposit accounts and credit. Includes undertaking enforcement such as administrative action, litigation or criminal action and referrals to other prosecution agencies or review bodies. Also includes the conduct of administrative hearings to review evidence and decisions." ;
    skos:inScheme :conceptScheme: ;
    skos:prefLabel "Investigation And Enforcement" .

:0350  a crs:Function, ra:Class,
        skos:Concept ;
    crs:isPerformedBy [ crs:hasAgent ca:8572 ] ;
    dct:source ras:2005-00516189 ;
    skos:definition "The function of providing scholarships and grants as part of the agency raising and maintaining its broad public profile." ;
    skos:inScheme :conceptScheme: ;
    skos:prefLabel "Community Relations (Scholarships)" .

:0351  a crs:Function, ra:Class,
        skos:Concept ;
    crs:isPerformedBy [ crs:hasAgent ca:8572 ] ;
    dct:source ras:2005-00516189 ;
    skos:definition "The function of managing enforcement action against entities and related parties under prudential regulation framework law. Includes undertaking enforcement action (including litigation), managing the case plan, developing appropriate procedures, exercising regulatory powers and referring appropriate matters to other enforcement agencies." ;
    skos:inScheme :conceptScheme: ;
    skos:prefLabel "Enforcement" .

:0352  a crs:Function, ra:Class,
        skos:Concept ;
    crs:isPerformedBy [ crs:hasAgent ca:8572 ] ;
    dct:source ras:2005-00516189 ;
    skos:definition "The function of establishing and maintaining formal and informal links with professional or industry groups, international or domestic associations and other regulators associated with the prudential industry. Includes committees or associations where the agency or its representatives are members, provision of services to overseas agencies, submissions to professional, industry, international or domestic associations or regulators and managing visits by overseas delegations who want to observe and learn about the Australian finance sector." ;
    skos:inScheme :conceptScheme: ;
    skos:prefLabel "Finance Sector Relations" .

:0353  a crs:Function, ra:Class,
        skos:Concept ;
    crs:isPerformedBy [ crs:hasAgent ca:8572 ] ;
    dct:source ras:2005-00516189 ;
    skos:definition "The function of managing all persons engaged by the organisation. Includes disclosures of interest." ;
    skos:inScheme :conceptScheme: ;
    skos:prefLabel "Human Resources" .

:0354  a crs:Function, ra:Class,
        skos:Concept ;
    crs:isPerformedBy [ crs:hasAgent ca:8572 ] ;
    dct:source ras:2005-00516189 ;
    skos:definition "The function of establishing courses of action and prudential requirements applicable to regulated entities that are developed under prudential regulation framework law. Includes: reviewing and developing policies; assisting the drafting and amendment of legislation and subordinate legislation, such as regulations and operating standards; and drafting, making and tabling other instruments, such as prudential standards, reporting standards, prudential rules and guidance notes. Also includes conducting research, consultation and answering enquiries related to these activities." ;
    skos:inScheme :conceptScheme: ;
    skos:prefLabel "Policy And Standards" .

:0355  a crs:Function, ra:Class,
        skos:Concept ;
    crs:isPerformedBy [ crs:hasAgent ca:8572 ],
        [ crs:hasAgent ca:8572 ] ;
    dct:source ras:2005-00516189 ;
    skos:definition """The function of supervising the prudent management of financial institutions under prudential regulation framework law. Includes the licensing, ongoing supervision and review of regulated entities
subject to prudential regulation, managing complaints about entities and exercising regulatory powers relating to prudential supervision. Also includes developing appropriate internal and external procedures and the provision of services that support prudential regulation.""",
        "The function of supervising the prudent management of financial institutions under prudential regulation framework law. Includes the licensing, ongoing supervision and review of regulated entities subject to prudential regulation, managing complaints about entities and exercising regulatory powers relating to prudential supervision. Also includes developing appropriate internal and external procedures and the provision of services that support prudential regulation." ;
    skos:inScheme :conceptScheme: ;
    skos:prefLabel "Prudential Supervision" .

:0356  a crs:Function, ra:Class,
        skos:Concept ;
    crs:isPerformedBy [ crs:hasAgent ca:8572 ] ;
    dct:source ras:2005-00516189 ;
    skos:definition """The function of having works published in international journals.
""";
    skos:inScheme :conceptScheme: ;
    skos:prefLabel "Publication (International)" .

:0357  a crs:Function, ra:Class,
        skos:Concept ;
    crs:isPerformedBy [ crs:hasAgent ca:8572 ] ;
    dct:source ras:2005-00516189 ;
    skos:definition "The function of collecting and analysing data under prudential regulation framework law. Includes the management of financial, economic and prudential statistics about reporting entities and related parties. Also includes managing secure data transfer." ;
    skos:inScheme :conceptScheme: ;
    skos:prefLabel "Statistics Management" .

:0358  a crs:Function, ra:Class,
        skos:Concept ;
    crs:isPerformedBy [ crs:hasAgent ca:8610 ],
        [ crs:hasAgent ca:8610 ] ;
    dct:source ras:2000-00000499,
        ras:2001-00000676 ;
    skos:definition " " ;
    skos:inScheme :conceptScheme: ;
    skos:prefLabel "Administrative Functions" .

:0359  a crs:Function, ra:Class,
        skos:Concept ;
    crs:isPerformedBy [ crs:hasAgent ca:8610 ] ;
    dct:source ras:2001-00000676 ;
    skos:definition "The function of providing governance to the Pig Research and Development Corporation" ;
    skos:inScheme :conceptScheme: ;
    skos:prefLabel "Corporate Governance" .

:0360  a crs:Function, ra:Class,
        skos:Concept ;
    crs:isPerformedBy [ crs:hasAgent ca:8610 ] ;
    dct:source ras:2000-00000499 ;
    skos:definition """The function of cooperating and liaising with other bodies to further the wool industry nationally and internationally. This includes bodies such as:
Federal and State Government departments (eg AFFA, DFAT, DISR);
Grower and industry peak bodies and organisations (eg. Wool Council);
Rural research organisations (eg. GRDC);
International organisations (eg. IWS, Wool producing country boards, International Wool Textile Organisation, World Trade Organisation, Asian Development Bank); and
Governments of other countries (eg. Korea, India).""";
    skos:inScheme :conceptScheme: ;
    skos:prefLabel "Industry Liaison" .

:0361  a crs:Function, ra:Class,
        skos:Concept ;
    crs:isPerformedBy [ crs:hasAgent ca:8610 ] ;
    dct:source ras:2001-00000524 ;
    skos:definition "The function of managing the marketing schemes for wool including the reserve price scheme and government initiated grower support schemes." ;
    skos:inScheme :conceptScheme: ;
    skos:prefLabel "Management Of Wool Marketing Schemes" .

:0362  a crs:Function, ra:Class,
        skos:Concept ;
    crs:isPerformedBy [ crs:hasAgent ca:8610 ] ;
    dct:source ras:2000-00000499 ;
    skos:definition "The gathering, analysis and dissemination of information and data on the global textile industry and international economies, including wool production, wool demand, textile processing, promotion, trade, trade barriers, and marketing in Australia and overseas. To identify trends in the global wool supply, processing and demand from raw wool production to retail demand. " ;
    skos:inScheme :conceptScheme: ;
    skos:prefLabel "Market Intelligence" .

:0363  a crs:Function, ra:Class,
        skos:Concept ;
    crs:isPerformedBy [ crs:hasAgent ca:8610 ] ;
    dct:source ras:2001-00000676 ;
    skos:definition "The function of managing funds on behalf of the Australian pig industry and the Commonwealth Government for the purposes on investing in research and development programs to improve the economic and environmental sustainability of the pig industry. Includes the adaptation of that research for practical and commercial uses. " ;
    skos:inScheme :conceptScheme: ;
    skos:prefLabel "Pig Research And Development" .

:0364  a crs:Function, ra:Class,
        skos:Concept ;
    crs:isPerformedBy [ crs:hasAgent ca:8610 ] ;
    dct:source ras:2000-00000499 ;
    skos:definition "The function of developing new or existing processes or products, after assessment and approval. Includes the technical work associated with the machinery, plant set up, fabric development, processing of wool involving staff expertise and collaboration with industry partnerships. " ;
    skos:inScheme :conceptScheme: ;
    skos:prefLabel "Product And Process Development" .

:0365  a crs:Function, ra:Class,
        skos:Concept ;
    crs:isPerformedBy [ crs:hasAgent ca:8610 ] ;
    dct:source ras:2000-00000499 ;
    skos:definition "Push and pull programs used to stimulate global consumer demands. These programs include a brand marketing strategy based on the Woolmark, consumer advertising campaigns and support for merchandising and joint retail promotions. The programs are directed at those directly involved in production, processing, manufacture and retail and at the general public. " ;
    skos:inScheme :conceptScheme: ;
    skos:prefLabel "Promotion" .

:0366  a crs:Function, ra:Class,
        skos:Concept ;
    crs:isPerformedBy [ crs:hasAgent ca:8610 ] ;
    dct:source ras:2000-00000499 ;
    skos:definition """The function of funding, and administering research into development of new processes, products and materials.
For the results or outcomes of research, use PRODUCT AND PROCESS DEVELOPMENT""";
    skos:inScheme :conceptScheme: ;
    skos:prefLabel "Research And Administration" .

:0367  a crs:Function, ra:Class,
        skos:Concept ;
    crs:isPerformedBy [ crs:hasAgent ca:8610 ] ;
    dct:source ras:2009-00097481 ;
    skos:definition """The business of managing research and development by the primary industry Research and Development Corporations (RDCs) established under the Primary Industries and Energy Research and Development Act 1989. The definition of primary industry in the Act includes industries involved in the production of agricultural or other primary produce, industries that extract minerals, extract energy or extract substances that provide energy from the environment and industries involved in the conservation and sustainable use and management of natural resources.

The role of the RDCs is to investigate and evaluate the requirements for research and development in primary industry. They use investigation and evaluation outcomes to set 5 year research and development plans that are subject to regular review and revision. Annual operational plans are developed, consistent with the 5 year plan.

The RDCs fund and coordinate research consistent with the annual operational plan by entering into agreements with research providers and brokering research by establishing joint ventures or collaborations. Joint ventures involve joint operations such as co-research or collaboration with other organisations, including government or private sector organisations, where there is a joint contribution of funds and/or time. The RDCs facilitate the dissemination, adoption and commercialisation of the results of research in the relevant primary industry. Managing the resulting intellectual property generated from research and licensing its use is an important part of the RDCs’ role. They monitor, evaluate and report to the Parliament, the Minister and its representative organisations on the research they fund and coordinate and its impact on the relevant primary industry.

This work includes the specific tasks of:
• giving and receiving advice
• negotiating and establishing agreements with research providers
• managing committees
• evaluating research and development needs for the relevant industry and evaluating research proposals
• managing joint venture arrangements with organisations
• liaising with the industry, Minister and representative organisations
• licensing the purchase of research outcomes
• planning research and development
• developing policies
• promoting research outcomes and making them accessible within the sector, a process known in the sector as extension
• reporting on the progress of research and on research outcomes
• representing the agency on sector committees
• administering contracted research
• receiving final research outcomes
• soliciting and evaluating research proposals from research providers
• reviewing research plans and programs
• making submissions.

The performance of the business is supported by routine administrative tasks such as:
• conducting audits
• authorising delegations of power to agency staff
• managing meetings
• receiving and responding to enquiries
• developing procedures.""";
    skos:inScheme :conceptScheme: ;
    skos:prefLabel "Research And Development Management" .

:0368  a crs:Function, ra:Class,
        skos:Concept ;
    crs:isPerformedBy [ crs:hasAgent ca:8610 ] ;
    dct:source ras:2001-00000524 ;
    skos:definition "The function of managing the marketing of wool to ensure quality of clip presented for sale to maximise grower payments." ;
    skos:inScheme :conceptScheme: ;
    skos:prefLabel "Wool Marketing Management" .

:0369  a crs:Function, ra:Class,
        skos:Concept ;
    crs:isPerformedBy [ crs:hasAgent ca:8615 ] ;
    dct:source ras:2005-00056212 ;
    skos:definition "The function of developing and establishing business and partnership relationships with community and service delivery organisations, academics, business leaders, consumer representatives and officials from three levels of government to help implement the delivery of the organisation's policies and programs to the community. Includes establishing, maintaining and reviewing business partnership agreements, memorandums of understanding, international social security, service level and grant funding agreements. Also includes conducting market research and analysis, receiving and responding to tenders with the aim of obtaining international consultancies for which remuneration is paid to the organisation. " ;
    skos:inScheme :conceptScheme: ;
    skos:prefLabel "Business Development" .

:0370  a crs:Function, ra:Class,
        skos:Concept ;
    crs:isPerformedBy [ crs:hasAgent ca:8615 ] ;
    dct:source ras:2005-00056212 ;
    skos:definition "The function of developing social welfare policies, programs and projects that are relevant to family and community functioning, economic and social participation. Includes providing advice, conducting research and evaluation activities, working with public and private sectors on joint ventures and hosting visits from international organisations. Also includes contracting-out research projects to external organisations. Also includes contracting-out research projects to external organisations." ;
    skos:inScheme :conceptScheme: ;
    skos:prefLabel "Social Welfare Development" .

:0371  a crs:Function, ra:Class,
        skos:Concept ;
    crs:isPerformedBy [ crs:hasAgent ca:8615 ],
        [ crs:hasAgent ca:8615 ] ;
    dct:source ras:2005-00056212,
        ras:2005-00669323 ;
    skos:definition "The function of providing social welfare services to the Australian community nationally and internationally. Includes the processes involved in assessing claimants' eligibility for welfare entitlements, preparing and paying benefits and allowances to eligible recipients, providing referrals to external bodies and counselling services, and conducting periodic circumstance, compliance and entitlement reviews of payments to recipients. Also includes investigating and identifying criminal activity and payment fraud, managing the processes involved in recovering legally recoverable payment and compensation debts, conducting outreach visits to ensure the community is aware of available welfare payments and related services, and joint ventures where there is a contract or joint contribution of funds andlor time." ;
    skos:inScheme :conceptScheme: ;
    skos:prefLabel "Social Welfare Services" .

:0372  a crs:Function, ra:Class,
        skos:Concept ;
    crs:isPerformedBy [ crs:hasAgent ca:8618 ] ;
    dct:source ras:2004-00616220 ;
    skos:definition "The function of developing and delivering regional and local government programs. Includes fostering partnerships among communities, government and the private sector to achieve sustainable regional development. Also includes facilitating programs, services and policies affecting rural, regional and remote Australia, together with granting financial assistance to state, territory and local governments and the public. " ;
    skos:inScheme :conceptScheme: ;
    skos:prefLabel "Regional Services Development And Local Government" .

:0373  a crs:Function, ra:Class,
        skos:Concept ;
    crs:isPerformedBy [ crs:hasAgent ca:8618 ] ;
    dct:source ras:2004-00616220 ;
    skos:definition "The function of providing advice and Commonwealth programs to the Territories. Includes agreements, appeals, ceremonies, liaison, planning, reporting and the coordination of resources for illegal immigrants. Also includes the review and amendment of legislation, including constitutional development. Excludes thet Australian Antarctic Territory. " ;
    skos:inScheme :conceptScheme: ;
    skos:prefLabel "Territory Policy And Development" .

:0374  a crs:Function, ra:Class,
        skos:Concept ;
    crs:isPerformedBy [ crs:hasAgent ca:8618 ] ;
    dct:source ras:2004-00616220 ;
    skos:definition "The provision of research, analysis and advice that influences policy decisions on transport and the environment.  Includes identification and measurement of the impact on the environment resulting from transport and transport infrastructure.  Also includes the development and analysis of policy to reduce the impact of the Australian transport sector on the environment and the promotion of ecologically sustainable transport development principles." ;
    skos:inScheme :conceptScheme: ;
    skos:prefLabel "Transport Environment Management" .

:0375  a crs:Function, ra:Class,
        skos:Concept ;
    crs:isPerformedBy [ crs:hasAgent ca:8618 ] ;
    dct:source ras:2004-00616220 ;
    skos:definition "The function of providing funding for capital development of Australia's hard and soft transport infrastructure network. Includes the provision of expert advice to Government and the community and improving the understanding of economic factors influencing the transport sector. Also includes trade facilitation and participation in international forums. " ;
    skos:inScheme :conceptScheme: ;
    skos:prefLabel "Transport Infrastructure Development" .

:0376  a crs:Function, ra:Class,
        skos:Concept ;
    crs:isPerformedBy [ crs:hasAgent ca:8618 ] ;
    dct:source ras:2004-00616220 ;
    skos:definition "The function of investigating, researching and analysing safety data for all marine, aviation, rail and road transport modes, to identify and monitor transport safety issues. Includes independent investigation of transport related accidents, incidents and safety deficiencies, and the dissemination of investigation findings and recommendations for improvements to transport safety. Also includes advising on policy decisions that influence transport safety; liaision with authorities and other bodies to develop safety recommendations; and providing transport safety related information to stakeholders and the public. " ;
    skos:inScheme :conceptScheme: ;
    skos:prefLabel "Transport Safety" .

:0377  a crs:Function, ra:Class,
        skos:Concept ;
    crs:isPerformedBy [ crs:hasAgent ca:8618 ] ;
    dct:source ras:2004-00616220 ;
    skos:definition "The function of providing advice, policy and the regulating of transport industry and services. Covers the licensing of facilities and activities for all modes of transport, which includes aviation, rail, maritime and road transport. Includes the provision of transport permits, compliance with design rules, and oversight of Australia's transport security environment. " ;
    skos:inScheme :conceptScheme: ;
    skos:prefLabel "Transport Services And Regulations" .

:0378  a crs:Function, ra:Class,
        skos:Concept ;
    crs:isPerformedBy [ crs:hasAgent ca:8869 ] ;
    dct:source ras:2003-00330307 ;
    skos:definition "The function of implementing labour market programs. Includes managing and coordinating the delivery of employment services and assistance to job seekers; administering the provision of grants and programs to assist targeted groups in the community, such as Indigenous Australians and disadvantaged job seekers; and liaising with local communities. " ;
    skos:inScheme :conceptScheme: ;
    skos:prefLabel "Employment Services" .

:0379  a crs:Function, ra:Class,
        skos:Concept ;
    crs:isPerformedBy [ crs:hasAgent ca:8869 ] ;
    dct:source ras:2004-00666919 ;
    skos:definition "The function of developing policy and providing advice in relation to employment, wages and the effective operation of the labour market. Supported by research, analysis, evaluation and promotion of the labour market. Includes trends in labour demand and supply, trends in enterprise bargaining, wages issues and the role of the awards system, transitions into and out of the labour market, the transition from welfare to work, evaluation of the labour market programs and services, and the development of information and promotional material intended to improve labour market efficiency.  " ;
    skos:inScheme :conceptScheme: ;
    skos:prefLabel "Labour Market Development" .

:0380  a crs:Function, ra:Class,
        skos:Concept ;
    crs:isPerformedBy [ crs:hasAgent ca:8869 ] ;
    dct:source ras:2004-00666919 ;
    skos:definition "The functiion of establishing a workplace relations framework to achieve flexible and fair workplace relations for organisations. Includes developing policies, strategies, programs, advising government, research and analysis of workplace relations trends and practices. Also includes the department's involvement with international organisations including the International Labour Organisation (ILO) and Asia-Pacific Economic Co-operation (APEC).  " ;
    skos:inScheme :conceptScheme: ;
    skos:prefLabel "Workplace Relations Development" .

:0381  a crs:Function, ra:Class,
        skos:Concept ;
    crs:isPerformedBy [ crs:hasAgent ca:8869 ] ;
    dct:source ras:2004-00666919 ;
    skos:definition "The function of implementing workplace relations programs and providing enquiry and information services to assist employers and employees to understand their rights and responsibilities under workplace relations legislation, such as the Workplace Relations Act, federal awards and certified agreements. Includes compliance, advocacy, education and training services. " ;
    skos:inScheme :conceptScheme: ;
    skos:prefLabel "Workplace Relations Services" .

:0382  a crs:Function, ra:Class,
        skos:Concept ;
    crs:isPerformedBy [ crs:hasAgent ca:8871 ] ;
    dct:source ras:2007-00307997 ;
    skos:definition """The function of developing, implementing and monitoring standards and regulations impacting on the Australian building industry.  Includes liaison with industry and Commonwealth, State and Territory governments.
""";
    skos:inScheme :conceptScheme: ;
    skos:prefLabel "Building Code Development" .

:0383  a crs:Function, ra:Class,
        skos:Concept ;
    crs:isPerformedBy [ crs:hasAgent ca:8871 ] ;
    dct:source ras:2007-00307997 ;
    skos:definition "The function of facilitating and providing Australian businesses with a single point of access to aggregated information from all levels of Government in Australia to assist them to plan, start and run their businesses.  Includes access through online services; the aggregation and syndication of content; the development and management of websites; liaison and consultation with industry; and marketing." ;
    skos:inScheme :conceptScheme: ;
    skos:prefLabel "Business Information Access" .

:0384  a crs:Function, ra:Class,
        skos:Concept ;
    crs:isPerformedBy [ crs:hasAgent ca:8871 ] ;
    dct:source ras:2007-00307997 ;
    skos:definition "The function of developing policies for the sustainable use and management of energy and mineral resources (fossil fuels, renewable energy sources and minerals), and associated infrastructure.  Includes: the development and maintenance of the regulatory framework applicable to the use and exploitation of energy and mineral resources; administering programs to evaluate resource consumption and exploitation practices; and regulating and supporting industries that realise the economic potential of energy and mineral resources.  Also includes the development and administration of legislation and regulations; the granting of licences, leases and permits; oversight of exploration and mapping activities; the promotion of industry partnerships including with traditional owners; liaising and negotiating in international arenas; research; monitoring compliance with standards, regulations and risk management procedures; and land rehabilitation and environmental issues." ;
    skos:inScheme :conceptScheme: ;
    skos:prefLabel "Energy And Mineral Resources" .

:0385  a crs:Function, ra:Class,
        skos:Concept ;
    crs:isPerformedBy [ crs:hasAgent ca:8871 ] ;
    dct:source ras:2007-00307997 ;
    skos:definition """The function of attracting foreign business investment in Australia. Includes: the development and implementation of policies, strategies and programs; liaison with State and Territory governments; the promotion of Australia as an attractive location for investment; specialist investment services such as the facilitation of major projects; advice on investment opportunities; the management of investment leads; the analysis of investment proposals; benchmarking studies; and grant funding.
""";
    skos:inScheme :conceptScheme: ;
    skos:prefLabel "Foreign Investment Attraction" .

:0386  a crs:Function, ra:Class,
        skos:Concept ;
    crs:isPerformedBy [ crs:hasAgent ca:8871 ] ;
    dct:source ras:2007-00307997 ;
    skos:definition "The function of formulating policy to regulate and support the private sector, including small business.  Includes the development of strategies to foster innovation and growth in business and industry and the provision of assistance to industry through a range of measures including advisory services, entitlements, grants, funding and subsidies.  Also includes industry development, industry assistance schemes, small business services, business sponsorship, regulatory reform and collaboration with industry and government bodies within Australia and overseas." ;
    skos:inScheme :conceptScheme: ;
    skos:prefLabel "Industry Support And Development" .

:0387  a crs:Function, ra:Class,
        skos:Concept ;
    crs:isPerformedBy [ crs:hasAgent ca:8871 ] ;
    dct:source ras:2007-00307997 ;
    skos:definition """The function of ensuring the quality and continuous improvement of laboratory processes, products and services to meet performance requirements and adhere to relevant industry standards.  Includes the identification, development, implementation, management and evaluation of strategies and programs designed to ensure the organisation remains accredited or certified to industry standards.
""";
    skos:inScheme :conceptScheme: ;
    skos:prefLabel "Laboratory Quality Management" .

:0388  a crs:Function, ra:Class,
        skos:Concept ;
    crs:isPerformedBy [ crs:hasAgent ca:8871 ] ;
    dct:source ras:2007-00307997 ;
    skos:definition """The function of developing the organisation's commercial opportunities relating to metrological services. Includes contracts and agreements for all research, and technology transfer arrangements and confidentiality agreements other than with personnel.
""";
    skos:inScheme :conceptScheme: ;
    skos:prefLabel "Metrological Business Development" .

:0389  a crs:Function, ra:Class,
        skos:Concept ;
    crs:isPerformedBy [ crs:hasAgent ca:8871 ] ;
    dct:source ras:2007-00307997 ;
    skos:definition "The function of developing and maintaining the national metrology infrastructure and ensuring harmonisation with international metrology infrastructure.  Includes the definition of scientific and Australian legal units of measurement; the development and maintenance of legislation; the development of documentary standards; the appointment of legal metrology authorities; liaison and consultation with the Australian and international standards and conformance infrastructure, industry, government and overseas organisations; participation in and support for international treaties and agreements; management of visits by national and international visitors." ;
    skos:inScheme :conceptScheme: ;
    skos:prefLabel "Metrological Coordination" .

:0390  a crs:Function, ra:Class,
        skos:Concept ;
    crs:isPerformedBy [ crs:hasAgent ca:8871 ] ;
    dct:source ras:2007-00307997 ;
    skos:definition "The function of providing physical, biological and chemical metrological services. Includes the development of analytical methods, tests and procedures, including measurements and calibration of metrological instruments; analytical services, including analysis of samples and testing of instruments; consulting and training services; the issuing of certificates under trade measurement legislation; proficiency testing; pattern approval, testing and compliance. " ;
    skos:inScheme :conceptScheme: ;
    skos:prefLabel "Metrological Services" .

:0391  a crs:Function, ra:Class,
        skos:Concept ;
    crs:isPerformedBy [ crs:hasAgent ca:8871 ] ;
    dct:source ras:2007-00307997 ;
    skos:definition """The function of receiving, registering, storing and maintaining micro-organism samples in line with the requirements of the Budapest Treaty on the International Recognition of the Deposit of Microorganisms for the Purposes of Patent Procedure.  Includes liaison with other government agencies and international organisations; the receipt, registration and storage of micro-organism samples; the transfer of a micro-organism sample to another depositary authority; and the disposal of micro-organism samples.
""";
    skos:inScheme :conceptScheme: ;
    skos:prefLabel "Microorganism Collection" .

:0392  a crs:Function, ra:Class,
        skos:Concept ;
    crs:isPerformedBy [ crs:hasAgent ca:8871 ] ;
    dct:source ras:2007-00307997 ;
    skos:definition """The function of managing science buildings, which have been purpose built and have unique or specialised design features.
""";
    skos:inScheme :conceptScheme: ;
    skos:prefLabel "Property Management (Special Buildings)" .

:0393  a crs:Function, ra:Class,
        skos:Concept ;
    crs:isPerformedBy [ crs:hasAgent ca:8871 ] ;
    dct:source ras:2007-00307997 ;
    skos:definition "The function of investigating or enquiring into a subject or area of interest to discover facts and principles.  Includes the development of projects, measurement standards and guidelines; international comparisons of measurement standards; liaison between scientists; meetings to discuss technical issues and unpublished technical papers; scientific conferences; and the design and construction of mechanical, technical and electronic equipment to support the organisation's business activities." ;
    skos:inScheme :conceptScheme: ;
    skos:prefLabel "Scientific Research" .

:0394  a crs:Function, ra:Class,
        skos:Concept ;
    crs:isPerformedBy [ crs:hasAgent ca:8871 ] ;
    dct:source ras:2001-00000782 ;
    skos:definition "Development and management of the Snowy Mountains Hydro-electric Scheme." ;
    skos:inScheme :conceptScheme: ;
    skos:prefLabel "Snowy Mountains Hydro-Electric Scheme" .

:0395  a crs:Function, ra:Class,
        skos:Concept ;
    crs:isPerformedBy [ crs:hasAgent ca:8871 ] ;
    dct:source ras:2007-00307997 ;
    skos:definition "The function of ensuring Australian (civilian) space activities are conducted in a safe and accountable manner. Includes legislative changes and recognition arrangements; administering space licences, launch permits, return authorisations and overseas launch certificates; monitoring the safety of space related activities; investigating accidents and incidents; and maintaining the Australian register of space objects." ;
    skos:inScheme :conceptScheme: ;
    skos:prefLabel "Space Licensing And Safety" .

:0396  a crs:Function, ra:Class,
        skos:Concept ;
    crs:isPerformedBy [ crs:hasAgent ca:8871 ] ;
    dct:source ras:2007-00307997 ;
    skos:definition "The function of producing predictions of space weather based on observations of the sun, the ionosphere and the earth.  Includes: solar, ionospheric and geomagnetic observation; space weather predictions based on those observations; the giving of advice and external training to people, bodies and organisations that use high frequency (HF) radio systems; the development, promotion and sale of software; international collaboration; and external consulting services for the management of radio, geophysical and space systems." ;
    skos:inScheme :conceptScheme: ;
    skos:prefLabel "Space Weather Prediction" .

:0397  a crs:Function, ra:Class,
        skos:Concept ;
    crs:isPerformedBy [ crs:hasAgent ca:8871 ] ;
    dct:source ras:2007-00307997 ;
    skos:definition """The function of developing policies and programs to foster the development of the tourism industry. Includes the development and implementation of long term strategies for tourism development; encouraging Australian and international partnerships and coordinating initiatives to optimise tourism employment and create a favourable environment for investment; the coordination across jurisdictions on tourism projects; the recognition of excellence in the tourism industry; and the provision of grants, sponsorships and funding.
""";
    skos:inScheme :conceptScheme: ;
    skos:prefLabel "Tourism" .

:0398  a crs:Function, ra:Class,
        skos:Concept ;
    crs:isPerformedBy [ crs:hasAgent ca:8926 ] ;
    dct:source ras:2003-00288428 ;
    skos:definition "The function of establishing, developing and managing relationships with national and international contacts, clients and investors, monitoring developments in the food industry and increasing the awareness of the available technologies, representation an" ;
    skos:inScheme :conceptScheme: ;
    skos:prefLabel "Business Relations" .

:0399  a crs:Function, ra:Class,
        skos:Concept ;
    crs:isPerformedBy [ crs:hasAgent ca:8926 ] ;
    dct:source ras:2003-00288428 ;
    skos:definition "The function of determining the objectives, strategies and policies of the organisation and undertaking activities to ensure that the organisation carries out its functions properly, efficiently and effectively. Includes activities associated with providi" ;
    skos:inScheme :conceptScheme: ;
    skos:prefLabel "Corporate Governance" .

:0400  a crs:Function, ra:Class,
        skos:Concept ;
    crs:isPerformedBy [ crs:hasAgent ca:8926 ] ;
    dct:source ras:2003-00288428 ;
    skos:definition "The function of managing the Joint Venture employees of the respective parent organisations employed as either CSIRO employees under the Science and Industry Act 1949, CSIRO Terms & Conditions of Employment, and CSIRO Enterprise Agreement 2001, or as Afis" ;
    skos:inScheme :conceptScheme: ;
    skos:prefLabel "Joint Venture Personnel" .

:0401  a crs:Function, ra:Class,
        skos:Concept ;
    crs:isPerformedBy [ crs:hasAgent ca:8926 ] ;
    dct:source ras:2003-00288428 ;
    skos:definition "The function of undertaking original scientific investigations, experimentation and theoretical, innovative development or systematic work aimed at the creation of new knowledge, and the application of this knowledge to new or improved practices, products" ;
    skos:inScheme :conceptScheme: ;
    skos:prefLabel "Research And Development" .

:0402  a crs:Function, ra:Class,
        skos:Concept ;
    crs:isPerformedBy [ crs:hasAgent ca:8926 ] ;
    dct:source ras:2003-00288428 ;
    skos:definition "The function of providing overall management of and strategic direction to the organisation’s research and development, technical and consulting services, and scientific support functions. Also includes formulating and reviewing project management discipl" ;
    skos:inScheme :conceptScheme: ;
    skos:prefLabel "Science Management" .

:0403  a crs:Function, ra:Class,
        skos:Concept ;
    crs:isPerformedBy [ crs:hasAgent ca:8926 ] ;
    dct:source ras:2003-00288428 ;
    skos:definition "The function of providing specialist resources to support science programs. Includes the acquisition, marketing and management of collections of data or specimens for on-going reference purposes and the recruitment and maintenance of trained sensory panel" ;
    skos:inScheme :conceptScheme: ;
    skos:prefLabel "Science Support" .

:0404  a crs:Function, ra:Class,
        skos:Concept ;
    crs:isPerformedBy [ crs:hasAgent ca:8926 ] ;
    dct:source ras:2003-00288428 ;
    skos:definition "The function of providing clients with technical services, consultation and professional training. Technical services are narrowly focused projects with routinely achievable outcomes requiring no original research and development or the creation of intell" ;
    skos:inScheme :conceptScheme: ;
    skos:prefLabel "Technical And Consulting Services" .

:0405  a crs:Function, ra:Class,
        skos:Concept ;
    crs:isPerformedBy [ crs:hasAgent ca:8929 ] ;
    dct:source ras:2007-00440378 ;
    skos:definition "The function of establishing and implementing processes that support service delivery to payers and clients. Includes service accreditation, standards, acquisition of service providers, quality assurance and improvement, community liaison, identification and development of new markets and related services and liaison with service payers such as government agencies and private businesses." ;
    skos:inScheme :conceptScheme: ;
    skos:prefLabel "Service Development And Support" .

:0406  a crs:Function, ra:Class,
        skos:Concept ;
    crs:isPerformedBy [ crs:hasAgent ca:8929 ] ;
    dct:source ras:2007-00440378 ;
    skos:definition """The function of delivering services to people with a disability, injury or health condition, to manage their condition and utilise their abilities so as to obtain or keep work and enhance their personal skills and ability to participate in community life. Includes delivery of services such as vocational and occupational
rehabilitation, disability management, injury prevention and management and assessments relating to job capacity, independent living and wage levels.""";
    skos:inScheme :conceptScheme: ;
    skos:prefLabel "Vocational Rehabilitation, Disability And Injury Management" .

:0407  a crs:Function, ra:Class,
        skos:Concept ;
    crs:isPerformedBy [ crs:hasAgent ca:8981 ] ;
    dct:source ras:2007-00210158 ;
    skos:definition "The function of managing the Parliament House Construction Authority. Includes Board meetings, appointments and remuneration." ;
    skos:inScheme :conceptScheme: ;
    skos:prefLabel "Board Management" .

:0408  a crs:Function, ra:Class,
        skos:Concept ;
    crs:isPerformedBy [ crs:hasAgent ca:8981 ] ;
    dct:source ras:2007-00210158 ;
    skos:definition """The function of designing, constructing and maintaining Parliament House and its surrounds. Includes the development and implementation of the maintenance program, preservation of the design, and management of the building structure, fabric, and landscape. Includes construction and design management processes, maintenance of electrical components, the plant and equipment, fabric services, mechanical services (hydraulic services, air quality systems, main flag operations), the maintenance of the gardens, plant control and chemical storage. Also includes the design competition of both the provisional and new Parliament Houses and the strategic planning focused on future requirements of the building design integrity, furnishing and furniture integrity and sustainability and on
engineering services critical to the building's long-term operability.""";
    skos:inScheme :conceptScheme: ;
    skos:prefLabel "Building And Design Management" .

:0409  a crs:Function, ra:Class,
        skos:Concept ;
    crs:isPerformedBy [ crs:hasAgent ca:8981 ] ;
    dct:source ras:2007-00210158 ;
    skos:definition "The function of providing and managing a range of services and facilities for Senators, Members and Parliament House occupants, staff and visitors. Includes catering, cleaning, retail services, visitor services, material distribution, storage and waste removal. Also includes facilitating events at Parliament House." ;
    skos:inScheme :conceptScheme: ;
    skos:prefLabel "Business And Facility Services" .

:0410  a crs:Function, ra:Class,
        skos:Concept ;
    crs:isPerformedBy [ crs:hasAgent ca:8981 ] ;
    dct:source ras:2007-00210158 ;
    skos:definition """The function of acquiring, preserving, controlling, developing and promoting the commissioned works, general art collection, gifts and historic memorials collection of Parliament House. Includes providing
access to works for display in Parliament House and Parliamentary precincts, reproduction and contributing to national arts activities.""";
    skos:inScheme :conceptScheme: ;
    skos:prefLabel "Collection Management" .

:0411  a crs:Function, ra:Class,
        skos:Concept ;
    crs:isPerformedBy [ crs:hasAgent ca:8981 ] ;
    dct:source ras:2007-00210158 ;
    skos:definition "The function of providing health and recreation services to Senators, Members, staff, occupants and visitors of Parliament House. Includes first aid and emergency medical services, fitness programs and health promotion." ;
    skos:inScheme :conceptScheme: ;
    skos:prefLabel "Health And Recreation Services" .

:0412  a crs:Function, ra:Class,
        skos:Concept ;
    crs:isPerformedBy [ crs:hasAgent ca:8981 ] ;
    dct:source ras:2008-00533770 ;
    skos:definition """The activities associated with providing information, analysis and advisory services to Senators and Members of Parliament and their staff (clients). Clients can request information, research and/or analysis on any topic. Depending on the request, responses range from a link to an internet site or a list of contact details (eg a list of newspapers in an electoral area), to detailed research and analysis providing policy advice or an understanding or analysis of a subject. The confidentiality of the client, and any confidential information provided by the client is protected. However, published or publishable information that is used for one response may also be used for another where another client asks the same or similar question, or may be used to form the basis of a more general brief or publication.
The tasks associated with the information, analysis and advisory services business include:
• receive and provide tailored responses to requests for information, including acknowledgements of requests
• correspondence regarding the status of research and manage/track responses
• research and analyse a subject and provide reports, and/or advice, including an independent perspective on government legislation
• develop and present briefing products and seminars on major issues
• train clients in accessing services, tools and resources
• conduct and evaluate client surveys provided by the agency
• manage complaints and compliments
• support fellowship recipients
• research and develop official historical publications and oral histories commissioned or produced by the agency for significant events or on subjects to enhance the knowledge and understanding
of Australia's parliamentary history
• plan and conduct audits
• review programs, products, processes and practices
• develop policy, procedures, working tools and subject files.""";
    skos:inScheme :conceptScheme: ;
    skos:prefLabel "Information, Analysis And Advisory Services" .

:0413  a crs:Function, ra:Class,
        skos:Concept ;
    crs:isPerformedBy [ crs:hasAgent ca:8981 ] ;
    dct:source ras:2007-00210158 ;
    skos:definition "The function of managing the receipt of awards to Parliament House or awards received by the department." ;
    skos:inScheme :conceptScheme: ;
    skos:prefLabel "Parliamentary Awards" .

:0414  a crs:Function, ra:Class,
        skos:Concept ;
    crs:isPerformedBy [ crs:hasAgent ca:8981 ] ;
    dct:source ras:2007-00545420 ;
    skos:definition "The function of broadcasting and reporting Parliamentary proceedings and events. This includes Hansard transcripts of proceedings in the House of Representatives, the Senate and the Main Committee of the House of Representatives; Hansard transcripts of hearings of parliamentary committees; internal and external television and radio broadcasts of proceedings and audiovisual recordings. The function also includes the audiovisual recordings of special events at Parliament House, recordings requested by Members of Parliament and Senators for their personal use, the provision of audiovisual services to clients, such as Members of Parliament and Senators, and the transcription of some parliament-related conferences." ;
    skos:inScheme :conceptScheme: ;
    skos:prefLabel "Parliamentary Broadcasting And Hansard" .

:0415  a crs:Function, ra:Class,
        skos:Concept ;
    crs:isPerformedBy [ crs:hasAgent ca:8981 ] ;
    dct:source ras:2007-00210158 ;
    skos:definition "The function of managing the professional indemnity insurance requirements of Parliament House and Parliamentary departments. Includes arranging insurance cover and managing insurance claims." ;
    skos:inScheme :conceptScheme: ;
    skos:prefLabel "Parliamentary Insurance" .

:0416  a crs:Function, ra:Class,
        skos:Concept ;
    crs:isPerformedBy [ crs:hasAgent ca:8981 ] ;
    dct:source ras:2007-00210158 ;
    skos:definition "The function of developing, planning and managing security and emergency arrangements at Parliament House and its environment, to protect property and occupants, including Parliamentary members, dignitaries and visitors. Includes acquisition, installation and maintenance of security equipment, implementing advice received from security management bodies, management of contracts with protective service officers, liaising with emergency and police services, and management of security breaches and security controls." ;
    skos:inScheme :conceptScheme: ;
    skos:prefLabel "Parliamentary Protection" .

:0417  a crs:Function, ra:Class,
        skos:Concept ;
    crs:isPerformedBy [ crs:hasAgent ca:9004 ] ;
    dct:source ras:2009-00000482 ;
    skos:definition "The function of delivering services to separated parents to enable the transfer of payments for the benefit of their children. Includes registration, assessment, collection and transfer of payments and the development of guidelines and procedures. Also includes referring parents to other services, processing objections to child support decisions and following up on complaints relating to service delivery." ;
    skos:inScheme :conceptScheme: ;
    skos:prefLabel "Child Support" .

:0418  a crs:Function, ra:Class,
        skos:Concept ;
    crs:isPerformedBy [ crs:hasAgent ca:9019 ] ;
    dct:source ras:2007-00122120 ;
    skos:definition "The function of managing the governance framework and strategic direction of the agency. Includes providing advice, authorising the funding of projects, taking of board minutes, arranging board members travel, allowances and expenses to be paid, and evaluating and monitoring performance of  the board. The function of managing the governance framework and strategic direction of the agency. Includes providing advice, authorising the funding of projects, taking of board minutes, arranging board members travel, allowances and expenses to be paid, and evaiuating and monitoring performance of the board." ;
    skos:inScheme :conceptScheme: ;
    skos:prefLabel "Board Management" .

:0419  a crs:Function, ra:Class,
        skos:Concept ;
    crs:isPerformedBy [ crs:hasAgent ca:9019 ] ;
    dct:source ras:2007-00122120 ;
    skos:definition "The function of providing policing information services to meet the needs of operational policing, justice administration and third parties, such as accredited external agencies. Includes negotiating, establishing and maintaining agreements for information services, and providing record checking services for accredited agencies. Includes arranging meetings and conferences held by the organisation to support the function. Includes the review of systems and processes used to support the delivery and exchange of information services, developing costing models for the delivery of these services, and processing applications for accreditation, distribution of products and provision of agency specific training." ;
    skos:inScheme :conceptScheme: ;
    skos:prefLabel "Policing Information Services" .

:0420  a crs:Function, ra:Class,
        skos:Concept ;
    crs:isPerformedBy [ crs:hasAgent ca:9095 ] ;
    dct:source ras:2007-00268385 ;
    skos:definition "The function of managing assets and liabilities for the purpose of managing the Australian Government's net Commonwealth government securities (CGS) debt. Includes issuing and redeeming debt in the form of Commonwealth government securities, managing the overall level of cash in the Australian Government's official public account, managing assets on the organisation's balance sheet, execution of financial derivatives in the form of interest rate swap transactions, managing associated risks and liaising with investors and financial market participants to monitor financial markets conditions." ;
    skos:inScheme :conceptScheme: ;
    skos:prefLabel "Asset And Liability Management" .

:0421  a crs:Function, ra:Class,
        skos:Concept ;
    crs:isPerformedBy [ crs:hasAgent ca:9095 ] ;
    dct:source ras:2007-00268385 ;
    skos:definition "The function of providing investment services to client agencies. Includes executing investment transactions, managing those investments in accordance with investment policies, liaising with investors and financial market participants to monitor financial markets conditions and administering supporting arrangements such as investment dealer panels and investment committees." ;
    skos:inScheme :conceptScheme: ;
    skos:prefLabel "Client Investment Services" .

:0422  a crs:Function, ra:Class,
        skos:Concept ;
    crs:isPerformedBy [ crs:hasAgent ca:9126 ],
        [ crs:hasAgent ca:9126 ] ;
    dct:source ras:2006-00374098,
        ras:2006-00444996 ;
    skos:definition "The function of promoting a culture that respects privacy principles and rights and obligations under privacy legislation, in Australian society. Includes activities to increase knowledge and understanding, such as giving addresses, and developing and conducting educational programs. Also includes establishing and maintaining media relations." ;
    skos:inScheme :conceptScheme: ;
    skos:prefLabel "Privacy Awareness And Education" .

:0423  a crs:Function, ra:Class,
        skos:Concept ;
    crs:isPerformedBy [ crs:hasAgent ca:9126 ] ;
    dct:source ras:2006-00374098 ;
    skos:definition "The function of monitoring, and taking action to ensure compliance with statutory obligations under privacy legislation and other relevant legislation administered by the agency. Includes investigating complaints lodged by individuals about interferences with their privacy, attempting to resolve complaints by conciliation, and where appropriate making enforceable determinations in relation to compiaints, conducting investigations, initiated by the agency, of possible breaches of privacy and associated legisiation, and undertaking compliance audits to ensure that individuals, agencies or organisations comply with the requirements of privacy and related legislation. Also includes compiling and arranging for publication records of personal information held by Australian government agencies and maintaining a register of smail business operators who have.chosen to be treated as organisations." ;
    skos:inScheme :conceptScheme: ;
    skos:prefLabel "Privacy Compliance" .

:0424  a crs:Function, ra:Class,
        skos:Concept ;
    crs:isPerformedBy [ crs:hasAgent ca:9126 ] ;
    dct:source ras:2006-00374098 ;
    skos:definition "The function of monitoring and analysing developments in privacy policy, and providing privacy related advice and guidance to ministers, agencies, organisations and individuals, in order to avoid adverse effects on the privacy of individuals. Includes the preparation of guidelines that enable agencies or organisations to comply with privacy principles, approving privacy codes, making submissions to parliament and other inquiries, and reporting to the Minister on any legisiative or administrative action needed to protect the privacy interests of individuals." ;
    skos:inScheme :conceptScheme: ;
    skos:prefLabel "Privacy Policy Development And Legislative Review" .

:0425  a crs:Function, ra:Class,
        skos:Concept ;
    crs:isPerformedBy [ crs:hasAgent ca:9128 ] ;
    dct:source ras:2006-00374066 ;
    skos:definition "The function of managing the national procurement of blood, blood products and services. Includes the tendering for products and services, the negotiation, establishment and review of procurement contracts, management of contracts including the handling of complaints, and the assessment of submissions from suppliers." ;
    skos:inScheme :conceptScheme: ;
    skos:prefLabel "Blood Procurement Management" .

:0426  a crs:Function, ra:Class,
        skos:Concept ;
    crs:isPerformedBy [ crs:hasAgent ca:9128 ] ;
    dct:source ras:2006-00374066 ;
    skos:definition "The function of providing secretariat services to, and managing the activities of, the agency's advisory Board and its appointed members. Includes the administration of Board meetings, documenting the appointments and termination of Board members, and the management of Board members' leave, remuneration and allowances" ;
    skos:inScheme :conceptScheme: ;
    skos:prefLabel "Board Management" .

:0427  a crs:Function, ra:Class,
        skos:Concept ;
    crs:isPerformedBy [ crs:hasAgent ca:9128 ] ;
    dct:source ras:2006-00374066 ;
    skos:definition "The function of developing and utilising strategies to reduce the demand for blood, blood products and services. Includes research and investigation of current and emerging best practice, clinical use benchmarking and guideline development and implementation, developing projects that will support the States and Territories in improving the appropriate use of blood and blood products and educating stakeholders through professional and community forums." ;
    skos:inScheme :conceptScheme: ;
    skos:prefLabel """Demand Management
""".

:0428  a crs:Function, ra:Class,
        skos:Concept ;
    crs:isPerformedBy [ crs:hasAgent ca:9128 ] ;
    dct:source ras:2006-00374066 ;
    skos:definition "The function of managing the compensation scheme relating to indemnity claims in respect of diseases transmitted by blood and blood products within Australia. Includes agreements between the parties contributing to the scheme and tendering out the case management of the scheme." ;
    skos:inScheme :conceptScheme: ;
    skos:prefLabel "National Managed Fund" .

:0429  a crs:Function, ra:Class,
        skos:Concept ;
    crs:isPerformedBy [ crs:hasAgent ca:9128 ] ;
    dct:source ras:2006-00374066 ;
    skos:definition "The function of planning and managing the national supply of blood products. Includes the collection and analysis of product usage data, the preparation of the annual supply plan and budget, and the management of supply problems and other blood related incidents." ;
    skos:inScheme :conceptScheme: ;
    skos:prefLabel "Supply Planning And Management" .

:0430  a crs:Function, ra:Class,
        skos:Concept ;
    crs:isPerformedBy [ crs:hasAgent ca:9135 ] ;
    dct:source ras:2006-00435306 ;
    skos:definition "The function of regulating Australia's personal insolvency system in accordance with bankruptcy legislation. Includes representing the agency where appeals against its decision are made, handling complaints against trustees, conducting reviews of trustees' decisions, attending meetings of creditors and conducting investigations into the financial affairs of bankrupts. Also includes inspecting records of trustees and debt agreement administrators, managing the process of registering trustees and determining whether trustees and debt agreement administrators are eligible to act." ;
    skos:inScheme :conceptScheme: ;
    skos:prefLabel "Bankruptcy Regulation" .

:0431  a crs:Function, ra:Class,
        skos:Concept ;
    crs:isPerformedBy [ crs:hasAgent ca:9135 ] ;
    dct:source ras:2006-00435306 ;
    skos:definition "The function of exercising official trustee powers by managing moneys on behalf of administered estates in an authorised deposit-taking institution account known as a common investment fund. Includes establishing, monitoring and maintaining bank accounts in each bankruptcy district. Also includes receipting, depositing and paying moneys into and from these accounts, investment of moneys held in the fund, payment of interest earned in consolidated revenue and reporting fund activity to the head of the agency and other stakeholders." ;
    skos:inScheme :conceptScheme: ;
    skos:prefLabel "Common Fund Management" .

:0432  a crs:Function, ra:Class,
        skos:Concept ;
    crs:isPerformedBy [ crs:hasAgent ca:9135 ] ;
    dct:source ras:2006-00435306 ;
    skos:definition "The function of dealing with matters alleging fraudulent and criminal activity by individuals or organisations external to the agency. Includes assessing referrals of alleged fraud and conducting investigations of offences under the relevant legislation (eg the Bankruptcy Act, the Commonwealth Crimes Act and the Criminal Code). Also includes liaising with other agencies, executing search warrants, finalising matters, recovering money or property and preparing submissions." ;
    skos:inScheme :conceptScheme: ;
    skos:prefLabel "Fraud Investigation" .

:0433  a crs:Function, ra:Class,
        skos:Concept ;
    crs:isPerformedBy [ crs:hasAgent ca:9135 ] ;
    dct:source ras:2006-00435306 ;
    skos:definition "The function of exercising official receiver powers to assist trustees in the administration of personal insolvency matters under their control. Activities include authorising access to premises and books, giving addresses (presentations), assessing documents presented for filing, processing debt agreements, responding to enquiries for information including national personal insolvency index searches and public file access, conducting examinations, assessing hardship applications, issuing bankruptcy notices and other statutory notices, dealing with reaction from the public such as complaints and compliments, acceptance and registration of documents in the agencies local database and the national personal insolvency index, remuneration reviews and taking inventories." ;
    skos:inScheme :conceptScheme: ;
    skos:prefLabel "Official Receiver Administration" .

:0434  a crs:Function, ra:Class,
        skos:Concept ;
    crs:isPerformedBy [ crs:hasAgent ca:9135 ] ;
    dct:source ras:2006-00435306 ;
    skos:definition "The function of the official receiver and the official trustee implementing orders made under the relevant Commonwealth legislation to collect child maintenance payments or deprive criminals of monetary gains made from illegal actions. Activities include accounting for financial transactions, delivering addresses (presentations), acquiring, protecting and realising property forfeited to the Commonwealth or in satisfaction of pecuniary penalty orders and child maintenance arrears, liaison, allocating orders, policy, procedures, reporting and preparing inventories." ;
    skos:inScheme :conceptScheme: ;
    skos:prefLabel "Special Trustee Management" .

:0435  a crs:Function, ra:Class,
        skos:Concept ;
    crs:isPerformedBy [ crs:hasAgent ca:9135 ] ;
    dct:source ras:2006-00435306 ;
    skos:definition "The function of exercising official trustee powers in the administration of personal insolvency matters.  Includes administering the affairs of a bankrupt, debtor or deceased debtor, scheme of arrangement or composition, deed of assignment, deed of arrangement or a composition and debt agreement. Also includes annulment of bankruptcy, discharge from bankruptcy, the discovery, acquisition, protection and realisation of assets, investigations, meetings of creditors, deciding on bankrupt's application for overseas travel and handling public reaction such as complaints and compliments." ;
    skos:inScheme :conceptScheme: ;
    skos:prefLabel "Trustee Administration" .

:0436  a crs:Function, ra:Class,
        skos:Concept ;
    crs:isPerformedBy [ crs:hasAgent ca:9136 ] ;
    dct:source ras:2003-00283436 ;
    skos:definition "The function of applying corporate level management strategies, plans and processes to meet regulatory requirements. Includes establishment and implementation of the company constitution and activities to meet legislative requirements such as those of the Corporations Act. " ;
    skos:inScheme :conceptScheme: ;
    skos:prefLabel "Corporate Management" .

:0437  a crs:Function, ra:Class,
        skos:Concept ;
    crs:isPerformedBy [ crs:hasAgent ca:9136 ] ;
    dct:source ras:2003-00283436 ;
    skos:definition "The function of providing high quality general practice vocational training at the regional level. Includes vertical integration of training and educational programs, the establishment of contracts with consortia, and accreditation of training programs. Also includes registrar selection, related promotional material, and research and implementation of specific programs to cover gaps in funding and delivery." ;
    skos:inScheme :conceptScheme: ;
    skos:prefLabel "General Practice Vocational Training" .

:0438  a crs:Function, ra:Class,
        skos:Concept ;
    crs:isPerformedBy [ crs:hasAgent ca:9138 ] ;
    dct:source ras:2009-00181784 ;
    skos:definition """The core business of providing agreed services such as family assistance and aged care payments and health screening programs, on behalf of government agencies or commercial enterprises for an agreed fee, and research and development of new business opportunities on behalf of the Commonwealth Government. Also includes Medicare Australia’s involvement in government policy, program development and business activities such as international consultancies, where Medicare Australia successfully tenders for, or is asked to provide services.

These opportunities may leverage Medicare Australia’s current capability such as the use of Medicare Australia’s
network of branch offices for depositing forms for other government programs or build on this capability for the future where the agency acts as a test-bed for government initiatives in particular areas such as e-commerce including e-signatures, public key infrastructure (PKI) and a unique health identifier (UHI). It may also involve service delivery improvements such as online claiming. Also includes consulting for other countries in Medicare Australia’s areas of expertise.

 Includes:
• Identification of the business opportunity either by Medicare Australia or a potential business partner
• Research and development of the capability required to support the business opportunity including testing
• Provision of advice in relation to government policy, programs and initiatives that impact on Medicare Australia’s business
• Documentation of the capability including business case development, commercialisation and production/implementation plans and registration of any intellectual property
• Stakeholder engagement and liaison with business partners and potential business partners on implementation of the program, policy inititative, business or service capability
• Reporting to government on the potential for use and business benefit across government
• Competing to deliver a new piece of business or consulting service such as international consultancies
• Negotiation of the service to be provided including the nature of the service, agreed performance criteria, service delivery mechanisms, reporting and fees payable for the service
• Reporting on the service for management purposes such as auditing, monitoring of performance and to customer agencies or businesses on services delivered
• Education of stakeholders such as potential business partners, agency management and staff about the application of the business or service capability. """;
    skos:inScheme :conceptScheme: ;
    skos:prefLabel "Business Development And Service Delivery" .

:0439  a crs:Function, ra:Class,
        skos:Concept ;
    crs:isPerformedBy [ crs:hasAgent ca:9138 ] ;
    dct:source ras:2009-00181784 ;
    skos:definition """The core business of making payments to eligible claimants in the form of government approved health and medical related benefits, incentives, reimbursements and rebates. Includes:
• Supporting administration for health and medical payment services
• Determination of eligibility under the relevant legislation or through an agreement with another agency; eligible enrolees include Australian residents, medical practitioners, pharmacists, hospitals, mental health providers, aged care providers, pharmaceutical associations, medical practices, medical graduates and pathology laboratories; notification of eligibility or otherwise
• Enrolment and registration of eligible applicants for payments for a range of schemes such as Medicare, pharmaceutical benefits, hearing services, pathology, private health insurance rebate, rural retention program and immunisation incentive payments for general practitioners and reimbursements of fees for medical students
• Receipt of claims for payment from claimants for approved schemes and services
• Processing of claims for payment including assessment of eligibility for the claim according to the business rules of the relevant scheme and including compensation recovery; notification of payment or non-payment to claimant where appropriate
• Making the appropriate payment to the claimant
• Investigating overpayment and fraud including receipt of information, monitoring of excessive and non-compliant claims, investigation activities such as document checks, compliance audits and other methods of establishing overpayment or non-compliance; also includes referral for prosecution
• Practitioner review including requests to review a practitioner, the review process including notification of the outcomes from a professional services review, action following from a review such as the revocation or suspension of approval to supply under the Pharmaceutical Benefits Scheme or suspension of access to Medicare
• Recovery of overpayment based on information establishing amount of overpayment and calculation of repayment amount and method of repayment
• Preparation of reports for management purposes such as auditing, monitoring and investigations for fraud and overpayment and other service performance reporting
• Education of providers and potential providers in how to participate in the health and medical payment schemes
• Responding to appeals relating to ineligibility for registration or payment
• Provision of reports and data from health and medical payments databases for government policy development, epidemiological studies and personal information for individual clients, their families and carers.""";
    skos:inScheme :conceptScheme: ;
    skos:prefLabel "Health And Medical Payments Services" .

:0440  a crs:Function, ra:Class,
        skos:Concept ;
    crs:isPerformedBy [ crs:hasAgent ca:9138 ] ;
    dct:source ras:2009-00181784 ;
    skos:definition """The core business of establishing, updating and maintaining national registers relating to health and medical matters such as childhood immunisation, organ donation and bowel cancer screening.
This core business provides de-personalised data from the health and medical registers to organisations and agencies for research purposes.
Includes:
• Supporting administration in relation to the health and medical registers
• Receipt and acknowledgement of requests for registration
• Creation, updating and monitoring of registers
• Provision of reports and data from registers for government policy development, eligibility for payments to providers, epidemiological studies and personal information for registrants, their families and carers.""";
    skos:inScheme :conceptScheme: ;
    skos:prefLabel "Health And Medical Register Services" .

:0441  a crs:Function, ra:Class,
        skos:Concept ;
    crs:isPerformedBy [ crs:hasAgent ca:9138 ] ;
    dct:source ras:2009-00181784 ;
    skos:definition """The core business of administering medical indemnity insurance to reduce the impact of large claims against medical practitioners. The aim is to make medical indemnity insurance more affordable for medical practitioners.
Also includes:
• Handling enquiries in relation to medical indemnity
• Development of procedures and service delivery guidelines and business rules
• Invoicing and receipt of payments for medical indemnity cover from medical practitioners and United Medical Protection (UMP)
• Determination of eligibility for a scheme under the medical indemnity legislation, notification of eligibility or otherwise
• Enrolment and registration of eligible applicants for payments and subsidies relating to medical indemnity schemes
• Receipt of claims for payment or subsidy from claimants for approved schemes
• Investigating overpayment and fraud including receipt of information, monitoring of non-compliant claims, investigation activities such as data and document checks, compliance audits and other methods of establishing that offences have been committed under the relevant legislation; also includes referral for prosecution, where appropriate
• Recovery of overpayment based on information establishing amount of overpayment and calculation of repayment amount and method of repayment
• Preparation of reports for management purposes such as auditing and monitoring and other service performance reporting.  """;
    skos:inScheme :conceptScheme: ;
    skos:prefLabel "Medical Indemnity" .

:0442  a crs:Function, ra:Class,
        skos:Concept ;
    crs:isPerformedBy [ crs:hasAgent ca:9152 ] ;
    dct:source ras:2009-00667625 ;
    skos:definition "The function of managing and supporting people in immigration detention facilities who, upon entry or attempted entry into the country and/or offshore national territories, are deemed to be unlawful non-citizens by national immigration legislation. Includes registering and monitoring the health and welfare of people at immigration detention facilities, apprehending detainees who left a detention facility without authorization and conducting investigations at immigration detention facilities. Also includes managing the services provided by designated contractors and the provision of information, education and recreational lifestyle services to people in immigration detention facilities." ;
    skos:inScheme :conceptScheme: ;
    skos:prefLabel "Detention Management" .

:0443  a crs:Function, ra:Class,
        skos:Concept ;
    crs:isPerformedBy [ crs:hasAgent ca:9152 ] ;
    dct:source ras:2009-00667625 ;
    skos:definition "The function of administering the temporary and permanent entry into, and the presence in, Australia of non-citizens.  Includes funding and promoting of migration to Australia, processing visas onshore and offshore, managing security bonds related to particular visa classes and the registration of migration agents.  Also includes the monitoring and enforcement of immigration laws and visa conditions within Australia and the investigation of apparent breaches of these laws and visa conditions. Also includes collecting, collating, processing and disseminating information and intelligence which assists in prosecution and deportation of unlawful non-citizens, liaison with national and international bodies and the provision of training and translating services." ;
    skos:inScheme :conceptScheme: ;
    skos:prefLabel "Migration Management" .

:0444  a crs:Function, ra:Class,
        skos:Concept ;
    crs:isPerformedBy [ crs:hasAgent ca:9154 ] ;
    dct:source ras:2007-00228350 ;
    skos:definition """The function of determining strategic directions and ensuring that the organisation fulfils its statutory functions and achieves its objectives. Includes managing the administration of the Board's
membership and remuneration and providing secretariat support services for the organisation's Board
as well as for those committees established by the Board. Also includes liaison with government and
non-government organisations.""";
    skos:inScheme :conceptScheme: ;
    skos:prefLabel "Corporate Governance" .

:0445  a crs:Function, ra:Class,
        skos:Concept ;
    crs:isPerformedBy [ crs:hasAgent ca:9154 ] ;
    dct:source ras:2007-00228350 ;
    skos:definition "The function of ensuring the safety of food in Australia through a range of activities including developing food regulatory measures, assessing applications for the development of such measures, the monitoring and surveillance of food available in Australia, and the coordination and monitoring of food recalls. Also includes the development of food education initiatives; the distribution of information to increase public awareness of food standards, food labels and food emergencies, and the development of policies in relation to food standards and safety." ;
    skos:inScheme :conceptScheme: ;
    skos:prefLabel "Food Standards And Safety" .

:0446  a crs:Function, ra:Class,
        skos:Concept ;
    crs:isPerformedBy [ crs:hasAgent ca:9154 ] ;
    dct:source ras:2007-00228350 ;
    skos:definition """The function of maintaining and strengthening relationships and strategic alliances with key countries, regions and international agencies. Includes the development of strategies to facilitate the
harmonisation of food standards throughout the Asia Pacific region; communication with other countries in relation to food regulations and standards; the development, facilitation and administration of technical assistance programs to regional countries; and the provision of training courses on various aspects of food safety or the development of standards. Also includes the hosting of visits from international delegations; the presentation of papers at international conferences; the exchange of personnel; and the conducting of research into the processes and activities employed by other countries in relation to the development and enforcement of food standards.""";
    skos:inScheme :conceptScheme: ;
    skos:prefLabel "International Collaboration" .

:0447  a crs:Function, ra:Class,
        skos:Concept ;
    crs:isPerformedBy [ crs:hasAgent ca:9160 ] ;
    dct:source ras:2007-00380834 ;
    skos:definition """The function of administering and managing domestic environment, heritage or natural management programs including in the areas of biodiversity conservation, chemicals management, climate change, coasts and oceans, natural and cultural heritage, environmental protection, natural resource management, water resources, and energy and water efficiency. Includes the coordination of national cooperative programs in collaboration with state and territory or local governments, industry and consumer representative bodies, property owners, Indigenous land owners and members of the community. Also includes coordinating the use of economic instruments such as tax incentives and financial assistance measures that may include supporting environment, heritage or natural resource
management projects through investment or funding programs, the administration of grants and rebates or the development of structural adjustment packages, the development of educational
resources, public awareness campaigns, information products and the provision of policy advice to Ministers.""";
    skos:inScheme :conceptScheme: ;
    skos:prefLabel "Environment And Heritage Program Administration" .

:0448  a crs:Function, ra:Class,
        skos:Concept ;
    crs:isPerformedBy [ crs:hasAgent ca:9160 ] ;
    dct:source ras:2007-00380834 ;
    skos:definition "The function of regulating activities to protect and conserve Australia's environment and heritage. Includes advising the Australian Government on the development of national policies, legislation, strategies and environmental standards. Also includes conducting investigations and inspections; processing permits, authorities or licences; approving referred actions; maintaining statutory lists and registers; developing environmental management plans; and making declarations and orders." ;
    skos:inScheme :conceptScheme: ;
    skos:prefLabel "Environment And Heritage Regulation" .

:0449  a crs:Function, ra:Class,
        skos:Concept ;
    crs:isPerformedBy [ crs:hasAgent ca:9160 ] ;
    dct:source ras:2007-00380834 ;
    skos:definition """The function of monitoring, advising and developing strategies in relation to global and regional environment, heritage and natural resource management issues, including the development of global and regional partnerships and institutions. Includes: developing and providing policy advice and briefings to support negotiations in relation to the representation of Australia’s interests at global or
regional conferences, conventions and other events; developing and providing policy advice in relation to the development and implementation of global and regional agreements and partnerships; ongoing liaison with global and regional forums and institutions with responsibility for monitoring and administering international agreements; evaluating Australia’s environmental performance and
conditions, including the development of performance indicators, and preparing national reports; monitoring compliance with global and regional agreements and preparing national progress reports; providing financial or technical assistance, including the sharing of expertise, to other countries and to global and regional institutions or forums; liaising with other countries, international institutions or forums, other Australian Government departments and agencies, state and territory governments and other stakeholders and administering nominations, appointments and resignations of Australian delegates or other representatives.""";
    skos:inScheme :conceptScheme: ;
    skos:prefLabel "International Relations" .

:0450  a crs:Function, ra:Class,
        skos:Concept ;
    crs:isPerformedBy [ crs:hasAgent ca:9168 ] ;
    dct:source ras:2007-00367755 ;
    skos:definition """The function of providing assistance and employment-related services to government agencies and employees. Includes developing and promoting Australian public service employment policies and practices, and offering employment services such as external reviews of employment-related decisions made by an external organisation. Also includes handling external inquiries, reporting on disclosures
made to the Public Service, Merit Protection and/or Parliamentary Commissioners and undertaking consultancy services.""";
    skos:inScheme :conceptScheme: ;
    skos:prefLabel "Employment-Related Services" .

:0451  a crs:Function, ra:Class,
        skos:Concept ;
    crs:isPerformedBy [ crs:hasAgent ca:9168 ] ;
    dct:source ras:2007-00367755 ;
    skos:definition """The function of providing learning and development services to government agencies and employees. Includes strengthening all aspects of leadership capability in the Australian Public Service by
developing, evaluating and delivering leadership programs. Also includes providing consultancy services, customised training and skills development programs.""";
    skos:inScheme :conceptScheme: ;
    skos:prefLabel "Learning And Development Services" .

:0452  a crs:Function, ra:Class,
        skos:Concept ;
    crs:isPerformedBy [ crs:hasAgent ca:9168 ] ;
    dct:source ras:2007-00367755 ;
    skos:definition """The function of providing organisational performance services to Australian Public Service agencies, evaluating the extent to which agencies incorporate and uphold the Australian Public Service Values,
and the adequacy of systems and procedures in agencies for ensuring compliance with the Code of Conduct. Includes facilitating continuous improvement in people management throughout the Australian Public Service and reporting on the performance and management of the Australian Public Service Values and Code of Conduct. Also includes providing advice and assistance on public service matters to agencies on request, as well as advice on policy and legislative issues affecting agencies, such as workplace diversity, workforce planning, human resources capability and governance.""";
    skos:inScheme :conceptScheme: ;
    skos:prefLabel "Organisational Performance Services" .

:0453  a crs:Function, ra:Class,
        skos:Concept ;
    crs:isPerformedBy [ crs:hasAgent ca:9170 ] ;
    dct:source ras:2008-00218668 ;
    skos:definition "The function of delivering services to separated parents to enable the transfer of payments for the benefit of their children. Includes registration, assessment, collection and transfer of payments and the development of guidelines and procedures. Also includes referring parents to other services, processing objections to child support decisions and following up on complaints relating to service delivery. " ;
    skos:inScheme :conceptScheme: ;
    skos:prefLabel "Child Support" .

:0454  a crs:Function, ra:Class,
        skos:Concept ;
    crs:isPerformedBy [ crs:hasAgent ca:9184 ] ;
    dct:source ras:2009-00941258 ;
    skos:definition """The core business of this area is to administer grants, in accordance with Departmental policy and legislation, to support and encourage Australian broadcasting and the digital economy.

Broadcasting is the delivery of television or radio programs to an audience through radiofrequency spectrum, cable, optical fibre or satellite. It does not include services that make programs available on demand.

Broadcasting covers the following activities:
• establishing cost effective access to national broadcasting and television services for the Australian public;
• establishing the viability and accountability of the community broadcasting sector in Australia;
• establishing and providing the accountability and funding of national broadcasters in Australia;
• establishing and providing digital broadcasting for radio and television.

The Digital Economy is the network of economic and social activities which are enabled by information and communications technologies, particularly the internet. The digital economy covers the following areas:
• developing the digital economy in Australia;
• managing online content issues and broader content issues related to the digital economy; and
• establishing and providing online security and internet safety within Australia.

The tasks associated with Administering Grants include:
• receiving grant proposals and allocating resources for their evaluation;
• performing an evaluation of grant proposals and advising applicants and stakeholders of the evaluation outcome;
• providing feedback to parties on the application process;
• establishing funding agreements;
• liaison with applicants;
• administering grant funding;
• monitoring the ongoing performance of grant related activity;
• dealing with breaches of grant conditions;
• audit activities;
• performing grant acquittals; and
• development of agency procedures supporting the administration of grants.""";
    skos:inScheme :conceptScheme: ;
    skos:prefLabel "Broadcasting And The Digital Economy Grant Management" .

:0455  a crs:Function, ra:Class,
        skos:Concept ;
    crs:isPerformedBy [ crs:hasAgent ca:9184 ] ;
    dct:source ras:2009-00941258 ;
    skos:definition """The core business of this area is to implement government-wide policies, plans, regulatory frameworks and legislation for broadcasting and the digital economy within Australia. This includes activities relating to the regulation of the digital economy, the information economy, digital television, radio and television broadcasting, and content within these media. It also includes monitoring to ensure that implementation goes according to schedule and that standards are met.

Broadcasting is the delivery of television or radio programs to an audience through radio frequency spectrum, cable, optical fibre or satellite. It does not include services that make programs available on demand.

Broadcasting covers the following activities:
• establishing cost effective access to national broadcasting and television services for the Australian public;
• establishing the viability and accountability of the community broadcasting sector in Australia;
• establishing and providing the accountability and funding of national broadcasters in Australia;
• establishing and providing digital broadcasting for radio and television;
• provision of commercial media regulation; and
• managing broadcasting content issues.

The Digital Economy is the network of economic and social activities which are enabled by information and communications technologies, particularly the internet. The digital economy covers the following activities:
• developing the digital economy in Australia;
• managing online content issues and broader content issues related to the digital economy;
• establishing and providing online security and internet safety within Australia;
• establishing Government strategy for the digital economy;
• the performance of Australian business in the digital economy;
• establishing cross-portfolio coordination on digital economy issues; and
• establishing International engagement on digital economy issues by Australia.

The tasks associated with Policy and Legislation Implementation in these activities include:
• maintaining regulatory frameworks based on legislation;
• providing advice on policy and legislation to stakeholders from outside of the Department, to whole-of-government and the Australian community;
• managing committee and ad-hoc meetings and task forces;
• consulting, informing and liaising with stakeholders;
• arranging or attending external conferences;
• monitoring, evaluating, reviewing and auditing regulatory activities;
• developing and implementing plans, procedures and instructions; and
• preparing submissions and reports.""";
    skos:inScheme :conceptScheme: ;
    skos:prefLabel "Broadcasting And The Digital Economy Policy And Legislation Implementation" .

:0456  a crs:Function, ra:Class,
        skos:Concept ;
    crs:isPerformedBy [ crs:hasAgent ca:9184 ] ;
    dct:source ras:2009-00941258 ;
    skos:definition """The core business of developing whole-of-government policy for Australia's digital economy and Australian broadcasting. This can include policy created for digital television, radio and television broadcasting, and content regulation.

Broadcasting is the delivery of television or radio programs to an audience through radio frequency spectrum, cable, optical fibre or satellite. It does not include services that make programs available on demand.

Broadcasting covers the following activities:
• establishing cost effective access to national broadcasting and television services for the Australian public;
• establishing the viability and accountability of the community broadcasting sector in Australia;
• establishing and providing the accountability and funding of national broadcasters in Australia;
• establishing and providing digital broadcasting for radio and television;
• provision of commercial media regulation; and
• managing broadcasting content issues.

The Digital Economy is the network of economic and social activities which are enabled by information and communications technologies, particularly the internet. The digital economy covers the following activities:
• developing the digital economy in Australia;
• managing online content issues and broader content issues related to the digital economy;
• establishing and providing online security and internet safety within Australia;
• establishing Government strategy for the digital economy;
• the performance of Australian business in the digital economy;
• establishing cross-portfolio coordination on digital economy issues; and
• establishing International engagement on digital economy issues by Australia.

The tasks associated with Policy Implementation in these activities include:
• researching, analysing and reviewing existing policy and legislation;
• consulting stakeholders;
• managing committees and taskforces;
• developing legal and policy frameworks;
• preparing papers, submissions and reports;
• establishing funding frameworks;
• providing policy advice to ministers and other stakeholders within the Department; and
• drafting and authorising policy.""";
    skos:inScheme :conceptScheme: ;
    skos:prefLabel "Broadcasting And The Digital Economy Policy Development" .

:0457  a crs:Function, ra:Class,
        skos:Concept ;
    crs:isPerformedBy [ crs:hasAgent ca:9184 ] ;
    dct:source ras:2009-00941258 ;
    skos:definition """The core business of supporting and fostering the development of the Australian broadcasting sector and the digital economy.

Broadcasting is the delivery of television or radio programs to an audience through radio frequency spectrum, cable, optical fibre or satellite. It does not include services that make programs available on demand.

Broadcasting covers the following activities:
• establishing cost effective access to national broadcasting and television services for the Australian public;
• establishing the viability and accountability of the community broadcasting sector in Australia;
• establishing and providing the accountability and funding of national broadcasters in Australia;
• establishing and providing digital broadcasting for radio and television;
• provision of commercial media regulation;
• managing broadcasting content issues;

The Digital Economy is the network of economic and social activities which are enabled by information and communications technologies, particularly the internet. The digital economy covers the following activities:
• developing the digital economy in Australia;
• managing online content issues and broader content issues related to the digital economy;
• establishing and providing online security and internet safety within Australia;
• establishing Government strategy for the digital economy;
• the performance of Australian business in the digital economy;
• establishing cross-portfolio coordination on digital economy issues; and
• establishing International engagement on digital economy issues by Australia.

The tasks associated with Sector and Industry Development in these activities includes:
• developing and operating Government programs for Australian sectors and industries;
• promoting Australian sectors and industries through international and regional organisations;
• promoting Australian sectors and industries by arranging or attending conferences;
• researching and analysing Australian sectors and industries;
• monitoring the ongoing performance of Government programs for Australian sectors and industries;
• consulting and informing stakeholders;
• preparing submissions and reports;
• administering funding for relevant Government programs;
• managing initiatives, projects and task forces for relevant Government programs; and
• development of internal procedures to manage sector and industry development activities.""";
    skos:inScheme :conceptScheme: ;
    skos:prefLabel "Broadcasting And The Digital Economy Sector And Industry Development" .

:0458  a crs:Function, ra:Class,
        skos:Concept ;
    crs:isPerformedBy [ crs:hasAgent ca:9184 ] ;
    dct:source ras:2009-00941258 ;
    skos:definition """The core business of this area is to administer grants, in accordance with Departmental policy and legislation, to support and encourage telecommunications, broadband and postal services.
Telecommunications is the carriage of communications by means of guided or unguided electromagnetic energy.

Telecommunications covers the following activities:
• establishing competitive and accessible telecommunication services for the Australian public; and
• improving telecommunications services to indigenous communities and regional Australia.

Broadband is a term used to describe fast, high bandwidth always-on access to the Internet.
Broadband covers the following activities:
• establishing equitable access to broadband services across Australia;
• investing in broadband and communications infrastructure;
• understanding the implications of broadband usage and broadband policy for the Government;
• postal Services provides the collection and distribution of postal articles, including letters and packages;
• postal services covers the following areas; and
• establishing cost effective and accessible postal services within Australia.

The tasks associated with Administering Grants in this area include:
• receiving grant proposals and allocating resources for their evaluation;
• performing an evaluation of grant proposals and advising applicants and stakeholders of the evaluation outcome;
• providing feedback to parties on the application process;
• liaison with applicants;
• establishing funding agreements;
• administering grant funding;
• monitoring the ongoing performance of grant related activity;
• dealing with breaches of grant conditions;
• conducting audits;
• performing grant acquittals; and
• development of agency procedures supporting the administration of grants.""";
    skos:inScheme :conceptScheme: ;
    skos:prefLabel "Telecommunications, Broadband And Postal Services Grant Management" .

:0459  a crs:Function, ra:Class,
        skos:Concept ;
    crs:isPerformedBy [ crs:hasAgent ca:9184 ] ;
    dct:source ras:2009-00941258 ;
    skos:definition """The core business of this area is to implement government-wide policies, regulatory frameworks and legislation relating to telecommunications, broadband and postal services. This includes activities relating to the development of broadband infrastructure and telecommunication networks, network and spectrum regulation, and consumer protection. It also includes monitoring to ensure that implementation goes according to schedule and that standards are met. Excludes managing grants to support the implementation of telecommunications, broadband and postal services.
Telecommunications is the carriage of communications by means of guided or unguided electromagnetic energy.

Telecommunications covers the following activities:
• establishing competitive and accessible telecommunication services for the Australian public;
• establishing telecommunications regulatory policy;
• improving telecommunications services to indigenous communities and regional Australia;
• establishing law enforcement and the use of telecommunications;
• establishing radio communications spectrum and telephone number regulation;
• establishing internet governance and domain name regulation;
• establishing communications infrastructure protection;
• establishing and directing Government enterprises in the telecommunications industry;
• establishing International agreements and trade policy for telecommunication and network services; and
• establishing International engagement on internet and telecommunication issues by Australia;

Broadband is a term used to describe fast, high bandwidth always-on access to the Internet. Broadband covers the following activities:
• establishing equitable access to broadband services across Australia;
• investing in broadband and communications infrastructure;
• understanding the implications of broadband usage and broadband policy for the Government; and
• establishing the rollout of high speed Broadband to Australia.

Postal Services provide the collection and distribution of postal articles, including letters and packages. Postal services cover the following activities:
• establishing and directing cost effective and accessible postal services within Australia;
• establishing and directing Australian postal services regulation;
• establishing and directing Government enterprises in the postal industry; and
• establishing International engagement on postal services issues by Australia.

The tasks associated with the Implementation of Policy and Legislation for these activities include:
• maintaining regulatory frameworks based on legislation;
• providing advice on policy and legislation to stakeholders from outside of the Department, to whole-of-government and the Australian community;
• managing committee meetings, ad-hoc meetings and taskforces;
• consulting stakeholder, informing and liaising with stakeholders;
• monitoring, evaluating and reviewing regulatory activities; and
• developing and implementing plans, procedures and instructions.""";
    skos:inScheme :conceptScheme: ;
    skos:prefLabel "Telecommunications, Broadband And Postal Services Policy And Legislation Implementation" .

:0460  a crs:Function, ra:Class,
        skos:Concept ;
    crs:isPerformedBy [ crs:hasAgent ca:9184 ] ;
    dct:source ras:2009-00941258 ;
    skos:definition """Telecommunications, Broadband and Postal Services Policy Development
The core business of this area is to develop whole-of-government policy for Australian telecommunications and broadband, and the postal industry of Australia. This includes policy and legislation created for the development of broadband infrastructure and telecommunication networks, network and spectrum regulation and consumer protection.
Telecommunications is the carriage of communications by means of guided or unguided electromagnetic energy.

Telecommunications covers the following activities:
• establishing competitive and accessible telecommunication services for the Australian public;
• establishing telecommunications regulatory policy;
• improving telecommunications services to indigenous communities and regional Australia;
• establishing law enforcement and the use of telecommunications;
• establishing radio communications spectrum and telephone number regulation;
• establishing internet governance and domain name regulation;
• establishing communications infrastructure protection;
• establishing and directing Government enterprises in the telecommunications industry;
• establishing International agreements and trade policy for telecommunication and network services;
• establishing International engagement on internet and telecommunication issues by Australia; and
• broadband is a term used to describe fast, high bandwidth always-on access to the Internet.

Broadband covers the following activities:
• establishing equitable access to broadband services across Australia;
• investing in broadband and communications infrastructure;
• understanding the implications of broadband usage and broadband policy for the Government;
• establishing the rollout of high speed Broadband to Australia; and
• Postal Services provides the collection and distribution of postal articles, including letters and packages.

Postal Services covers the following activities:
• establishing and directing cost effective and accessible postal services within Australia;
• establishing and directing Australian postal services regulation;
• establishing and directing Government enterprises in the postal industry; and
• establishing International engagement on postal services issues by Australia.

The tasks associated with the Development of Policy include:
• researching, analysing and reviewing existing policy and legislation;
• consulting with stakeholders;
• managing committee meetings, ad-hoc meetings and taskforces;
• developing legal and policy frameworks;
• preparing discussion papers, submissions and reports;
• establishing funding frameworks;
• providing policy advice to ministers and other stakeholders within the Department;
• drafting and authorising policy; and
• negotiating, reviewing and establishing agreements.""";
    skos:inScheme :conceptScheme: ;
    skos:prefLabel "Telecommunications, Broadband And Postal Services Policy Development" .

:0461  a crs:Function, ra:Class,
        skos:Concept ;
    crs:isPerformedBy [ crs:hasAgent ca:9184 ] ;
    dct:source ras:2009-00941258 ;
    skos:definition """The core business of supporting and fostering the development of Australia's telecommunication, broadband and postal sectors. Telecommunications is the carriage of communications by means of guided or unguided electromagnetic energy.

Telecommunications covers the following activities:
• establishing telecommunications regulatory policy;
• improving telecommunications services to indigenous communities and regional Australia;
• establishing law enforcement and the use of telecommunications;
• establishing Radio communications spectrum and telephone number regulation;
• establishing Internet governance and domain name regulation;
• establishing Communications infrastructure protection;
• establishing and directing Government enterprises in the telecommunications industry;
• establishing International agreements and trade policy for telecommunication and network services; and
• establishing International engagement on internet and telecommunication issues by Australia.

Broadband is a term used to describe fast, high bandwidth always-on access to the Internet.
Broadband covers the following activities:
• establishing equitable access to broadband services across Australia;
• investing in broadband and communications infrastructure;
• understanding the implications of broadband usage and broadband policy for the Government; and
• establishing the rollout of high speed Broadband to Australia.

Postal Services provide the collection and distribution of postal articles, including letters and packages. Postal services covers the following activities:
• establishing and directing cost effective and accessible postal services within Australia;
• establishing and directing Australian postal services regulation;
• establishing and directing Government enterprises in the postal industry; and
• establishing International engagement on postal services issues by Australia.

The tasks associated with Sector and Industry Development in these areas includes:
• developing and operating Government programs for Australian sectors and industries;
• promoting Australian sectors and industries through international and regional organisations;
• promoting Australian sectors and industries by arranging or attending conferences;
• researching and analysing Australian sectors and industries;
• monitoring the ongoing performance of Government programs for Australian sectors and industries;
• consulting and informing stakeholders;
• preparing submissions and reports;
• administering funding for relevant Government programs;
• managing initiatives, projects and task forces for relevant Government programs; and
• development of internal procedures to manage sector and industry development activities.""";
    skos:inScheme :conceptScheme: ;
    skos:prefLabel "Telecommunications, Broadband And Postal Services Sector And Industry Development " .

:0462  a crs:Function, ra:Class,
        skos:Concept ;
    crs:isPerformedBy [ crs:hasAgent ca:9185 ] ;
    dct:source ras:2009-00179260 ;
    skos:definition "The function of implementing labour market programs. Includes managing and coordinating the delivery of employment services and assistance to job seekers; administering the provision of grants and programs to assist targeted groups in the community, such as Indigenous Australians and disadvantaged job seekers; and liaising with local communities. " ;
    skos:inScheme :conceptScheme: ;
    skos:prefLabel "Employment Services" .

:0463  a crs:Function, ra:Class,
        skos:Concept ;
    crs:isPerformedBy [ crs:hasAgent ca:9185 ] ;
    dct:source ras:2009-00593947 ;
    skos:definition """The function of supporting Australia’s higher education systems. Higher education is post-secondary education offered by a university or other recognised higher education institution where students obtain formal qualifications ranging from an advanced diploma through to a doctoral degree. The tasks associated with higher education include:
•	the development of the regulatory framework and qualification standards for higher education
•	the planning and outcomes of evaluations, reviews, analyses and assessments of initiatives, programs or aspects of higher education
•	the management of enquiries about higher education programs, funding etc
•	development of internal and external higher education policies, frameworks, administrative arrangements, reports, procedures and guidelines
•	feedback provided to other agencies developing policies, frameworks and procedures
•	the design, development, promotion, establishment, implementation, review and management of higher education programs, schemes and projects
•	nomination, assessment, determination and presentation of awards, prizes and scholarships
•	receipt and provision of advice relating to higher education
•	management of conferences, forums etc arranged by the agency and participation in conference, forums etc arranged by other organisations
•	management of research and analysis into higher education
•	management of financial assistance to higher education stakeholders
•	management of appeals to the agency or higher authorities
•	delegations of power
•	liaison with stakeholders
•	negotiation, establishment, maintenance and review of agreements and arrangements
•	collection and analysis of statistics and information
•	management of internal and external committees and taskforces
•	monitoring accountability, quality, fairness and financial viability of higher education providers
•	audits of funding programs to ensure compliance with funding arrangements.
""";
    skos:inScheme :conceptScheme: ;
    skos:prefLabel "Higher Education" .

:0464  a crs:Function, ra:Class,
        skos:Concept ;
    crs:isPerformedBy [ crs:hasAgent ca:9185 ] ;
    dct:source ras:2009-00593947 ;
    skos:definition """The function of promoting Australia’s international profile as a leading provider of education and training to the world to encourage overseas students to study in Australia and develop relationships overseas to enable Australians to research, study or undertake professional development off-shore. The tasks associated with international education include:
•	development of internal and external international education policies, frameworks, administrative arrangements, reports, codes, standards, procedures and guidelines
•	management of research and analysis into international education
•	the design, development, promotion, establishment, implementation, review and management of international education programs and projects
•	management of internal and external committees and taskforces
•	receipt and provision of advice relating to international education
•	managing the registration and monitoring of registered education providers offering courses to overseas students studying in Australia on student visas and managing complaints against providers
•	management of conferences, forums etc arranged by the agency and participation in conferences, forums etc arranged by other organisations
•	the development and management of training workshops and seminars for education providers
•	monitoring the administration of funds following the collapse or closure of registered education providers
•	the planning and outcomes of evaluations, reviews, analyses and assessments of initiatives, programs or aspects of international education
•	collecting and monitoring information about overseas countries and their education stakeholders
•	the management of enquiries about international education programs, funding etc
•	the negotiation, establishment, maintenance and review of agreements and arrangements
•	collection and analysis of statistics and information
•	liaison with stakeholders and developing relationships with overseas governments and multilateral organisations for the purposes of achieving academic mobility
•	feedback provided to other agencies developing policies, frameworks and procedures
""";
    skos:inScheme :conceptScheme: ;
    skos:prefLabel "International Education" .

:0465  a crs:Function, ra:Class,
        skos:Concept ;
    crs:isPerformedBy [ crs:hasAgent ca:9185 ] ;
    dct:source ras:2009-00593947 ;
    skos:definition """The function of assisting the overseas trained to work and study in Australia by facilitating the recognition of overseas qualifications and skills in Australia; and assisting the Australian trained to work and study overseas by facilitating the recognition of Australian qualifications and skills in other countries. The tasks associated with qualifications and skills recognition include:
•	development of internal and external policies, frameworks, standards, procedures and guidelines
•	management of research and analysis
•	providing assessment of the recognition of educational and training qualifications and skills from overseas
•	the design, development, promotion, establishment, implementation, review and management of programs and projects
•	management of internal and external committees and taskforces
•	receipt and provision of advice relating to qualifications and skills recognition
•	the planning and outcomes of evaluations, reviews, analyses and assessments of initiatives, programs or aspects of qualifications and skills recognition
•	collecting and monitoring information about overseas countries and their education and training qualifications
•	the management of enquiries about the function of qualifications and skills recognition
•	the negotiation, establishment, maintenance and review of agreements eg bilateral and multilateral agreements and agreements for the provision of services
•	the development and management of training workshops and seminars
•	liaison with stakeholders
•	feedback provided to other agencies developing policies, frameworks and procedures
""";
    skos:inScheme :conceptScheme: ;
    skos:prefLabel "Qualifications And Skills Recognition" .

:0466  a crs:Function, ra:Class,
        skos:Concept ;
    crs:isPerformedBy [ crs:hasAgent ca:9185 ] ;
    dct:source ras:2009-00593947 ;
    skos:definition """The function of supporting Australia’s infant, primary and secondary school systems, through funding and assistance to non-government and government schools, research and analysis of national education issues, and developing national learning outcomes (eg literacy and numeracy) and programs to support the national school education system. The tasks associated with school education include:
•	the receipt and provision of advice relating to school education
•	negotiation, establishment, maintenance and review of agreements and arrangements, including bilateral agreement with State and Territory governments
•	the development of internal and external school education policies, frameworks, administrative arrangements, reports, procedures and guidelines
•	management of enquiries about school education programs, funding etc
•	development and management of seminars, education programs, presentations and training sessions
•	the planning and outcomes of evaluations, reviews, analyses and assessments of initiatives, programs or aspects of school education
•	the management of research and analysis into school education
•	audits of funding programs to ensure compliance with funding arrangements
•	the management of funding to schools and grant authorities
•	nominations, assessment, determination and presentation of awards, prizes and scholarships
•	design, development, promotion, establishment, implementation, review and management of school education programs, schemes and projects
•	management of appeals to the agency or higher authorities
•	management of financial assistance to school education stakeholders
•	liaison with stakeholders
•	feedback and comments provided to other agencies developing policies, frameworks, standards and procedures
•	management of conferences, forums etc arranged by the agency and participation in conferences, forums etc arranged by other organisations
•	collection and analysis of statistics and information
•	management of internal and external committees and taskforces
•	negotiation, establishment, maintenance and review of agreements and arrangements
•	delegations of power
""";
    skos:inScheme :conceptScheme: ;
    skos:prefLabel "School Education" .

:0467  a crs:Function, ra:Class,
        skos:Concept ;
    crs:isPerformedBy [ crs:hasAgent ca:9185 ] ;
    dct:source ras:2009-00593947 ;
    skos:definition """The function of managing and supporting the ongoing learning of trade skills development, personal development and general adult education to help people move into work or further study, or work in the community. The tasks associated with vocational education and training include:
•	the management of enquiries about vocational education and training programs, funding, student support etc
•	development of internal and external vocational education and training policies, frameworks, reports, administrative arrangements, procedures and guidelines
•	the planning and outcomes of evaluations, reviews, analyses and assessments of initiatives, programs or aspects of vocational education and training
•	the design, development, promotion, establishment, implementation, review and management of vocational education and training programs and projects
•	nomination, assessment, determination and presentation of awards, prizes and scholarships
•	management of internal and external committees and taskforces
•	management of research and analysis into vocational education and training
•	the monitoring and management of State and Territory vocational education and training plans and national projects
•	financial assistance to vocational education and training stakeholders
•	receipt and provision of advice relating to vocational education and training
•	the negotiation, establishment, maintenance and review of agreements
•	liaison with stakeholders
•	collection and analysis of statistics and information
•	management of conferences, forums etc arranged by the agency and participation in conferences, forums etc arranged by other organisations
•	maintenance of Australian apprentices register and national training register
•	audits of funding programs to ensure compliance with funding arrangements
•	the development of regulatory frameworks and standards
""";
    skos:inScheme :conceptScheme: ;
    skos:prefLabel "Vocational Education And Training" .

:0468  a crs:Function, ra:Class,
        skos:Concept ;
    crs:isPerformedBy [ crs:hasAgent ca:9186 ] ;
    dct:source ras:2009-00784107 ;
    skos:definition """The core business of developing and reviewing policy and administering programs to help Australia achieve a strong science and research capacity and to be engaged internationally on science and research to advance social development and economic growth. Includes:
• providing policy advice and opinions relating to portfolio research agencies, international matters and major strategic science and research issues;
• the design, development, promotion, establishment, implementation, review and evaluation of policy, frameworks, strategies, programs, schemes and projects;
• managing and monitoring programs for the delivery of financial assistance to science and research stakeholders, including appeals against decisions;
• representing Australia on key international bodies;
• supporting Australia’s international scientific research and technological collaboration relations with priority countries and organisations, including agreements with key countries and organisations;
• representing Australia in co-operative research infrastructure projects that advance national interests such as the bid to host the Square Kilometre Array radio telescope and providing funding of research infrastructure projects such as the Australian Square Kilometre Array Pathfinder (ASKAP);
• funding research and research training through the administration of block and competitive research grant schemes;
• conducting and participating in events such as science symposia;
• providing speeches and addresses to the science and research community;
• liaising and collaborating with research agencies on the establishment, monitoring and management of governance arrangements;
• providing committee and council support;
• promoting interaction between industry and scientific research institutions;
• promoting collaborative scientific research partnerships, such as those with Co-operative Research Centres promoting access to research information and resources; and
• assessing applications for Approved Research Institute status.""";
    skos:inScheme :conceptScheme: ;
    skos:prefLabel "Science And Research (Policy And Programs)" .

:0469  a crs:Function, ra:Class,
        skos:Concept ;
    crs:isPerformedBy [ crs:hasAgent ca:9186 ] ;
    dct:source ras:2009-00784107 ;
    skos:definition """The core business of developing and presenting creative, interactive science exhibitions and programs to encourage Australians to recognise and be aware of the importance of science, technology, maths and innovation, and to provide access to international visitors. Includes:
• project managing the development, build and maintenance of exhibitions, including travelling and temporary exhibitions, by means such as initial content research, market testing of exhibitions, graphic design;
• securing sponsorship and other funds, and entering into agreements with external national and international parties in relation to science communications programs;
• participating in meetings and committees with internal and external stakeholders;
• providing outreach programs to regional, remote and Indigenous communities;
• raising science awareness, promoting interest in science-based careers, and recognising outstanding contributions to science and education made by researchers and science teachers through science prizes and financial assistance programs;
• providing adult, school, family, children and member education programs and visitor events;
• promoting exhibitions, events and outreach programs;
• retail sales of merchandise through the shop and other outlets;
• managing corporate business names and brands
• venue hire in relation to the use of the organisation’s premises for events aligned to the organisation’s mission;
• visitor services including ticketing, facilitating visitor feedback and recording visitation statistics;
• receiving awards in recognition of the agency’s achievements;
• conducting and assisting with research into matters relating to science, technology, maths and innovation, and providing expert advice and assistance in relation to these matters;
• providing speeches and addresses to the science and research community;
• undertaking major reviews and audits of programs and operations;
• maintaining rare or unique accumulations of information documenting the organisation’s history;
• managing the development of special-purpose facilities and associated expansion projects required for the organisation’s program delivery; and
• developing policies, procedures, guidelines and plans in support of the science communication core business.""";
    skos:inScheme :conceptScheme: ;
    skos:prefLabel "Science Communications" .

:0470  a crs:Function, ra:Class,
        skos:Concept ;
    crs:isPerformedBy [ crs:hasAgent ca:9259 ] ;
    dct:source ras:2009-00921365 ;
    skos:definition "The function of patrolling coastal and offshore areas for the purpose of detecting illegal activity and coordinating interception. Includes the making of agreements and ongoing liaison with other agencies; coordination, conduct and review of air and sea surveillance and interception operations; referral of information from the community at large about suspect illegal activity; the use and control of defensive armaments or weapons; and provision of education and training." ;
    skos:inScheme :conceptScheme: ;
    skos:prefLabel "Civil Maritime Surveillance And Response" .

:0471  a crs:Function, ra:Class,
        skos:Concept ;
    crs:isPerformedBy [ crs:hasAgent ca:9259 ] ;
    dct:source ras:2009-00921365 ;
    skos:definition "The function of acquiring and breeding dogs for the detection of drugs and other prohibited or restricted imports carried or concealed on persons, and in baggage, parcels, cargo containers, vessels, aircraft and premises. Includes the conduct and support of breeding programs; the sale, donation or giving away of dogs to other agencies and organisations, or individuals; the deployment of dogs and handlers to assist in search operations conducted by Customs and other agencies; the training of dogs and handlers; the kennelling of dogs, including general care and upkeep; the selection of dogs to be trained and used for detection purposes." ;
    skos:inScheme :conceptScheme: ;
    skos:prefLabel "Detector Dogs" .

:0472  a crs:Function, ra:Class,
        skos:Concept ;
    crs:isPerformedBy [ crs:hasAgent ca:9259 ] ;
    dct:source ras:2009-00921365 ;
    skos:definition "The function of providing advice and assistance to industry through the delivery of concession schemes (eg Policy By-law Scheme, Project By-law Scheme, Tariff Concession System), dumping investigations (including application of anti-dumping and countervailing duties), import tariff quotas, duty drawback schemes, bounty schemes, and other programs and measures. Includes the case management of the provision of particular benefits and entitlements to clients, client training and education, representations from industry representative groups, formal review of decisions, etc." ;
    skos:inScheme :conceptScheme: ;
    skos:prefLabel "Industry Schemes And Trade Measures" .

:0473  a crs:Function, ra:Class,
        skos:Concept ;
    crs:isPerformedBy [ crs:hasAgent ca:9259 ] ;
    dct:source ras:2009-00921365 ;
    skos:definition "The function of collecting, analysing and distributing value-added, strategic information to meet the organisation’s compliance objectives. Includes making of agreements and liaison with other agencies, organisations and governments; development of case files or dossiers; development of intelligence product; tasking or allocation of intelligence product development work; joint ventures with other agencies involved in intelligence gathering; and provision of training to external clients etc." ;
    skos:inScheme :conceptScheme: ;
    skos:prefLabel "Intelligence" .

:0474  a crs:Function, ra:Class,
        skos:Concept ;
    crs:isPerformedBy [ crs:hasAgent ca:9259 ] ;
    dct:source ras:2009-00921365 ;
    skos:definition "The function of facilitating liaison and cooperation with other customs agencies, and international or regional organisations.  This includes advising or briefing of agency and other organisations on issues, trends, policies, programs etc; involvement in the making of international treaties, Memoranda of Understanding and other agreements; holding of bilateral meetings; facilitation of agency participation on international committees; conference facilitation and attendance; international policy agenda development; coordination of the provision of technical assistance to other customs administrations; hosting of visits by officials from other customs administrations and organisations." ;
    skos:inScheme :conceptScheme: ;
    skos:prefLabel "International Relations" .

:0475  a crs:Function, ra:Class,
        skos:Concept ;
    crs:isPerformedBy [ crs:hasAgent ca:9259 ] ;
    dct:source ras:2009-00921365 ;
    skos:definition "The function of investigating breaches of legislation administered by Customs that have been referred for special enquires. Includes conduct of case matters involving the initiation, planning, assessment, reporting and review of operations; the interview, search, detention and arrest of persons; surveillance of selected premises and people; securing of crime scenes; seizure of goods; collection and securing of evidence; making of enquiries; making of recommendations and decisions as to whether a case should be prosecuted, terminated, or settled out of court. Also includes the preparation of briefs of evidence, obtaining of warrants etc preceding litigation." ;
    skos:inScheme :conceptScheme: ;
    skos:prefLabel "Investigation" .

:0476  a crs:Function, ra:Class,
        skos:Concept ;
    crs:isPerformedBy [ crs:hasAgent ca:9259 ] ;
    dct:source ras:2009-00921365 ;
    skos:definition "The function of receiving and paying monies in the form of duties, taxes, penalties, drawbacks, refunds, reimbursements, securities, levies, remissions, rebates, bounties, damaged/missing goods claims etc. Includes collection of monies on behalf of other agencies, and the keeping of statistics." ;
    skos:inScheme :conceptScheme: ;
    skos:prefLabel "Revenue Management" .

:0477  a crs:Function, ra:Class,
        skos:Concept ;
    crs:isPerformedBy [ crs:hasAgent ca:9259 ] ;
    dct:source ras:2009-00921365 ;
    skos:definition "The function of controlling and facilitating the movement of commercial consignments of goods, including postal items, in and out of Australia. Includes provision of advice relating to tariff classification, goods valuation, and rules of origin; referral of matters to other agencies; making of agreements with clients and agencies (including copyright and trade mark ‘objections’); handling of appeals; the clearance of goods for import and export; the control of goods (including withholding) for the purposes of examination, treatment etc; the reporting of cargoes by carriers; the provision of education and training programmes; the enforcement of regulatory requirements relating to payment of duties and taxes, import/export prohibitions and restrictions etc; the handling of matters referred by industry for enquiry; the licensing of brokers and warehouse operators (including monitoring and control of licensee operations); formal review of decisions, the audit and checking of the commercial records of importers, exporters, brokers, carriers and warehouse operators." ;
    skos:inScheme :conceptScheme: ;
    skos:prefLabel "Trade Facilitation And Compliance" .

:0478  a crs:Function, ra:Class,
        skos:Concept ;
    crs:isPerformedBy [ crs:hasAgent ca:9259 ] ;
    dct:source ras:2009-00921365 ;
    skos:definition "The function of processing passengers, crews and their belongings, and the detection and interception of suspect illegal activity, at the border. Includes referral of matters (eg quarantine, immigration, permit requirements) to other agencies; making of agreements (eg carrier access to Customs computer systems); ship and aircraft arrival/departure reporting; authorisation, including ship and aircraft movement and docking/landing approvals, appointment of ports, airports, wharves and boarding stations; enforcement, including detention and search of passengers; goods control; processing of passengers and non-dutiable belongings through Customs gateways." ;
    skos:inScheme :conceptScheme: ;
    skos:prefLabel "Travel Facilitation And Compliance" .

:0479  a crs:Function, ra:Class,
        skos:Concept ;
    crs:isPerformedBy [ crs:hasAgent ca:9294 ] ;
    dct:source ras:2009-00436141 ;
    skos:definition """The wage setting management core business involves the setting of federal minimum wages and classification wages.
This core business involves a process of wage reviews and wage setting decisions based on information gathered through research, consultation and submission processes.  This includes:
• Issuing wage determinations
• Conducting and commissioning research
• Producing reports
• Promoting the core business of the agency to stakeholders and managing enquiries
• Consulting with key stakeholders Australia-wide
• Establishing and participating in committees and organising meetings
• Seeking written public submissions.
To support this process, the agency develops internal policies and charters to govern the administration and operation of this core business.""";
    skos:inScheme :conceptScheme: ;
    skos:prefLabel "Wage-Setting Management" .

:0480  a crs:Function, ra:Class,
        skos:Concept ;
    crs:isPerformedBy [ crs:hasAgent ca:9296 ] ;
    dct:source ras:2009-00775639 ;
    skos:definition """The core business of reviewing systemic tax administration issues and reporting to Government on how to improve them.
Includes:
• reporting to the Minister with recommendations for improving tax administration for the benefit of all taxpayers
• researching, reviewing, monitoring, evaluating and carrying out studies relating to tax administration systems, including the conduct of the tax office or the underlying tax laws dealing with administrative matters
• receiving submissions relating to tax administration systems
• consulting with the community and accounting, tax, legal and business bodies
• consulting with key Commonwealth stakeholders such as the Commonwealth Ombudsman, the Commonwealth Auditor-General and head of Commonwealth taxation agency
• liaising with government agencies and tax officials

Excludes:
• reviewing taxation policy issues
• dealing with individual taxpayer matters""";
    skos:inScheme :conceptScheme: ;
    skos:prefLabel "Taxation Administration Reviewing" .

:0481  a crs:Function, ra:Class,
        skos:Concept ;
    crs:isPerformedBy [ crs:hasAgent ca:9297 ] ;
    dct:source ras:2009-00803813 ;
    skos:definition """The core business of managing the lodgement, assessment, variation and termination of workplace agreements.  Includes:
•	Receipt of applications, agreements, declarations and supporting documentation;
•	Assessments of agreements to ensure compliance with legislative requirements;
•	Handling of complaints and enquiries and the provision of advice in relation to lodged applications;
•	Development of policy and procedures on agreement making and assessment processes;
•	Handling of agreement assessment reconsideration requests and referrals.
•	Provision of advice and information to clients in association with their lodgement application.
Also includes the handling of other legal matters relating to a potential or current workplace agreement such as pre lodgement and post lodgement prohibited content reviews, authorisation of multiple business agreements, the issuing of bargaining agent certificates and transmission of business receipts.""";
    skos:inScheme :conceptScheme: ;
    skos:prefLabel "Agreement Processing" .

:0482  a crs:Function, ra:Class,
        skos:Concept ;
    crs:isPerformedBy [ crs:hasAgent ca:9305 ] ;
    dct:source ras:2010-00031012 ;
    skos:definition """The core business of managing compliance with workplace relations legislation in order to protect the rights and interests of employees and employers.  Includes:
•	Management of audits and targeted compliance campaigns;
•	Receipt and handling of complaints and claims of alleged breaches of workplace relations laws;
•	Handling investigations of breaches from complaints, claims and targeted compliance activities;
•	Resolution of complaints and claims through voluntary compliance, the issue of notices and/or legal action;
•	Development of compliance handling policies and procedures and customer service quality assurance reports.
""";
    skos:inScheme :conceptScheme: ;
    skos:prefLabel "Compliance Management" .

:0483  a crs:Function, ra:Class,
        skos:Concept ;
    crs:isPerformedBy [ crs:hasAgent ca:9305 ] ;
    dct:source ras:2010-00031012 ;
    skos:definition """The core business of managing internal and external corporate communication channels in order to facilitate access to information, advice, products and resources in relation to workplace relations matters.  Includes:
•	Handling of customer/client complaints, enquiries, feedback and suggestions;
•	Development of policies and procedures supporting corporate communications and knowledge services;
•	The dissemination of information via the organisation’s contact centres, website and other channels;
•	Management of programs and educational activities offering information, advice and assistance to individuals, industries and associations in relation to workplace relations rights and obligations.
Also includes the development of pay scale summaries and the research, analysis and summarising of data in order to provide technical information, advice and support to internal and external clients.
""";
    skos:inScheme :conceptScheme: ;
    skos:prefLabel "Corporate Communications & Knowledge Services" .
